theories/NewNames.v
@@ -68,16 +68,11 @@ Arguments count_acc acc f {T}/ m.
 Definition count := @count_acc 0.
 Arguments count/ f {T} m.
 
-(*
-Lemma pull_out_of_acc acc f {T} (m : Map.to T)
-  : count_acc acc f m = acc + count f m.
-Proof.
-  cbn. unfold Map.fold. repeat rewrite MapCore.fold_spec. remember (MapCore.bindings m) as b eqn:Eb; clear m Eb.
-  generalize dependent acc. induction b as [| [k v] tail IH]; intros; cbn in *. { symmetry. apply PeanoNat.Nat.add_0_r. }
-  repeat rewrite (IH $ _ _). rewrite PeanoNat.Nat.add_assoc. f_equal.
-  destruct f. { symmetry. apply PeanoNat.Nat.add_1_r. } unfold id. symmetry. apply PeanoNat.Nat.add_0_r.
-Qed.
-*)
+Definition count_acc_range acc {T} (f : T -> bool) : Map.to T -> nat := Map.fold (fun _ x => if f x then S else id) acc.
+Arguments count_acc_range acc {T} f/ m.
+
+Definition count_range := @count_acc_range 0.
+Arguments count_range/ {T} f m.
 
 Lemma pull_out_of_acc acc orig_name {T} (li : list (_ * T))
   : List.fold_left (fun a kv => (if prefix orig_name (fst kv) then S else id) a) li acc =
@@ -151,9 +146,169 @@ Proof. rewrite unfold_new_name. destruct (Map.in_spec reserved name). 2: { refle
 
 
 
-(* TODO: speed up by accumulating results of `range` call *)
-Definition generate_acc acc reserved : Map.set -> Map.to String.string :=
-  Map.fold (fun k _ acc => Map.overriding_add k (new_name (Map.set_union reserved (Map.range acc)) k) acc) acc.
+Lemma le_prime_r x {T} (tail : list (_ * T))
+  : List.fold_right (fun kv a => (if prefix (x ++ "'") $ fst kv then S else id) a) 0 tail < S $
+    List.fold_right (fun kv a => (if prefix  x         $ fst kv then S else id) a) 0 tail.
+Proof.
+  generalize dependent x. induction tail as [| [k v] tail IH]; intros; cbn in *. { constructor. }
+  destruct prefix eqn:Ep'. { apply prefix_acc in Ep' as ->. apply -> PeanoNat.Nat.succ_lt_mono. apply IH. }
+  destruct (prefix x k) eqn:Ep; cbn in *. 2: { apply IH. } eapply PeanoNat.Nat.lt_trans. { apply IH. }
+  apply -> PeanoNat.Nat.succ_lt_mono. apply PeanoNat.Nat.lt_succ_diag_r.
+Qed.
+
+
+
+Equations new_name_3_acc (reserved : Map.set) (acc : Map.to string) (tail : Map.set) (orig_name : string)
+  (* : string by wf (count (prefix orig_name) reserved + count_range (prefix orig_name) acc + count (prefix orig_name) tail) lt := *)
+  : string by wf (count (prefix orig_name) $ Map.set_union reserved $ Map.set_union tail $ Map.range acc) lt :=
+  new_name_3_acc reserved acc tail orig_name with
+    Map.found_dec reserved orig_name, Map.in_range_dec acc orig_name, Map.found_dec tail orig_name => {
+    | Map.NotFound, Map.NotFoundInRange, Map.NotFound => orig_name
+    | _, _, _ => new_name_3_acc reserved acc tail $ next orig_name
+  }.
+Next Obligation.
+  clear new_name_3_acc. destruct v. assert (F : Map.Find (Map.set_union reserved $ Map.set_union tail $ Map.range acc) orig_name tt). {
+    apply Map.union_set. right. apply Map.union_set. left. exact Y. }
+  clear Y refine refine0. apply MapCore.bindings_spec1 in F. apply SetoidList.InA_rev in F. cbn in F.
+  unfold Map.fold in *. repeat rewrite MapCore.fold_spec in *. repeat rewrite <- List.fold_left_rev_right in *.
+  remember (List.rev _) as b eqn:Eb; clear reserved acc tail Eb. induction b as [| [k v] tail IH]. { invert F. }
+  invert F; cbn in *. { destruct H0. cbn in *. subst. rewrite prefix_prime. rewrite prefix_refl. apply le_prime_r. }
+  destruct prefix eqn:Ep'. { apply prefix_acc in Ep' as ->. apply -> PeanoNat.Nat.succ_lt_mono. apply IH. exact H0. }
+  destruct (prefix orig_name k) eqn:Ep; cbn in *. 2: { apply IH. exact H0. }
+  eapply PeanoNat.Nat.lt_trans. { apply IH. exact H0. } apply PeanoNat.Nat.lt_succ_diag_r.
+Qed.
+Next Obligation.
+  clear new_name_3_acc. assert (F : Map.Find (Map.set_union reserved $ Map.set_union tail $ Map.range acc) orig_name tt). {
+    apply Map.union_set. right. apply Map.union_set. right. apply Map.find_range. exists Y. exact H. }
+  clear N Y H refine. apply MapCore.bindings_spec1 in F. apply SetoidList.InA_rev in F. cbn in F.
+  unfold Map.fold in *. repeat rewrite MapCore.fold_spec in *. repeat rewrite <- List.fold_left_rev_right in *.
+  remember (List.rev _) as b eqn:Eb; clear reserved acc tail Eb. induction b as [| [k v] tail IH]. { invert F. }
+  invert F; cbn in *. { destruct H0. cbn in *. subst. rewrite prefix_prime. rewrite prefix_refl. apply le_prime_r. }
+  destruct prefix eqn:Ep'. { apply prefix_acc in Ep' as ->. apply -> PeanoNat.Nat.succ_lt_mono. apply IH. exact H0. }
+  destruct (prefix orig_name k) eqn:Ep; cbn in *. 2: { apply IH. exact H0. }
+  eapply PeanoNat.Nat.lt_trans. { apply IH. exact H0. } apply PeanoNat.Nat.lt_succ_diag_r.
+Qed.
+Next Obligation.
+  clear new_name_3_acc. destruct v. assert (F : Map.Find (Map.set_union reserved $ Map.set_union tail $ Map.range acc) orig_name tt). {
+    apply Map.union_set. left. exact Y. } clear Y N N0.
+  apply MapCore.bindings_spec1 in F. apply SetoidList.InA_rev in F. cbn in F.
+  unfold Map.fold in *. repeat rewrite MapCore.fold_spec in *. repeat rewrite <- List.fold_left_rev_right in *.
+  remember (List.rev _) as b eqn:Eb; clear reserved acc tail Eb. induction b as [| [k v] tail IH]. { invert F. }
+  invert F; cbn in *. { destruct H0. cbn in *. subst. rewrite prefix_prime. rewrite prefix_refl. apply le_prime_r. }
+  destruct prefix eqn:Ep'. { apply prefix_acc in Ep' as ->. apply -> PeanoNat.Nat.succ_lt_mono. apply IH. exact H0. }
+  destruct (prefix orig_name k) eqn:Ep; cbn in *. 2: { apply IH. exact H0. }
+  eapply PeanoNat.Nat.lt_trans. { apply IH. exact H0. } apply PeanoNat.Nat.lt_succ_diag_r.
+Qed.
+Fail Next Obligation.
+
+Lemma in_acc_not_3_acc {reserved acc tail orig_name}
+  (IR : Map.InRange acc $ new_name_3_acc reserved acc tail orig_name)
+  : False.
+Proof.
+  destruct IR as [k F]. generalize dependent k.
+  funelim (new_name_3_acc reserved acc tail orig_name); intros; try solve [apply H in F as []].
+  apply N0. exists k. exact F.
+Qed.
+
+Lemma in_reserved_not_3_acc {reserved acc tail orig_name}
+  (I : Map.In reserved (new_name_3_acc reserved acc tail orig_name))
+  : False.
+Proof.
+  destruct I as [[] F].
+  funelim (new_name_3_acc reserved acc tail orig_name); repeat rewrite <- Heqcall in *; try solve [apply H in F as []].
+  eapply N1. exact F.
+Qed.
+
+Lemma unfold_3_acc reserved acc tail orig_name
+  : new_name_3_acc reserved acc tail orig_name =
+    if (Map.in_ reserved orig_name || Map.in_range acc orig_name || Map.in_ tail orig_name)%bool then
+      new_name_3_acc reserved acc tail $ next orig_name
+    else orig_name.
+Proof.
+  funelim (new_name_3_acc reserved acc tail orig_name).
+  - destruct (Map.in_spec tail orig_name). 2: { contradiction N. exists v. exact Y. } rewrite Bool.orb_true_r. reflexivity.
+  - destruct (Map.in_range_spec acc orig_name). 2: { contradiction N0. } rewrite Bool.orb_true_r. reflexivity.
+  - destruct (Map.in_spec reserved orig_name). 2: { contradiction N1. exists v. exact Y. } reflexivity.
+  - destruct (Map.in_spec reserved orig_name). { destruct Y as [[] Y]. contradiction (N1 tt). } rewrite Bool.orb_false_l.
+    destruct (Map.in_range_spec acc orig_name). { contradiction N0. } rewrite Bool.orb_false_l.
+    destruct (Map.in_spec tail orig_name). { destruct Y as [[] Y]. contradiction (N tt). } reflexivity.
+Qed.
+
+Lemma det_3_acc
+  {r1 r2} (Er : Map.Eq r1 r2)
+  {a1 a2} (Ea : Map.Eq a1 a2)
+  {t1 t2} (Et : Map.Eq t1 t2)
+  {n1 n2} (En : n1 = n2)
+  : new_name_3_acc r1 a1 t1 n1 = new_name_3_acc r2 a2 t2 n2.
+Proof.
+  subst. rename n2 into n. funelim (new_name_3_acc r1 a1 t1 n).
+  - specialize (H _ Er _ Ea _ Et). rewrite (unfold_3_acc r2). destruct (Map.in_spec r2 orig_name); cbn. { exact H. }
+    destruct (Map.in_range_spec a2 orig_name); cbn. { exact H. }
+    destruct (Map.in_spec t2 orig_name); cbn. { exact H. } contradiction N1. exists v. apply Et. exact Y.
+  - specialize (H _ Er _ Ea _ Et). rewrite (unfold_3_acc r2). destruct (Map.in_spec r2 orig_name); cbn. { exact H. }
+    destruct (Map.in_range_spec a2 orig_name); cbn. { exact H. }
+    contradiction N1. destruct Y as [k F]. exists k. apply Ea. exact F.
+  - specialize (H _ Er _ Ea _ Et). rewrite (unfold_3_acc r2). destruct (Map.in_spec r2 orig_name); cbn. { exact H. }
+    contradiction N1. exists v. apply Er. exact Y.
+  - rewrite unfold_3_acc. destruct (Map.in_spec r2 orig_name); cbn. {
+      destruct Y as [[] F]. contradiction (N1 tt). apply Er. exact F. }
+    destruct (Map.in_range_spec a2 orig_name); cbn. {
+      destruct Y as [k F]. contradiction N0. exists k. apply Ea. exact F. }
+    destruct (Map.in_spec t2 orig_name); cbn. { destruct Y as [[] F]. contradiction (N tt). apply Et. exact F. } reflexivity.
+Qed.
+
+
+
+(* If a binding is *itself* in `tail`, let it pass; however, from then on out, we care if it would shadow another, so recurse: *)
+Definition new_name_3 reserved acc tail orig_name :=
+  if orb (Map.in_ reserved orig_name) $ Map.in_range acc orig_name then
+    new_name_3_acc reserved acc tail $ next orig_name
+  else orig_name.
+
+Lemma in_acc_not_3 {reserved acc tail orig_name}
+  (IR : Map.InRange acc $ new_name_3 reserved acc tail orig_name)
+  : False.
+Proof.
+  unfold new_name_3 in IR. destruct (Map.in_spec reserved orig_name); cbn in *. { eapply in_acc_not_3_acc. exact IR. }
+  destruct (Map.in_range_spec acc orig_name). 2: { apply N0. exact IR. }
+  clear N Y. remember (orig_name ++ "'")%string as x eqn:Ex; clear orig_name Ex. eapply in_acc_not_3_acc. exact IR.
+Qed.
+
+Lemma in_reserved_not_3 {reserved acc tail orig_name}
+  (I : Map.In reserved (new_name_3 reserved acc tail orig_name))
+  : False.
+Proof.
+  unfold new_name_3 in I. destruct (Map.in_spec reserved orig_name); cbn in *. { eapply in_reserved_not_3_acc. exact I. }
+  destruct (Map.in_range_spec acc orig_name). 2: { apply N in I as []. }
+  clear N Y. remember (orig_name ++ "'")%string as x eqn:Ex; clear orig_name Ex. eapply in_reserved_not_3_acc. exact I.
+Qed.
+
+Lemma det_3
+  {r1 r2} (Er : Map.Eq r1 r2)
+  {a1 a2} (Ea : Map.Eq a1 a2)
+  {t1 t2} (Et : Map.Eq t1 t2)
+  {n1 n2} (En : n1 = n2)
+  : new_name_3 r1 a1 t1 n1 = new_name_3 r2 a2 t2 n2.
+Proof.
+  subst. rename n2 into n. unfold new_name_3. destruct (Map.in_spec r1 n); cbn;
+  destruct (Map.in_spec r2 n); try solve [contradiction N; destruct Y as [[] F]; exists tt; apply Er; exact F];
+  cbn. { apply det_3_acc; try assumption. reflexivity. }
+  destruct (Map.in_range_spec a1 n); cbn;
+  destruct (Map.in_range_spec a2 n); try solve [destruct Y as [k F]; contradiction N1; exists k; apply Ea; exact F];
+  cbn. 2: { reflexivity. } apply det_3_acc; try eassumption. reflexivity.
+Qed.
+
+Lemma new_name_3_id {reserved acc tail name} (Nr : ~Map.In reserved name) (Na : ~Map.InRange acc name)
+  : new_name_3 reserved acc tail name = name.
+Proof.
+  unfold new_name_3. destruct (Map.in_spec reserved name); cbn in *. { apply Nr in Y as []. }
+  destruct (Map.in_range_spec acc name); cbn in *. { apply Na in Y as []. } reflexivity.
+Qed.
+
+
+
+Definition generate_acc acc reserved names :=
+  Map.fold (fun k _ acc => Map.overriding_add k (new_name_3 reserved acc names k) acc) acc names.
 Arguments generate_acc acc reserved names/.
 
 Definition generate : Map.set -> Map.set -> Map.to String.string := generate_acc Map.empty.
@@ -164,23 +319,25 @@ Arguments generate reserved names/.
 Lemma in_generate_acc acc reserved names k
   : Map.In (generate_acc acc reserved names) k <-> (Map.In names k \/ Map.In acc k).
 Proof.
-  cbn. unfold Map.fold. rewrite MapCore.fold_spec. assert (Iff
-    : ((exists v, Map.Find names k v) \/ (exists v, Map.Find acc k v)) <->
-      ((exists v, SetoidList.InA MapCore.eq_key_elt (k, v) (MapCore.bindings names)) \/ (exists v, Map.Find acc k v))). {
-    split; (intros [[v F] | [v F]]; [left | right]; exists v; [| exact F]); apply MapCore.bindings_spec1; exact F. }
-  rewrite Iff; clear Iff. remember (MapCore.bindings names) as b eqn:Eb; clear names Eb; rename b into names.
-  generalize dependent k. generalize dependent reserved. generalize dependent acc.
-  induction names as [| [k v] tail]; intros. {
-    cbn. split. { intros [v F]. right. exists v. exact F. }
-    intros [[v F] | [v F]]. 2: { exists v. exact F. } invert F. }
-  rename k0 into x. cbn. rewrite IHtail; clear IHtail. split; intros [[y F] | [y F]].
-  - left. exists y. right. exact F.
-  - apply Map.find_overriding_add in F as [[-> ->] | [N F]]. 2: { right. exists y. exact F. }
-    left. exists v. left. split; reflexivity.
-  - invert F. 2: { left. eexists. eassumption. }
-    destruct H0; cbn in *; subst. right. eexists. apply Map.find_overriding_add. left. split; reflexivity.
-  - right. destruct (String.eqb_spec x k); subst; eexists; apply Map.find_overriding_add;
-    [left | right]. { split; reflexivity. } split; eassumption.
+  unfold generate_acc. unfold Map.fold. rewrite MapCore.fold_spec. rewrite <- List.fold_left_rev_right.
+  assert (I : Map.In names k <-> exists v, SetoidList.InA MapCore.eq_key_elt (k, v) (List.rev (MapCore.bindings names))); [|
+    rewrite I; clear I]. { split; intros [v F]; exists v. { apply SetoidList.InA_rev. apply MapCore.bindings_spec1. exact F. }
+    apply MapCore.bindings_spec1. apply SetoidList.InA_rev. exact F. }
+  remember names as all_names eqn:En. apply (f_equal MapCore.bindings) in En. repeat rewrite En. clear En.
+  remember (List.rev (MapCore.bindings names)) as b eqn:Eb. generalize dependent k. generalize dependent names.
+  generalize dependent reserved. generalize dependent acc. induction b as [| [k v] tail IH]; intros; cbn in *. {
+    split. { intro I. right. exact I. } intros [[[] F] | I]. { invert F. } exact I. }
+  eassert (E : _); [| specialize (IH acc reserved (Map.remove k names) E k0)]. {
+    rewrite Map.bindings_remove. rewrite Utils.filter_rev. rewrite <- Eb. cbn. rewrite String.eqb_refl. cbn.
+    assert (ND := MapCore.bindings_spec2w names). apply SetoidList.NoDupA_rev in ND. 2: { exact Map.eq_key_equiv. }
+    rewrite <- Eb in ND. invert ND. symmetry. apply List.forallb_filter_id. apply List.forallb_forall. intros [k' v'] I.
+    cbn in *. destruct (String.eqb_spec k k'). 2: { reflexivity. } subst. contradiction H1.
+    apply SetoidList.InA_alt. exists (k', v'). split. { reflexivity. } exact I. }
+  rewrite Map.in_overriding_add. split.
+  - intros [-> | I]. { left. exists v. left. split; reflexivity. }
+    destruct IH as [[[v0 IH] | IH] _]. { exact I. } { left. exists v0. right. exact IH. } right. exact IH.
+  - intros [[v0 F] | I]. { invert F; [left | right]. { apply H0. } apply IH. left. exists v0. exact H0. }
+    right. apply IH. right. exact I.
 Qed.
 
 Lemma in_generate reserved names k
@@ -203,62 +360,6 @@ Proof.
   edestruct IH as [IH' | IH']; clear IH; [| left | right]. { exact F. } { exact IH'. } right. exact IH'.
 Qed.
 
-Lemma in_range_generate_acc {acc} (O2O : Map.OneToOne acc) {x y} (F : Map.Find acc x y) {names} (N : ~Map.In names x) reserved
-  : Map.InRange (generate_acc acc reserved names) y.
-Proof.
-  unfold generate_acc. unfold Map.fold. rewrite MapCore.fold_spec. rewrite <- List.fold_left_rev_right.
-  assert (N' : ~SetoidList.InA MapCore.eq_key_elt (x, tt) $ List.rev (MapCore.bindings names)). {
-    intro I. apply N. eexists. apply MapCore.bindings_spec1. apply SetoidList.InA_rev. exact I. } clear N. rename N' into N.
-  assert (ND := MapCore.bindings_spec2w names). apply SetoidList.NoDupA_rev in ND.
-  remember (List.rev (MapCore.bindings names)) as b eqn:Eb; clear names Eb.
-  generalize dependent reserved. generalize dependent y. generalize dependent x. generalize dependent acc.
-  induction ND as [| [k []] tail N ND IH]; intros; cbn in *. { exists x. exact F. }
-  edestruct IH as [x' IH']; clear IH; try eassumption. 3: { exact Map.eq_key_equiv. } { intro I. apply N0. right. exact I. }
-  eexists. apply Map.overwrite_if_present_overwrite. right. split. 2: { exact IH'. }
-  intros ->. apply in_right in IH' as [IH | IH]. 2: { apply N in IH as []. }
-  specialize (O2O _ _ F _ IH) as ->. apply N0. left. split; reflexivity.
-Qed.
-
-Lemma not_in_generate_acc
-  reserved x (R : Map.In reserved x)
-  acc (N : forall k (R : Map.In reserved k) (A : Map.InRange acc k), False)
-  names (G : Map.InRange (generate_acc acc reserved names) x)
-  : False.
-Proof.
-  cbn in G. destruct G as [y G]. unfold Map.fold in G. rewrite MapCore.fold_spec in G.
-  remember (MapCore.bindings names) as b eqn:Eb; clear names Eb; rename b into names.
-  generalize dependent y. generalize dependent acc. generalize dependent x. generalize dependent reserved.
-  induction names as [| [k v] tail]; intros. { cbn in *. destruct R. eapply N; eexists; eassumption. }
-  simpl List.fold_left in G. apply IHtail in G as []; clear IHtail. { exact R. }
-  intros z Rz I. destruct I as [z' F]. apply Map.find_overriding_add in F as [[-> ->] | [Nz F]].
-  - eapply not_in_new_name. apply Map.in_overriding_union. left. exact Rz.
-  - eapply N. { exact Rz. } eexists. exact F.
-Qed.
-
-Lemma not_in_generate
-  reserved k (R : Map.In reserved k)
-  names (G : Map.InRange (generate reserved names) k)
-  : False.
-Proof. eapply not_in_generate_acc; try eassumption. intros x I [y C]. invert C. Qed.
-
-Lemma generate_acc_det {a1 a2} (Ea : a1 = a2) {r1 r2} (Er : Map.Eq r1 r2) {n1 n2} (En : Map.Eq n1 n2)
-  : generate_acc a1 r1 n1 = generate_acc a2 r2 n2.
-Proof.
-  unfold generate_acc. unfold Map.fold. repeat rewrite MapCore.fold_spec. apply Map.bindings_eq in En.
-  remember (MapCore.bindings n1) as b1 eqn:E1; clear n1 E1; rename b1 into n1.
-  remember (MapCore.bindings n2) as b2 eqn:E2; clear n2 E2; rename b2 into n2.
-  subst. rename n2 into names. generalize dependent r2. generalize dependent r1. generalize dependent a2.
-  induction names as [| [k v] tail IH]; intros; cbn in *. { reflexivity. }
-  erewrite IH; clear IH. 2: { exact Er. } erewrite new_name_det. { reflexivity. }
-  intros k' v'. repeat rewrite Map.find_iff. repeat rewrite Map.find_overriding_union.
-  destruct (Map.find_spec r1 k'). { apply Er in Y. apply Map.find_iff in Y. rewrite Y. reflexivity. }
-  destruct (Map.find_spec r2 k'). { apply Er in Y. apply N in Y as []. } reflexivity.
-Qed.
-
-Lemma generate_det {r1 r2} (Er : Map.Eq r1 r2) {n1 n2} (En : Map.Eq n1 n2)
-  : generate r1 n1 = generate r2 n2.
-Proof. apply generate_acc_det; try assumption. reflexivity. Qed.
-
 Lemma unfold_right {X Y} f (acc : Y) (hd : X) tl
   : List.fold_right f acc (List.cons hd tl) = f hd (List.fold_right f acc tl).
 Proof. reflexivity. Qed.
@@ -267,26 +368,106 @@ Lemma unfold_left {X Y} f (acc : Y) (hd : X) tl
   : List.fold_left f (List.cons hd tl) acc = List.fold_left f tl (f acc hd).
 Proof. reflexivity. Qed.
 
+
+
 Theorem one_to_one_generate_acc {acc} (O2O : Map.OneToOne acc) reserved names
   : Map.OneToOne (generate_acc acc reserved names).
 Proof.
-  unfold generate_acc. unfold Map.fold. rewrite MapCore.fold_spec. assert (ND := MapCore.bindings_spec2w names).
-  remember (MapCore.bindings names) as b eqn:Eb; clear names Eb; rename b into names.
-  generalize dependent reserved. generalize dependent acc.
-  induction ND as [| [head []] tail N ND IH]; intros. { simpl List.fold_left. exact O2O. }
-  rewrite unfold_left. simpl fst. apply IH; clear IH.
-  intro; intros. apply Map.find_overriding_add in F1 as [[-> ->] | [N1 F1]].
-  - apply Map.find_overriding_add in F2 as [[-> _] | [N2 F2]]. { reflexivity. }
-    eassert (IR : Map.InRange acc _). { eexists. exact F2. } apply Map.in_range in IR.
-    eapply or_intror in IR. apply Map.in_overriding_union in IR. apply not_in_new_name in IR as [].
-  - apply Map.find_overriding_add in F2 as [[-> ->] | [N2 F2]]. 2: { eapply O2O; eassumption. }
-    eassert (IR : Map.InRange acc _). { eexists. exact F1. } apply Map.in_range in IR.
-    eapply or_intror in IR. apply Map.in_overriding_union in IR. apply not_in_new_name in IR as [].
+  unfold generate_acc. unfold Map.fold. rewrite MapCore.fold_spec.
+  remember names as all_names eqn:En. remember (MapCore.bindings names) as b eqn:Eb.
+  apply (f_equal MapCore.bindings) in En. repeat rewrite En. clear En. repeat rewrite <- Eb in *. clear names Eb.
+  generalize dependent all_names. generalize dependent reserved. generalize dependent acc.
+  induction b as [| [head []] tail IH]; intros. { simpl List.fold_left. exact O2O. }
+  rewrite unfold_left. simpl fst. apply IH; clear IH. unfold Map.OneToOne. intros.
+  apply Map.find_overriding_add in F1 as [[-> ->] | [N1 F1]]; apply Map.find_overriding_add in F2 as [[-> E'] | [N2 F2]];
+  cbn in *; subst. { reflexivity. }
+  - edestruct @in_acc_not_3 as []. exists k2. exact F2.
+  - edestruct @in_acc_not_3 as []. exists k1. exact F1.
+  - eapply O2O. { exact F1. } exact F2.
 Qed.
 
 Theorem one_to_one_generate reserved names
   : Map.OneToOne (generate reserved names).
 Proof. apply one_to_one_generate_acc. apply Map.one_to_one_empty. Qed.
+
+Lemma fold_left_extn {X Y} {f1 f2 : Y -> X -> Y} (Ef : forall y x, f1 y x = f2 y x) li acc
+  : List.fold_left f1 li acc = List.fold_left f2 li acc.
+Proof.
+  generalize dependent Y. induction li as [| head tail IH]; intros. { reflexivity. }
+  cbn. rewrite Ef. apply IH. exact Ef.
+Qed.
+
+
+
+Lemma generate_acc_det {a1 a2} (Ea : a1 = a2) {r1 r2} (Er : Map.Eq r1 r2) {n1 n2} (En : Map.Eq n1 n2)
+  : generate_acc a1 r1 n1 = generate_acc a2 r2 n2.
+Proof.
+  subst. rename a2 into acc. unfold generate_acc. unfold Map.fold. repeat rewrite MapCore.fold_spec.
+  assert (Eb := En). apply Map.bindings_eq in Eb. rewrite Eb. erewrite fold_left_extn. { reflexivity. }
+  intros y [x []]. cbn. f_equal. apply det_3; try assumption. { apply Map.eq_refl. } reflexivity.
+Qed.
+
+Lemma generate_det {r1 r2} (Er : Map.Eq r1 r2) {n1 n2} (En : Map.Eq n1 n2)
+  : generate r1 n1 = generate r2 n2.
+Proof. apply generate_acc_det; try assumption. reflexivity. Qed.
+
+
+
+Lemma not_in_generate_acc
+  reserved y (R : Map.In reserved y)
+  acc (N : forall k (R : Map.In reserved k) (A : Map.InRange acc k), False)
+  names (G : Map.InRange (generate_acc acc reserved names) y)
+  : False.
+Proof.
+  destruct G as [x F]. unfold generate_acc in F. unfold Map.fold in F. rewrite MapCore.fold_spec in F.
+  remember names as all_names eqn:En in F at 1. clear En.
+  remember (MapCore.bindings names) as b eqn:Eb; clear names Eb; rename b into names. generalize dependent x.
+  generalize dependent acc. generalize dependent y. generalize dependent reserved. generalize dependent all_names.
+  induction names as [| [k v] tail]; intros. { cbn in *. destruct R as [z R]. eapply N; eexists; eassumption. }
+  rewrite unfold_left in F. simpl fst in F. apply IHtail in F as []; clear IHtail. { exact R. }
+  intros z Rz I. destruct I as [z' F']. apply Map.find_overriding_add in F' as [[-> ->] | [Nz F']].
+  - eapply in_reserved_not_3 in Rz as [].
+  - eapply N. { exact Rz. } eexists. exact F'.
+Qed.
+
+Lemma not_in_generate
+  reserved k (R : Map.In reserved k)
+  names (G : Map.InRange (generate reserved names) k)
+  : False.
+Proof. eapply not_in_generate_acc; try eassumption. intros x I [y C]. invert C. Qed.
+
+(*
+Lemma in_range_generate_acc {acc} (O2O : Map.OneToOne acc) {x y} (F : Map.Find acc x y) {names} (N : ~Map.In names x) reserved
+  : Map.InRange (generate_acc acc reserved names) y.
+Proof.
+  unfold generate_acc. unfold Map.fold. rewrite MapCore.fold_spec. rewrite <- List.fold_left_rev_right.
+  assert (Nn := N). remember names as all_names eqn:En. rewrite En in N. apply (f_equal MapCore.bindings) in En.
+  repeat rewrite En. clear En. assert (N' : ~SetoidList.InA MapCore.eq_key_elt (x, tt) $ List.rev (MapCore.bindings names)). {
+    intro I. apply N. eexists. apply MapCore.bindings_spec1. apply SetoidList.InA_rev. exact I. } clear N. rename N' into N.
+  assert (ND := MapCore.bindings_spec2w names). apply SetoidList.NoDupA_rev in ND. 2: { exact Map.eq_key_equiv. }
+  remember (List.rev (MapCore.bindings names)) as b eqn:Eb. generalize dependent reserved.
+  generalize dependent names. generalize dependent y. generalize dependent x. generalize dependent acc.
+  induction ND as [| [k []] tail N ND IH]; intros; cbn in *. { exists x. exact F. } (*
+  eassert (N' : _); [| eassert (E : _); [| specialize (IH _ O2O x Nn N' _ F (Map.remove k names) E reserved)
+    as [k' IH]]]. { intro I. apply N0. right. exact I. } {
+    rewrite Map.bindings_remove. rewrite Utils.filter_rev. rewrite <- Eb. cbn. rewrite String.eqb_refl. cbn.
+    assert (ND' := MapCore.bindings_spec2w names). apply SetoidList.NoDupA_rev in ND'. 2: { exact Map.eq_key_equiv. }
+    rewrite <- Eb in ND'. invert ND'. symmetry. apply List.forallb_filter_id. apply List.forallb_forall. intros [k' v'] I.
+    cbn in *. destruct (String.eqb_spec k k'). 2: { reflexivity. } subst. contradiction H1.
+    apply SetoidList.InA_alt. exists (k', v'). split. { reflexivity. } exact I. } *)
+  destruct (String.eqb_spec y $ new_name_3 reserved (List.fold_right (fun y0 x0 => Map.overriding_add (fst y0)
+    (new_name_3 reserved x0 all_names (fst y0)) x0) acc tail) all_names k). {
+    exists k. apply Map.overwrite_if_present_overwrite. left. split. { reflexivity. } exact e. }
+  edestruct IH as [k' IH']; clear IH. 6: { exists k'. apply Map.overwrite_if_present_overwrite. right.
+    split. 2: { exact IH'. } { intros ->. apply N0. left. split; reflexivity. }
+
+
+
+  edestruct IH as [x' IH']; clear IH; try eassumption. { intro I. apply N0. right. exact I. }
+  eexists. apply Map.overwrite_if_present_overwrite. right. split. 2: { exact IH'. }
+  intros ->. apply in_right in IH' as [IH | IH]. 2: { apply N in IH as []. }
+  specialize (O2O _ _ F _ IH) as ->. apply N0. left. split; reflexivity.
+Qed.
 
 (*
 Lemma in_acc_right {acc k v} (F : Map.Find acc k v) reserved tail
@@ -354,3 +535,16 @@ Proof.
   apply range_generate_acc. { exact N. } { exact I. } { apply Map.one_to_one_empty. }
   intros k In C. apply Map.empty_empty in C as [].
 Qed.
+
+Lemma generate_acc_id {acc reserved names k v} (F : Map.Find (generate_acc acc reserved names) k v)
+  (N : forall (I : Map.In reserved k), False) (Na : forall v' (F' : Map.Find acc k v'), v' = k)
+  : v = k.
+Proof.
+  unfold generate_acc in F. unfold Map.fold in F. rewrite MapCore.fold_spec in F. rewrite <- List.fold_left_rev_right in F.
+  remember (List.rev (MapCore.bindings names)) as b eqn:Eb; clear names Eb. generalize dependent v. generalize dependent k.
+  generalize dependent reserved. generalize dependent acc. induction b as [| [k v] tail IH]; intros; cbn in *. { apply Na. exact F. }
+  apply Map.overwrite_if_present_overwrite in F as [[-> ->] | [NF F]]. 2: { eapply IH. { exact N. } { exact Na. } exact F. }
+  eapply new_name_id. intro I. apply Map.in_overriding_union in I as [I | I]. { apply N in I as []. }
+  apply Map.in_range in I as [j F]. specialize (IH _ _ _ N Na _ F).
+Qed.
+*)
