theories/Unshadow.v
@@ -18,41 +18,42 @@ Fixpoint unshadow_acc (acc : Map.to String.string) (cant_bind : Map.set) t :=
   | Term.Ctr ctor => Some (cant_bind, Term.Ctr ctor)
   | Term.Var k ownership =>
       (* Have to supply a plan for any free variables (or they have to have been bound & added to the plan): *)
-      match Map.find acc k with None => None | Some v => Some (cant_bind, Term.Var v ownership) end
+      match Map.find acc k with None => None | Some v => Some (Map.set_add v cant_bind, Term.Var v ownership) end
   | Term.App f a =>
-      match unshadow_acc acc cant_bind f with None => None | Some (cant_bind, f') =>
-        match unshadow_acc acc cant_bind a with None => None | Some (cant_bind, a') =>
-          Some (cant_bind, Term.App f' a')
+      match unshadow_acc acc cant_bind f with None => None | Some (bound_or_used_f, f') =>
+        match unshadow_acc acc bound_or_used_f a with None => None | Some (bound_or_used_a, a') =>
+          Some (bound_or_used_a, Term.App f' a')
         end
       end
   | Term.For variable type body =>
-      match unshadow_acc acc cant_bind type with None => None | Some (cant_bind, type') =>
-        let variable' := NewNames.new_name cant_bind variable in
-        let acc := Map.overwrite variable variable' acc in
-        let cant_bind := Map.set_add variable' cant_bind in
-        match unshadow_acc acc cant_bind body with None => None | Some (cant_bind, body') =>
-          Some (cant_bind, Term.For variable' type' body')
+      let variable' := NewNames.new_name cant_bind variable in
+      let cant_bind_v := Map.set_add variable' cant_bind in
+      match unshadow_acc acc cant_bind_v type with None => None | Some (bound_or_used_t, type') =>
+        let acc' := Map.overwrite variable variable' acc in
+        match unshadow_acc acc' bound_or_used_t body with None => None | Some (bound_or_used_b, body') =>
+          Some (bound_or_used_b, Term.For variable' type' body')
         end
       end
   | Term.Cas pattern body_if_match other_cases =>
-      match unshadow_acc acc cant_bind other_cases with None => None | Some (cant_bind, other_cases') =>
-        let bindings := BoundIn.pattern pattern in
-        let rebindings := NewNames.generate cant_bind bindings in
+      let rebindings := NewNames.generate cant_bind (BoundIn.pattern pattern) in
+      let cant_bind_p := Map.set_union (Map.range rebindings) cant_bind in
+      match unshadow_acc acc cant_bind_p other_cases with None => None | Some (bound_or_used_o, other_cases') =>
         match Rename.pattern rebindings pattern with
         | None => None
         | Some pattern' =>
-            let acc := Map.bulk_overwrite rebindings acc in
-            let cant_bind := Map.set_union (Map.range rebindings) cant_bind in
-            match unshadow_acc acc cant_bind body_if_match with None => None | Some (cant_bind, body_if_match') =>
-              Some (cant_bind, Term.Cas pattern' body_if_match' other_cases')
+            let acc' := Map.bulk_overwrite rebindings acc in
+            match unshadow_acc acc' bound_or_used_o body_if_match with None => None | Some (bound_or_used_b, body_if_match') =>
+              Some (bound_or_used_b, Term.Cas pattern' body_if_match' other_cases')
             end
         end
       end
   end.
 
 Definition unshadow_reserve_bindings cant_bind t :=
-  let generated := NewNames.generate cant_bind $ UsedIn.term t in
-  unshadow_acc generated (Map.set_union cant_bind $ Map.range generated) t.
+  (* let generated := NewNames.generate cant_bind $ UsedIn.term t in *)
+  let used := UsedIn.term t in
+  let generated := Map.to_self used in
+  unshadow_acc generated (Map.set_union cant_bind used) t.
 Arguments unshadow_reserve_bindings cant_bind t/.
 
 Definition unshadow_reserve cant_bind t := option_map snd $ unshadow_reserve_bindings cant_bind t.
@@ -60,6 +61,47 @@ Arguments unshadow_reserve cant_bind t/.
 
 Definition unshadow := unshadow_reserve Map.empty.
 Arguments unshadow/ t.
+
+
+
+Lemma unshadow_app acc cant_bind f a
+  : unshadow_acc acc cant_bind (Term.App f a) =
+    match unshadow_acc acc cant_bind f with None => None | Some (bound_or_used_f, f') =>
+      match unshadow_acc acc bound_or_used_f a with None => None | Some (bound_or_used_a, a') =>
+        Some (bound_or_used_a, Term.App f' a')
+      end
+    end.
+Proof. reflexivity. Qed.
+
+Lemma unshadow_for acc cant_bind variable type body
+  : unshadow_acc acc cant_bind (Term.For variable type body) =
+    match
+      unshadow_acc acc (Map.set_add (NewNames.new_name cant_bind variable) cant_bind) type
+    with None => None | Some (bound_or_used_t, type') =>
+      match
+        unshadow_acc (Map.overwrite variable (NewNames.new_name cant_bind variable) acc) bound_or_used_t body
+      with None => None | Some (bound_or_used_b, body') =>
+        Some (bound_or_used_b, Term.For (NewNames.new_name cant_bind variable) type' body')
+      end
+    end.
+Proof. reflexivity. Qed.
+
+Lemma unshadow_cas acc cant_bind pattern body_if_match other_cases
+  : unshadow_acc acc cant_bind (Term.Cas pattern body_if_match other_cases) =
+    match
+      unshadow_acc acc (Map.set_union (Map.range $ NewNames.generate cant_bind (BoundIn.pattern pattern)) cant_bind) other_cases
+    with None => None | Some (bound_or_used_o, other_cases') =>
+      match
+        Rename.pattern (NewNames.generate cant_bind (BoundIn.pattern pattern)) pattern
+      with None => None | Some pattern' =>
+          match
+            unshadow_acc (Map.bulk_overwrite (NewNames.generate cant_bind (BoundIn.pattern pattern)) acc) bound_or_used_o body_if_match
+          with None => None | Some (bound_or_used_b, body_if_match') =>
+            Some (bound_or_used_b, Term.Cas pattern' body_if_match' other_cases')
+          end
+      end
+    end.
+Proof. reflexivity. Qed.
 
 
 
@@ -111,141 +153,108 @@ Lemma det_acc
   : Equiv (unshadow_acc a1 r1 t1) (unshadow_acc a2 r2 t2).
 Proof.
   subst. rename t2 into t. generalize dependent r2. generalize dependent r1.
-  generalize dependent a2. generalize dependent a1. { induction t; intros; cbn in *.
+  generalize dependent a2. generalize dependent a1. induction t; intros.
   - constructor; assumption.
   - unfold unshadow_acc. destruct (Map.find_spec a1 name).
-    + apply Ea in Y. apply Map.find_iff in Y. rewrite Y. constructor. exact Er.
+    + apply Ea in Y. apply Map.find_iff in Y. rewrite Y. constructor. intros k [].
+      split; (intro F; apply Map.add_set; apply Map.add_set in F as [[-> _] | F];
+        [left | right]; [split; reflexivity | apply Er; exact F]).
     + destruct (Map.find_spec a2 name). { apply Ea in Y. apply N in Y as []. } constructor.
-  - destruct (IHt1 _ _ Ea _ _ Er). { constructor. }
+  - cbn. destruct (IHt1 _ _ Ea _ _ Er). { constructor. }
     destruct (IHt2 _ _ Ea _ _ Ecant_bind); constructor; eassumption.
-  - destruct (IHt1 _ _ Ea _ _ Er). { constructor. } eassert (Ea' : _); [| eassert (Er' : _); [| destruct (IHt2
-      (Map.overriding_add variable (NewNames.new_name cant_bind1 variable) a1)
-      (Map.overriding_add variable (NewNames.new_name cant_bind2 variable) a2) Ea'
-      (Map.overriding_add (NewNames.new_name cant_bind1 variable) tt cant_bind1)
-      (Map.overriding_add (NewNames.new_name cant_bind2 variable) tt cant_bind2) Er')]]. 3: { constructor. }
-    + split; intro F; apply Map.find_overriding_add; (apply Map.find_overriding_add in F as [[-> ->] | [N F]]; [left | right];
-      [split; [reflexivity | apply NewNames.new_name_det] | split; [exact N |]; apply Ea; exact F]); [| apply Map.eq_sym]; exact Ecant_bind.
-    + split; intro F; apply Map.find_overriding_add; (apply Map.find_overriding_add in F as [[-> ->] | [N F]]; [left | right];
-      [split; [| reflexivity]; apply NewNames.new_name_det | split; [| apply Ecant_bind; exact F];
-        intros ->; contradiction N; apply NewNames.new_name_det]); try exact Ecant_bind; apply Map.eq_sym; exact Ecant_bind.
-    + erewrite NewNames.new_name_det. { constructor. exact Ecant_bind0. } exact Ecant_bind.
-  - destruct (IHt2 _ _ Ea _ _ Er). { constructor. } destruct Rename.pattern eqn:ER. 2: {
-      destruct Rename.pattern eqn:ER2 at 1. 2: { constructor. }
-      eapply (Rename.pattern_iff (NewNames.one_to_one_generate _ _)) in ER2.
-      eapply (@Rename.pattern_eq _ (NewNames.one_to_one_generate _ _)) in ER2; try reflexivity.
-      * eapply Rename.pattern_iff in ER2. rewrite ER2 in ER. discriminate ER.
-      * erewrite <- NewNames.generate_det. { apply Map.eq_refl. } { exact Ecant_bind. } apply Map.eq_refl. }
-    apply (Rename.pattern_iff (NewNames.one_to_one_generate _ _)) in ER.
-    eapply (@Rename.pattern_eq _ (NewNames.one_to_one_generate _ _)) in ER; try reflexivity; [
-      eapply Rename.pattern_iff in ER; rewrite ER; clear ER |
-      erewrite NewNames.generate_det; try apply Map.eq_refl; exact Ecant_bind].
-    eassert (Ea' : _); [| eassert (Er' : _); [| destruct (IHt1
-      (Map.overriding_union (Map.fold (fun k _ acc => Map.overriding_add k (NewNames.new_name
-        (Map.overriding_union cant_bind1 $ Map.fold (fun _ v acc0 => Map.overriding_add v tt acc0) Map.empty acc) k) acc)
-        Map.empty (BoundIn.pattern pattern)) a1)
-      (Map.overriding_union (Map.fold (fun k _ acc => Map.overriding_add k (NewNames.new_name
-        (Map.overriding_union cant_bind2 $ Map.fold (fun _ v acc0 => Map.overriding_add v tt acc0) Map.empty acc) k) acc)
-        Map.empty (BoundIn.pattern pattern)) a2) Ea'
-      (Map.overriding_union (Map.fold (fun _ v acc => Map.overriding_add v tt acc) Map.empty
-        (Map.fold (fun k _ acc => Map.overriding_add k (NewNames.new_name (Map.overriding_union cant_bind1
-          (Map.fold (fun _ v acc0 => Map.overriding_add v tt acc0) Map.empty acc)) k) acc)
-          Map.empty (BoundIn.pattern pattern))) cant_bind1)
-      (Map.overriding_union (Map.fold (fun _ v acc => Map.overriding_add v tt acc) Map.empty
-        (Map.fold (fun k _ acc => Map.overriding_add k (NewNames.new_name (Map.overriding_union cant_bind2
-          (Map.fold (fun _ v acc0 => Map.overriding_add v tt acc0) Map.empty acc)) k) acc)
-          Map.empty (BoundIn.pattern pattern))) cant_bind2) Er')]]. 3: { constructor. }
-    + assert (G := @NewNames.generate_det). cbn in G. erewrite G.
-      * split; intro F; apply Map.bulk_overwrite_bulk_overwrite;
-        (apply Map.bulk_overwrite_bulk_overwrite in F as [F | [N F]]; [left; exact F | right]);
-        (split; [intro I; apply N; exact I |]; apply Ea; exact F).
-      * exact Ecant_bind.
-      * apply Map.eq_refl.
-    + assert (G := @NewNames.generate_det). cbn in G. erewrite G.
-      * split; intro F; apply Map.bulk_overwrite_bulk_overwrite;
-        (apply Map.bulk_overwrite_bulk_overwrite in F as [F | [N F]]; [left; exact F | right]);
-        (split; [intro I; apply N; exact I |]; apply Ecant_bind; exact F).
-      * exact Ecant_bind.
-      * apply Map.eq_refl.
-    + constructor. exact Ecant_bind0. }
-  Unshelve.
-  - apply NewNames.one_to_one_generate.
-  - apply NewNames.one_to_one_generate.
+  - repeat rewrite unshadow_for. specialize (IHt1 _ _ Ea $ Map.set_add (NewNames.new_name r1 variable) r1).
+    specialize (IHt1 $ Map.set_add (NewNames.new_name r2 variable) r2). destruct IHt1. 2: { constructor. } {
+      intros k []. unfold Map.set_add. repeat rewrite Map.find_overriding_add.
+      repeat rewrite (NewNames.new_name_det Er). split; (intros [[-> _] | [N F]]; [left | right];
+      [split; reflexivity | split; [exact N |]; apply Er; exact F]). }
+    specialize (IHt2 $ Map.overwrite variable (NewNames.new_name r1 variable) a1).
+    specialize (IHt2 $ Map.overwrite variable (NewNames.new_name r2 variable) a2).
+    eassert (Ea' : _); [| specialize (IHt2 Ea')]. {
+      intros k v. unfold Map.overwrite. repeat rewrite Map.find_overriding_add. repeat rewrite (NewNames.new_name_det Er).
+      split; (intros [[-> ->] | [N F]]; [left | right]; [split; reflexivity | split; [exact N |]; apply Ea; exact F]). }
+    specialize (IHt2 cant_bind1 cant_bind2 Ecant_bind) as []. { constructor. }
+    repeat rewrite (NewNames.new_name_det Er). constructor. exact Ecant_bind0.
+  - repeat rewrite unshadow_cas. rewrite (NewNames.generate_det Er $ Map.eq_refl _).
+    specialize (IHt2 _ _ Ea $ Map.set_union (Map.range $ NewNames.generate r2 $ BoundIn.pattern pattern) r1).
+    specialize (IHt2 $ Map.set_union (Map.range $ NewNames.generate r2 $ BoundIn.pattern pattern) r2).
+    destruct IHt2. 2: { constructor. } { intros k []. repeat rewrite (Map.union_set _ _ _). rewrite (Er k). reflexivity. }
+    destruct Rename.pattern eqn:R. 2: { constructor. }
+    specialize (IHt1 $ Map.bulk_overwrite (NewNames.generate r2 $ BoundIn.pattern pattern) a1).
+    specialize (IHt1 $ Map.bulk_overwrite (NewNames.generate r2 $ BoundIn.pattern pattern) a2).
+    eassert (Ea' : _); [| specialize (IHt1 Ea')]. {
+      intros k v. repeat rewrite (Map.bulk_overwrite_bulk_overwrite _ _ _). rewrite (Ea k). reflexivity. }
+    specialize (IHt1 cant_bind1 cant_bind2 Ecant_bind) as []; constructor. exact Ecant_bind0.
+Qed.
+
+Lemma det_bindings {r1 r2} (Er : Map.Eq r1 r2) {t1 t2} (Et : t1 = t2)
+  : Equiv (unshadow_reserve_bindings r1 t1) (unshadow_reserve_bindings r2 t2).
+Proof.
+  subst. rename t2 into t. eapply det_acc. 3: { reflexivity. } { intros k v. reflexivity. }
+  intros k v. repeat rewrite (Map.union_set _ _ _). rewrite (Er _). reflexivity.
 Qed.
 
 Lemma det_reserve
   {r1 r2} (Er : Map.Eq r1 r2)
   {t1 t2} (Et : t1 = t2)
   : unshadow_reserve r1 t1 = unshadow_reserve r2 t2.
+Proof. unfold unshadow_reserve. destruct (det_bindings Er Et); reflexivity. Qed.
+
+
+
+Lemma bound_or_used {acc cant_bind term bound_or_used renamed}
+  (E : unshadow_acc acc cant_bind term = Some (bound_or_used, renamed))
+  : Map.Reflect (fun x => BoundIn.Term renamed x \/ UsedIn.Term renamed x \/ Map.In cant_bind x) bound_or_used.
 Proof.
-  unfold unshadow_reserve. unfold unshadow_reserve_bindings.
-  eassert (E1 : Map.Eq (NewNames.generate r1 $ UsedIn.term t1) (NewNames.generate r2 $ UsedIn.term t2)). {
-    erewrite NewNames.generate_det. { apply Map.eq_refl. } { exact Er. } subst. apply Map.eq_refl. }
-  eassert (E2 : Map.Eq
-    (Map.set_union r1 $ Map.range $ NewNames.generate r1 $ UsedIn.term t1)
-    (Map.set_union r2 $ Map.range $ NewNames.generate r2 $ UsedIn.term t2)). {
-    split; intro F; apply Map.bulk_overwrite_bulk_overwrite;
-    (apply Map.bulk_overwrite_bulk_overwrite in F as [F | [N F]]; [left; apply Er; exact F | right]);
-    (split; [intro I; apply N; eapply Map.in_eq; [| exact I]; try exact Er; apply Map.eq_sym; exact Er |]);
-    apply Map.find_range; apply Map.find_range in F as [j F]; eexists; apply E1; exact F. }
-  destruct (det_acc E1 E2 Et); reflexivity.
-Qed.
-
-
-
-Lemma bindings {acc cant_bind term bindings renamed}
-  (E : unshadow_acc acc cant_bind term = Some (bindings, renamed))
-  (prev : forall x y (Fa : Map.Find acc x y), Map.In cant_bind y)
-  : Map.Reflect (fun x => BoundIn.Term renamed x \/ Map.In cant_bind x) bindings.
-Proof.
-  generalize dependent renamed. generalize dependent bindings.
-  generalize dependent cant_bind. generalize dependent acc. induction term; intros; simpl unshadow_acc in *.
-  - invert E. split. { intro I. right. exact I. }
-    intros [B | I]. { invert B. } exact I.
-  - destruct (Map.find_spec acc name) as [name' F | N]; invert E.
-    split. { intro I. right. exact I. }
-    intros [B | I]. { invert B. } exact I.
-  - destruct unshadow_acc as [[r1 t1] |] eqn:E1 in E. 2: { discriminate E. }
+  generalize dependent renamed. generalize dependent bound_or_used.
+  generalize dependent cant_bind. generalize dependent acc. induction term; intros.
+  - invert E. split. { intro I. right. right. exact I. }
+    intros [B | [U | I]]. { invert B. } { invert U. } exact I.
+  - cbn in E. destruct (Map.find_spec acc name) as [name' F | N]; invert E. split.
+    + intro I. apply Map.in_overriding_add in I as [-> | I]. { right. left. constructor. } right. right. exact I.
+    + intros [B | [U | I]]. { invert B. } { invert U. apply Map.in_overriding_add. left. reflexivity. }
+      apply Map.in_overriding_add. right. exact I.
+  - cbn in E. destruct unshadow_acc as [[r1 t1] |] eqn:E1 in E. 2: { discriminate E. }
     destruct unshadow_acc as [[r2 t2] |] eqn:E2 in E; invert E. eapply IHterm1 in E1; try eassumption.
-    eapply IHterm2 in E2; try eassumption. 2: { intros. apply E1. right. eapply prev. exact Fa. } split.
-    + intro I. apply E2 in I as [B | I].
+    eapply IHterm2 in E2; try eassumption. split.
+    + intro I. apply E2 in I as [B | [U | I]].
       * left. apply BoundIn.TApA. exact B.
-      * apply E1 in I as [B | I]; [left | right].
-        { apply BoundIn.TApF. exact B. } exact I.
-    + intro UI. apply E2. destruct UI as [B | I].
-      * invert B. 2: { left. exact bound_in_argument. }
-        right. apply E1. left. exact bound_in_function.
-      * right. apply E1. right. exact I.
-  - destruct unshadow_acc as [[r1 t1] |] eqn:E1 in E. 2: { discriminate E. }
+      * right. left. apply UsedIn.ApA. exact U.
+      * apply E1 in I as [B | [U | I]]; [left | right; left | right; right]. { apply BoundIn.TApF. exact B. } 2: { exact I. }
+        apply UsedIn.ApF. exact U.
+    + intro UI. apply E2. destruct UI as [B | [U | I]].
+      * invert B. 2: { left. exact bound_in_argument. } right. right. apply E1. left. exact bound_in_function.
+      * invert U. 2: { right. left. exact used_in_argument. } right. right. apply E1. right. left. exact used_in_function.
+      * right. right. apply E1. right. right. exact I.
+  - rewrite unshadow_for in E. destruct unshadow_acc as [[r1 t1] |] eqn:E1 in E. 2: { discriminate E. }
     destruct unshadow_acc as [[r2 t2] |] eqn:E2 in E; invert E.
-    apply IHterm1 in E1. 2: { exact prev. } apply IHterm2 in E2. 2: { intros. apply Map.in_overriding_add.
-      apply Map.find_overriding_add in Fa as [[-> ->] | [Na Fa]]; [left | right]. { reflexivity. }
-      apply E1. right. eapply prev. exact Fa. } split.
-    + intro I. apply E2 in I as [B | I]. { left. apply BoundIn.TFoB. exact B. }
-      apply Map.in_overriding_add in I as [-> | I]. { left. apply BoundIn.TFoV. }
-      apply E1 in I as [B | I]. { left. apply BoundIn.TFoT. exact B. } right. exact I.
-    + intro BI. apply E2. rewrite Map.in_overriding_add.
-      destruct BI as [B | I]. 2: { right. right. apply E1. right. exact I. }
-      invert B. { right. left. reflexivity. } 2: { left. exact bound_in_body. }
-      right. right. apply E1. left. exact bound_in_type.
-  - destruct unshadow_acc as [[r2 t2] |] eqn:E2 in E. 2: { discriminate E. }
-    destruct (@Rename.pattern_spec (Map.fold (fun k _ acc => Map.overriding_add k (NewNames.new_name
-      (Map.overriding_union r2 (Map.fold (fun _ v acc' => Map.overriding_add v tt acc') Map.empty acc))
-      k) acc) Map.empty (BoundIn.pattern pattern)) (NewNames.one_to_one_generate _ _) pattern). 2: { discriminate E. }
+    apply IHterm1 in E1. apply IHterm2 in E2. split.
+    + intro I. apply E2 in I as [B | [U | I]]. { left. apply BoundIn.TFoB. exact B. }
+      * destruct (String.eqb_spec x $ NewNames.new_name cant_bind variable); [| right]; left. { subst. apply BoundIn.TFoV. }
+        apply UsedIn.FoB. { exact n. } exact U.
+      * apply E1 in I as [B | [U | I]]. { left. apply BoundIn.TFoT. exact B. } { right. left. apply UsedIn.FoT. exact U. }
+        apply Map.in_overriding_add in I as [-> | I]. { left. apply BoundIn.TFoV. } right. right. exact I.
+    + intro BI. apply E2. destruct BI as [B | [U | I]].
+      * invert B; [| | left; exact bound_in_body]; right; right; apply E1. 2: { left. exact bound_in_type. }
+        right. right. apply Map.in_overriding_add. left. reflexivity.
+      * right. invert U. 2: { left. exact used_in_body. } right. apply E1. right. left. exact used_in_type.
+      * right. right. apply E1. right. right. apply Map.in_overriding_add. right. exact I.
+  - rewrite unshadow_cas in E. destruct unshadow_acc as [[r2 t2] |] eqn:E2 in E. 2: { discriminate E. }
+    destruct Rename.pattern eqn:R. 2: { discriminate E. } eapply (Rename.pattern_iff $ NewNames.one_to_one_generate _ _) in R.
     destruct unshadow_acc as [[r1 t1] |] eqn:E1 in E; invert E.
-    apply IHterm2 in E2. 2: { exact prev. } apply IHterm1 in E1. 2: {
-      intros k v Fa. apply Map.in_overriding_union. rewrite Map.in_range.
-      apply Map.bulk_overwrite_bulk_overwrite in Fa as [Fa | [Na Fa]]. { left. eexists. exact Fa. }
-      right. apply E2. right. eapply prev. exact Fa. } split.
-    + intro I. apply E1 in I as [B | I]. { left. apply BoundIn.TCaB. exact B. }
-      apply Map.in_overriding_union in I as [I | I].
-      * apply Map.in_range in I as [y0 F]. eassert (I : Map.In _ _). { eexists. exact F. }
-        apply NewNames.in_generate in I. apply BoundIn.pattern_iff in I as B.
-        eapply Rename.bound_in_pattern in Y. left. apply BoundIn.TCaP. apply Y. eexists. split. { exact B. } exact F.
-      * apply E2 in I as [B | I]. { left. apply BoundIn.TCaO. exact B. } right. exact I.
-    + intro BI. apply E1. rewrite Map.in_overriding_union. rewrite Map.in_range.
-      destruct BI as [B | I]. 2: { right. right. apply E2. right. exact I. }
-      invert B. 2: { left. exact bound_in_body. } 2: { right. right. apply E2. left. exact bound_in_another_case. }
-      eapply Rename.bound_in_pattern in Y. apply Y in bound_in_pattern as [z [B F]]. right. left. eexists. exact F.
+    apply IHterm2 in E2. apply IHterm1 in E1. split.
+    + intro I. apply E1 in I as [B | [U | I]]. { left. apply BoundIn.TCaB. exact B. } {
+        destruct (BoundIn.pattern_spec p x); [| right]; left. { apply BoundIn.TCaP. exact Y. }
+        apply UsedIn.CaB. 2: { exact U. } exact N. }
+      apply E2 in I as [B | [U | I]]. { left. apply BoundIn.TCaO. exact B. } { right. left. apply UsedIn.CaO. exact U. }
+      apply Map.in_overriding_union in I as [I | I]. 2: { right. right. exact I. }
+      apply Map.in_space_range in I as [w F]. left. apply BoundIn.TCaP. eapply (Rename.bound_in_pattern R).
+      exists w. split. 2: { exact F. } apply BoundIn.pattern_iff. eapply NewNames.in_generate. exists x. exact F.
+    + intro BUI. apply E1. destruct BUI as [B | [U | I]].
+      * invert B; [| left; exact bound_in_body |]; right; right; apply E2. 2: { left. exact bound_in_another_case. }
+        right. right. apply Map.in_overriding_union. left. apply (Rename.bound_in_pattern R) in bound_in_pattern as [w [B F]].
+        apply Map.in_space_range. exists w. exact F.
+      * right. invert U. { left. exact used_in_body. } right. apply E2. right. left. exact used_in_another_case.
+      * right. right. apply E2. right. right. apply Map.in_overriding_union. right. exact I.
 Qed.
 
 
@@ -257,12 +266,12 @@ Lemma wf_patterns_spec_acc acc cant_bind t
       forall x (U : UsedIn.Term t x), Map.In acc x
     ) $ unshadow_acc acc cant_bind t.
 Proof.
-  generalize dependent cant_bind. generalize dependent acc. induction t; intros; cbn in *.
+  generalize dependent cant_bind. generalize dependent acc. induction t; intros.
   - constructor. split. { constructor. } split. { constructor. } intros. invert U.
-  - destruct (Map.find_spec acc name); constructor.
+  - cbn. destruct (Map.find_spec acc name); constructor.
     + split; intros. { constructor. } split. { constructor. } intros. invert U. eexists. exact Y.
     + intros [cant_bind' t'] [WF [WF' C]]. edestruct C. { constructor. } apply N in H as [].
-  - destruct (IHt1 acc cant_bind) as [[r1 t1'] [WF1 [WF1' IH1]] |]. 2: {
+  - cbn. destruct (IHt1 acc cant_bind) as [[r1 t1'] [WF1 [WF1' IH1]] |]. 2: {
       constructor. intros [cant_bind' t'] [WF [WF' C]]. invert WF. eapply (N (cant_bind', t')).
       split. { exact APf. } split. { exact WF'. } intros. apply C. apply UsedIn.ApF. exact U. }
     destruct (IHt2 acc r1) as [[r2 t2'] [WF2 [WF2' IH2]] |]; constructor.
@@ -270,11 +279,11 @@ Proof.
       intros. invert U; [apply IH1 | apply IH2]; assumption.
     + intros [cant_bind' t'] [WF [WF' C]]. invert WF. apply (N (cant_bind', t')).
       split. { exact APa. } split. { exact WF'. } intros. apply C. apply UsedIn.ApA. exact U.
-  - destruct (IHt1 acc cant_bind) as [[r1 t1'] [WF1 [WF1' IH1]] |]. 2: {
+  - rewrite unshadow_for.
+    destruct (IHt1 acc $ Map.set_add (NewNames.new_name cant_bind variable) cant_bind) as [[r1 t1'] [WF1 [WF1' IH1]] |]. 2: {
       constructor. intros [cant_bind' t'] [WF [WF' C]]. invert WF. apply (N (cant_bind', t')).
       split. { exact APt. } split. { exact WF'. } intros. apply C. apply UsedIn.FoT. exact U. }
-    destruct (IHt2 (Map.overriding_add variable (NewNames.new_name r1 variable) acc)
-      (Map.overriding_add (NewNames.new_name r1 variable) tt r1)) as [[r2 t2'] [WF2 [WF2' IH2]] |]; constructor.
+    destruct (IHt2 (Map.overwrite variable (NewNames.new_name cant_bind variable) acc) r1) as [[r2 t2'] [WF2 [WF2' IH2]] |]; constructor.
     + split. { constructor; assumption. } split. { constructor. { exact WF1'. } exact WF2'. }
       intros. invert U. { apply IH1. exact used_in_type. }
       apply IH2 in used_in_body. apply Map.in_overriding_add in used_in_body as [-> | I]. 2: { exact I. }
@@ -282,38 +291,33 @@ Proof.
     + intros [cant_bind' t'] [WF [WF' C]]. invert WF. apply (N (cant_bind', t')).
       split. { exact APb. } split. { exact WF'. } intros. apply Map.in_overriding_add.
       destruct (String.eqb_spec x variable); [left | right]. { assumption. } apply C. apply UsedIn.FoB; assumption.
-  - destruct (IHt2 acc cant_bind) as [[r2 t2'] [WF2 [WF2' IH2]] |]. 2: {
+  - rewrite unshadow_cas. destruct (IHt2 acc $ Map.set_union (Map.range $ NewNames.generate cant_bind $ BoundIn.pattern pattern)
+      cant_bind) as [[r2 t2'] [WF2 [WF2' IH2]] |]. 2: {
       constructor. intros [cant_bind' t'] [WF [WF' C]]. invert WF. apply (N (cant_bind', t')).
       split. { exact APo. } split. { exact WF'. } intros. apply C. apply UsedIn.CaO. exact U. }
-    destruct (@Rename.pattern_spec (Map.fold (fun k _ acc' => Map.overriding_add k (NewNames.new_name
-      (Map.overriding_union r2 (Map.fold (fun _ v acc'' => Map.overriding_add v tt acc'') Map.empty acc'))
-      k) acc') Map.empty (BoundIn.pattern pattern)) (NewNames.one_to_one_generate _ _) pattern). 2: {
+    destruct Rename.pattern eqn:R. 2: {
       constructor. intros [cant_bind' t'] [WF [WF' C]]. invert WF. eassert (RC : Rename.CompatiblePattern _ _). 2: {
-        apply Rename.pattern_iff_compatible in RC as [O2O [renamed R]].
-        eapply Rename.pattern_eq in R; try reflexivity. { apply N in R as []. } apply Map.eq_refl. }
+        apply Rename.pattern_iff_compatible in RC as [O2O [renamed R']].
+        apply (Rename.pattern_iff O2O) in R'. rewrite R' in R. discriminate R. }
       invert WFp; constructor. { apply NewNames.one_to_one_generate. } {
         apply NewNames.in_generate. apply Map.in_singleton. reflexivity. }
       invert move_or_reference_well_formed; constructor; (split; [apply NewNames.one_to_one_generate |]);
       (split; [exact strict_well_formed |]); intros k [] F; apply Map.find_domain;
       apply NewNames.in_generate; cbn; exists tt; exact F. }
-    eassert (RC : Rename.CompatiblePattern _ _). { apply Rename.pattern_iff_compatible. do 2 eexists. exact Y. }
-    destruct (IHt1
-      (Map.overriding_union (Map.fold (fun k _ acc' => Map.overriding_add k (NewNames.new_name (Map.overriding_union r2
-        (Map.fold (fun _ v acc'' => Map.overriding_add v tt acc'') Map.empty acc')) k) acc') Map.empty (BoundIn.pattern pattern)) acc)
-      (Map.overriding_union (Map.fold (fun _ v acc' => Map.overriding_add v tt acc') Map.empty (Map.fold
-        (fun k _ acc' => Map.overriding_add k (NewNames.new_name (Map.overriding_union r2 (Map.fold
-          (fun _ v acc'' => Map.overriding_add v tt acc'') Map.empty acc')) k) acc')
-        Map.empty (BoundIn.pattern pattern))) r2)) as [[r1 t1'] [WF1 [WF1' IH1]] |]; constructor.
+    apply (Rename.pattern_iff $ NewNames.one_to_one_generate _ _) in R.
+    eassert (RC : Rename.CompatiblePattern _ _). { apply Rename.pattern_iff_compatible. do 2 eexists. exact R. }
+    destruct (IHt1 (Map.bulk_overwrite (NewNames.generate cant_bind $ BoundIn.pattern pattern) acc)
+      r2) as [[r1 t1'] [WF1 [WF1' IH1]] |]; constructor.
     + constructor. { constructor; try assumption. invert RC; constructor. invert C; constructor; apply CS. }
-      split. { constructor. 2: { exact WF1'. } 2: { exact WF2'. } invert Y; constructor.
+      split. { constructor. 2: { exact WF1'. } 2: { exact WF2'. } invert R; constructor.
         invert rename_move_or_reference; constructor; eapply Rename.wf_strict; exact rename_strict. }
       intros z U. invert U. 2: { apply IH2. exact used_in_another_case. } apply IH1 in used_in_body.
       apply Map.in_overriding_union in used_in_body as [I | I]. 2: { exact I. }
       apply NewNames.in_generate in I. apply BoundIn.pattern_iff in I. apply not_shadowed in I as [].
     + intros [cant_bind' t'] [WF [WF' C]]. invert WF. apply (N (cant_bind', t')).
       split. { exact APb. } split. { exact WF'. } intros.
-      apply Map.in_overriding_union. destruct (BoundIn.pattern_spec pattern x0); [left | right].
-      * apply NewNames.in_generate. apply BoundIn.pattern_iff. exact Y0.
+      apply Map.in_overriding_union. destruct (BoundIn.pattern_spec pattern x); [left | right].
+      * apply NewNames.in_generate. apply BoundIn.pattern_iff. exact Y.
       * apply C. apply UsedIn.CaB; assumption.
 Qed.
 
@@ -323,11 +327,11 @@ Lemma wf_patterns_spec_bindings cant_bind t
     ) $ unshadow_reserve_bindings cant_bind t.
 Proof.
   unfold unshadow_reserve. unfold unshadow_reserve_bindings.
-  destruct (wf_patterns_spec_acc (NewNames.generate cant_bind $ UsedIn.term t)
-    (Map.set_union cant_bind $ Map.range $ NewNames.generate cant_bind $ UsedIn.term t) t) as [[domain' renamed] |]; cbn; constructor.
+  destruct (wf_patterns_spec_acc (Map.to_self $ UsedIn.term t)
+    (Map.set_union cant_bind $ UsedIn.term t) t) as [[domain' renamed] |]; cbn; constructor.
   - destruct Y as [WF [WF' AU]]. split. { exact WF. } exact WF'.
   - intros [cant_bind' t'] [WF WF']. apply (N (cant_bind', t')). split. { exact WF. }
-    split. { exact WF'. } intros. apply NewNames.in_generate. apply UsedIn.term_iff. exact U.
+    split. { exact WF'. } intros. apply Map.in_to_self. apply UsedIn.term_iff. exact U.
 Qed.
 
 Lemma wf_patterns_spec domain t
@@ -343,128 +347,84 @@ Qed.
 
 Lemma disjoint_used {acc cant_bind term cant_bind' renamed}
   (E : unshadow_acc acc cant_bind term = Some (cant_bind', renamed))
-  (prev : forall x y (Fa : Map.Find acc x y), Map.In cant_bind y)
   {y} (I : Map.In cant_bind y) (U : UsedIn.Term renamed y)
   : exists x, Map.Find acc x y.
 Proof.
   generalize dependent y. generalize dependent renamed. generalize dependent cant_bind'.
-  generalize dependent cant_bind. generalize dependent acc. induction term; intros; cbn in *.
+  generalize dependent cant_bind. generalize dependent acc. induction term; intros.
   - invert E. invert U.
-  - destruct (Map.find_spec acc name); invert E. invert U. eexists. exact Y.
-  - destruct unshadow_acc as [[r1 t1] |] eqn:E1 in E. 2: { discriminate E. }
+  - cbn in E. destruct (Map.find_spec acc name); invert E. invert U. eexists. exact Y.
+  - cbn in E. destruct unshadow_acc as [[r1 t1] |] eqn:E1 in E. 2: { discriminate E. }
     destruct unshadow_acc as [[r2 t2] |] eqn:E2 in E; invert E.
-    invert U. { eapply IHterm1. { exact prev. } { exact E1. } { exact I. } exact used_in_function. }
-    eapply IHterm2. 2: { exact E2. } 3: { exact used_in_argument. }
-    + intros. eapply bindings. { exact E1. } { exact prev. } right. eapply prev. exact Fa.
-    + eapply bindings. { exact E1. } { exact prev. } right. exact I.
-  - destruct unshadow_acc as [[r1 t1] |] eqn:E1 in E. 2: { discriminate E. }
+    invert U. { eapply IHterm1. { exact E1. } { exact I. } exact used_in_function. }
+    eapply IHterm2. { exact E2. } 2: { exact used_in_argument. }
+    eapply bound_or_used. { exact E1. } right. right. exact I.
+  - rewrite unshadow_for in E. destruct unshadow_acc as [[r1 t1] |] eqn:E1 in E. 2: { discriminate E. }
     destruct unshadow_acc as [[r2 t2] |] eqn:E2 in E; invert E.
-    invert U. { eapply IHterm1. { exact prev. } { exact E1. } { exact I. } exact used_in_type. }
-    eapply IHterm2 in E2 as [x IH2]. 4: { exact used_in_body. }
+    invert U. { eapply IHterm1. { exact E1. } 2: { exact used_in_type. } apply Map.in_overriding_add. right. exact I. }
+    eapply IHterm2 in E2 as [x IH2]. 3: { exact used_in_body. }
     + apply Map.find_overriding_add in IH2 as [[-> ->] | [N F]]. { contradiction not_shadowed. reflexivity. } eexists. exact F.
-    + intros. apply Map.in_overriding_add. apply Map.find_overriding_add in Fa as [[-> ->] | [Na Fa]]; [left | right]. { reflexivity. }
-      eapply bindings. { exact E1. } { exact prev. } right. eapply prev. exact Fa.
-    + apply Map.in_overriding_add. right. eapply bindings. { exact E1. } { exact prev. } right. exact I.
-  - destruct unshadow_acc as [[r2 t2] |] eqn:E2 in E. 2: { discriminate E. }
-    destruct (@Rename.pattern_spec (Map.fold (fun k _ acc' => Map.overriding_add k (NewNames.new_name
-      (Map.overriding_union r2 (Map.fold (fun _ v acc'' => Map.overriding_add v tt acc'') Map.empty acc'))
-      k) acc') Map.empty (BoundIn.pattern pattern)) (NewNames.one_to_one_generate _ _) pattern). 2: { discriminate E. }
+    + eapply bound_or_used. { exact E1. } right. right. apply Map.in_overriding_add. right. exact I.
+  - rewrite unshadow_cas in E. destruct unshadow_acc as [[r2 t2] |] eqn:E2 in E. 2: { discriminate E. }
+    destruct Rename.pattern eqn:R. 2: { discriminate E. } apply (Rename.pattern_iff $ NewNames.one_to_one_generate _ _) in R.
     destruct unshadow_acc as [[r1 t1] |] eqn:E1 in E; invert E.
-    invert U. 2: { eapply IHterm2. { exact prev. } { exact E2. } { exact I. } exact used_in_another_case. }
-    eapply IHterm1 in E1 as [z IH1]. 4: { exact used_in_body. }
+    invert U. 2: { eapply IHterm2. { exact E2. } 2: { exact used_in_another_case. } apply Map.in_overriding_union. right. exact I. }
+    eapply IHterm1 in E1 as [z IH1]. 3: { exact used_in_body. }
     + apply Map.bulk_overwrite_bulk_overwrite in IH1 as [F | [N F]]. 2: { eexists. exact F. }
       eassert (I' : Map.In _ _). { eexists. exact F. } apply NewNames.in_generate in I'. apply BoundIn.pattern_iff in I' as B.
-      contradiction not_shadowed. eapply Rename.bound_in_pattern. { exact Y. } eexists. split. { exact B. } exact F.
-    + intros k v F. apply Map.in_overriding_union.
-      apply Map.bulk_overwrite_bulk_overwrite in F as [F | [N F]]. { left. apply Map.in_range. eexists. exact F. }
-      right. eapply bindings. { exact E2. } { exact prev. } right. eapply prev. exact F.
-    + apply Map.in_overriding_union. right. eapply bindings. { exact E2. } { exact prev. } right. exact I.
+      contradiction not_shadowed. eapply Rename.bound_in_pattern. { exact R. } eexists. split. { exact B. } exact F.
+    + eapply bound_or_used. { exact E2. } right. right. apply Map.in_overriding_union. right. exact I.
 Qed.
 
 Lemma disjoint_bound {acc cant_bind term cant_bind' renamed}
   (E : unshadow_acc acc cant_bind term = Some (cant_bind', renamed))
-  (prev : forall x y (Fa : Map.Find acc x y), Map.In cant_bind y)
   {x} (I : Map.In cant_bind x) (B : BoundIn.Term renamed x)
   : False.
 Proof.
   generalize dependent x. generalize dependent renamed. generalize dependent cant_bind'.
-  generalize dependent cant_bind. generalize dependent acc. induction term; intros; cbn in *.
+  generalize dependent cant_bind. generalize dependent acc. induction term; intros.
   - invert E. invert B.
-  - destruct (Map.find_spec acc name); invert E. invert B.
-  - destruct unshadow_acc as [[r1 t1] |] eqn:E1 in E. 2: { discriminate E. }
+  - cbn in E. destruct (Map.find_spec acc name); invert E. invert B.
+  - cbn in E. destruct unshadow_acc as [[r1 t1] |] eqn:E1 in E. 2: { discriminate E. }
     destruct unshadow_acc as [[r2 t2] |] eqn:E2 in E; invert E.
-    invert B. { eapply IHterm1. { exact prev. } { exact E1. } { exact I. } exact bound_in_function. }
-    eapply IHterm2. 2: { exact E2. } 3: { exact bound_in_argument. }
-    + intros. eapply bindings. { exact E1. } { exact prev. } right. eapply prev. exact Fa.
-    + eapply bindings. { exact E1. } { exact prev. } right. exact I.
-  - destruct unshadow_acc as [[r1 t1] |] eqn:E1 in E. 2: { discriminate E. }
+    invert B. { eapply IHterm1. { exact E1. } { exact I. } exact bound_in_function. }
+    eapply IHterm2. { exact E2. } 2: { exact bound_in_argument. }
+    eapply bound_or_used. { exact E1. } right. right. exact I.
+  - rewrite unshadow_for in E. destruct unshadow_acc as [[r1 t1] |] eqn:E1 in E. 2: { discriminate E. }
     destruct unshadow_acc as [[r2 t2] |] eqn:E2 in E; invert E. invert B.
-    + eapply NewNames.not_in_new_name. eapply bindings. { exact E1. } { exact prev. } right. exact I.
-    + eapply IHterm1. { exact prev. } { exact E1. } { exact I. } exact bound_in_type.
-    + eapply IHterm2 in E2 as []. 3: { exact bound_in_body. }
-      * intros. apply Map.in_overriding_add. apply Map.find_overriding_add in Fa as [[-> ->] | [Na Fa]]. { left. reflexivity. }
-        right. eapply bindings. { exact E1. } { exact prev. } right. eapply prev. exact Fa.
-      * apply Map.in_overriding_add. right. eapply bindings. { exact E1. } { exact prev. } right. exact I.
-  - destruct unshadow_acc as [[r2 t2] |] eqn:E2 in E. 2: { discriminate E. }
-    destruct (@Rename.pattern_spec (Map.fold (fun k _ acc' => Map.overriding_add k (NewNames.new_name
-      (Map.overriding_union r2 (Map.fold (fun _ v acc'' => Map.overriding_add v tt acc'') Map.empty acc'))
-      k) acc') Map.empty (BoundIn.pattern pattern)) (NewNames.one_to_one_generate _ _) pattern). 2: { discriminate E. }
+    + eapply NewNames.not_in_new_name in I as [].
+    + eapply IHterm1. { exact E1. } 2: { exact bound_in_type. } apply Map.in_overriding_add. right. exact I.
+    + eapply IHterm2 in E2 as []. 2: { exact bound_in_body. }
+      eapply bound_or_used. { exact E1. } right. right. apply Map.in_overriding_add. right. exact I.
+  - rewrite unshadow_cas in E. destruct unshadow_acc as [[r2 t2] |] eqn:E2 in E. 2: { discriminate E. }
+    destruct Rename.pattern eqn:R. 2: { discriminate E. } apply (Rename.pattern_iff $ NewNames.one_to_one_generate _ _) in R.
     destruct unshadow_acc as [[r1 t1] |] eqn:E1 in E; invert E. invert B.
-    + apply (Rename.bound_in_pattern Y) in bound_in_pattern as [z [B F]]. eapply NewNames.not_in_generate. 2: { eexists. exact F. }
-      eapply bindings. { exact E2. } { exact prev. } right. exact I.
-    + eapply IHterm1 in E1 as []. 3: { exact bound_in_body. }
-      * intros k v F. apply Map.in_overriding_union. rewrite Map.in_range.
-        apply Map.bulk_overwrite_bulk_overwrite in F as [F | [N F]]. { left. eexists. exact F. }
-        right. eapply bindings. { exact E2. } { exact prev. } right. eapply prev. exact F.
-      * apply Map.in_overriding_union. rewrite Map.in_range. right. eapply bindings. { exact E2. } { exact prev. } right. exact I.
-    + eapply IHterm2. { exact prev. } { exact E2. } { exact I. } exact bound_in_another_case.
+    + apply (Rename.bound_in_pattern R) in bound_in_pattern as [z [B F]].
+      eapply NewNames.not_in_generate. { exact I. } exists z. exact F.
+    + eapply IHterm1 in E1 as []. 2: { exact bound_in_body. }
+      eapply bound_or_used. { exact E2. } right. right. apply Map.in_overriding_union. right. exact I.
+    + eapply IHterm2. { exact E2. } 2: { exact bound_in_another_case. } apply Map.in_overriding_union. right. exact I.
 Qed.
 
 Lemma used_cant_bind {acc cant_bind term cant_bind' renamed}
   (E : unshadow_acc acc cant_bind term = Some (cant_bind', renamed))
-  (prev : forall x y (Fa : Map.Find acc x y), Map.In cant_bind y)
   {x} (U : UsedIn.Term renamed x)
   : Map.In cant_bind' x.
 Proof.
   generalize dependent x. generalize dependent renamed. generalize dependent cant_bind'.
   generalize dependent cant_bind. generalize dependent acc. induction term; intros; cbn in *.
   - invert E. invert U.
-  - destruct (Map.find_spec acc name); invert E. invert U. eapply prev. exact Y.
+  - destruct (Map.find_spec acc name); invert E. invert U. apply Map.in_overriding_add. left. reflexivity.
   - destruct unshadow_acc as [[r1 t1] |] eqn:E1 in E. 2: { discriminate E. }
-    destruct unshadow_acc as [[r2 t2] |] eqn:E2 in E; invert E.
-    eassert (prev' : forall k v (F : Map.Find acc k v), Map.In r1 v). {
-      intros k v F. eapply bindings; try eassumption. right. eapply prev. exact F. }
-    invert U. 2: { eapply IHterm2. 2: { eassumption. } 2: { eassumption. } exact prev'. }
-    eapply IHterm1 in E1; try eassumption. eapply bindings; try eassumption. right. exact E1.
+    destruct unshadow_acc as [[r2 t2] |] eqn:E2 in E; invert E. invert U. 2: { eapply IHterm2; eassumption. }
+    eapply IHterm1 in E1; try eassumption. eapply bound_or_used; try eassumption. right. right. exact E1.
   - destruct unshadow_acc as [[r1 t1] |] eqn:E1 in E. 2: { discriminate E. }
-    eassert (prev' : forall k v (F : Map.Find (Map.overriding_add variable (NewNames.new_name r1 variable) acc) k v),
-      Map.In (Map.overriding_add (NewNames.new_name r1 variable) tt r1) v). {
-      intros k v F. apply Map.in_overriding_add. apply Map.find_overriding_add in F as [[-> ->] | [N F]]. { left. reflexivity. }
-      right. eapply bindings. { exact E1. } { exact prev. } right. eapply prev. exact F. }
-    destruct unshadow_acc as [[r2 t2] |] eqn:E2 in E; invert E. invert U. 2: {
-      eapply IHterm2. 2: { exact E2. } 2: { exact used_in_body. } exact prev'. }
-    eapply IHterm1 in E1; try eassumption. eapply bindings; try eassumption.
-    right. apply Map.in_overriding_add. right. exact E1.
+    destruct unshadow_acc as [[r2 t2] |] eqn:E2 in E; invert E. invert U. 2: { eapply IHterm2. { exact E2. } exact used_in_body. }
+    eapply IHterm1 in E1; try eassumption. eapply bound_or_used; try eassumption. right. right. exact E1.
   - destruct unshadow_acc as [[r2 t2] |] eqn:E2 in E. 2: { discriminate E. }
-    destruct (@Rename.pattern_spec (Map.fold (fun k _ acc' => Map.overriding_add k (NewNames.new_name
-      (Map.overriding_union r2 (Map.fold (fun _ v acc'' => Map.overriding_add v tt acc'') Map.empty acc'))
-      k) acc') Map.empty (BoundIn.pattern pattern)) (NewNames.one_to_one_generate _ _) pattern). 2: { discriminate E. }
-    eassert (prev' : forall z y,
-      Map.Find (Map.overriding_union (Map.fold (fun k _ acc' => Map.overriding_add k (NewNames.new_name
-        (Map.overriding_union r2 (Map.fold (fun _ v acc1 => Map.overriding_add v tt acc1) Map.empty acc'))
-        k) acc') Map.empty (BoundIn.pattern pattern)) acc) z y ->
-      exists v : unit,
-      Map.Find (Map.overriding_union (Map.fold (fun (_ v0 : String.string) (acc' : Map.to unit) =>
-        Map.overriding_add v0 tt acc') Map.empty (Map.fold (fun k _ acc' => Map.overriding_add k (NewNames.new_name
-        (Map.overriding_union r2 (Map.fold (fun _ v0 acc1 => Map.overriding_add v0 tt acc1) Map.empty acc'))
-        k) acc') Map.empty (BoundIn.pattern pattern))) r2) y v). {
-      intros k v F. apply Map.in_overriding_union. rewrite Map.in_range.
-      apply Map.bulk_overwrite_bulk_overwrite in F as [F | [N F]]. { left. eexists. exact F. }
-      right. eapply bindings. { exact E2. } { exact prev. } right. eapply prev. exact F. }
-    destruct unshadow_acc as [[r1 t1] |] eqn:E1 in E; invert E. invert U. {
-      eapply IHterm1. 2: { exact E1. } 2: { exact used_in_body. } exact prev'. }
-    eapply IHterm2 in E2; try eassumption. eapply bindings; try eassumption.
-    right. apply Map.in_overriding_union. right. exact E2.
+    destruct Rename.pattern eqn:R. 2: { discriminate E. } apply (Rename.pattern_iff $ NewNames.one_to_one_generate _ _) in R.
+    destruct unshadow_acc as [[r1 t1] |] eqn:E1 in E; invert E. invert U. { eapply IHterm1. { exact E1. } exact used_in_body. }
+    eapply IHterm2 in E2; try eassumption. eapply bound_or_used; try eassumption. right. right. exact E2.
 Qed.
 
 
@@ -553,9 +513,9 @@ Fixpoint well_formed_in_acc cant_bind context t :=
       ) (well_formed_in_acc cant_bind context function)
   | Term.For variable type body =>
       bind (fun bound_in_type used_in_type =>
-        let cant_bind_in_body_without_bindings := Map.set_union cant_bind $ Map.set_union bound_in_type used_in_type in
-        if Map.in_ cant_bind_in_body_without_bindings variable then None else
-        let cant_bind_in_body := Map.set_add variable cant_bind_in_body_without_bindings in
+        let bound_or_used_in_body_without_bindings := Map.set_union cant_bind $ Map.set_union bound_in_type used_in_type in
+        if Map.in_ bound_or_used_in_body_without_bindings variable then None else
+        let bound_or_used_in_body := Map.set_add variable bound_or_used_in_body_without_bindings in
         let context_in_body := Map.set_add variable context in
         bind (fun bound_in_body used_in_body =>
           if Map.disjoint bound_in_type bound_in_body then
@@ -566,15 +526,15 @@ Fixpoint well_formed_in_acc cant_bind context t :=
               else None
             else None
           else None
-        ) (well_formed_in_acc cant_bind_in_body context_in_body body)
+        ) (well_formed_in_acc bound_or_used_in_body context_in_body body)
       ) (well_formed_in_acc cant_bind context type)
   | Term.Cas pattern body_if_match other_cases =>
       bind (fun bound_in_other_cases used_in_other_cases =>
-        let cant_bind_in_body_without_bindings := Map.set_union cant_bind $ Map.set_union bound_in_other_cases used_in_other_cases in
+        let bound_or_used_in_body_without_bindings := Map.set_union cant_bind $ Map.set_union bound_in_other_cases used_in_other_cases in
         if WellFormed.pattern pattern then
           let bound_in_pattern := BoundIn.pattern pattern in
-          if Map.disjoint cant_bind_in_body_without_bindings bound_in_pattern then
-            let cant_bind_in_body_if_match := Map.set_union bound_in_pattern cant_bind_in_body_without_bindings in
+          if Map.disjoint bound_or_used_in_body_without_bindings bound_in_pattern then
+            let bound_or_used_in_body_if_match := Map.set_union bound_in_pattern bound_or_used_in_body_without_bindings in
             let context_in_body_if_match := Map.set_union bound_in_pattern context in
             bind (fun bound_in_body_if_match used_in_body_if_match =>
               if Map.disjoint bound_in_other_cases bound_in_body_if_match then
@@ -585,7 +545,7 @@ Fixpoint well_formed_in_acc cant_bind context t :=
                   else None
                 else None
               else None
-            ) (well_formed_in_acc cant_bind_in_body_if_match context_in_body_if_match body_if_match)
+            ) (well_formed_in_acc bound_or_used_in_body_if_match context_in_body_if_match body_if_match)
           else None
         else None
       ) (well_formed_in_acc cant_bind context other_cases)
@@ -654,7 +614,7 @@ Qed.
 
 Lemma well_formed_in_acc_spec
   {t context} (no_free_vars : forall x (U : UsedIn.Term t x), Map.In context x)
-  {cant_bind} (cant_bind_context : forall x (I : Map.In context x), Map.In cant_bind x)
+  {cant_bind} (bound_or_used_context : forall x (I : Map.In context x), Map.In cant_bind x)
   : Reflect.Option (fun _ => WellFormedNegInAcc cant_bind context t) $
     well_formed_in_acc cant_bind context t.
 Proof.
@@ -663,13 +623,13 @@ Proof.
   - destruct (Map.in_spec context name); constructor.
     + split. { split. { constructor. } repeat split; intro C; invert C. } split; intros. { invert B. } invert U. exact Y.
     + eintros _ [_ [_ C]]. apply N in C as []. constructor.
-  - eassert (no_free_vars_1 : _); [| specialize (IHt1 context no_free_vars_1 cant_bind cant_bind_context)]. {
+  - eassert (no_free_vars_1 : _); [| specialize (IHt1 context no_free_vars_1 cant_bind bound_or_used_context)]. {
       intros. apply no_free_vars. apply UsedIn.ApF. exact U. }
     destruct well_formed_in_acc as [[b1 u1] |] eqn:E1 in IHt1; rewrite E1; invert IHt1. 2: {
       constructor. intros pair [[AP [NH [NS [NP NL]]]] C]. apply (N pair). split. 2: { intro x. specialize (C x) as [C1 C2].
         split; intros; [apply C1 | apply C2]. { apply BoundIn.TApF. exact B. } { exact I. } apply UsedIn.ApF. exact U. }
       split. { invert AP. exact APf. } repeat split; intro; [apply NH | apply NS | apply NP | apply NL]; apply ARAF; assumption. }
-    eassert (no_free_vars_2 : _); [| specialize (IHt2 context no_free_vars_2 cant_bind cant_bind_context)]. {
+    eassert (no_free_vars_2 : _); [| specialize (IHt2 context no_free_vars_2 cant_bind bound_or_used_context)]. {
       intros. apply no_free_vars. apply UsedIn.ApA. exact U. }
     destruct well_formed_in_acc as [[b2 u2] |] eqn:E2 in IHt2; rewrite E2; invert IHt2. 2: {
       constructor. intros pair [[AP [NH [NS [NP NL]]]] C]. apply (N pair). split. 2: { intro x. specialize (C x) as [C1 C2].
@@ -694,7 +654,7 @@ Proof.
     + destruct Y as [_ H1]. destruct Y0 as [_ H2]. split; intros.
       * invert B; [eapply H1 | eapply H2]; eassumption.
       * invert U; [apply H1 | apply H2]; assumption.
-  - eassert (no_free_vars_1 : _); [| specialize (IHt1 context no_free_vars_1 cant_bind cant_bind_context)]. {
+  - eassert (no_free_vars_1 : _); [| specialize (IHt1 context no_free_vars_1 cant_bind bound_or_used_context)]. {
       intros. apply no_free_vars. apply UsedIn.FoT. exact U. }
     destruct well_formed_in_acc as [[b1 u1] |] eqn:E1 in IHt1; rewrite E1; invert IHt1. 2: {
       constructor. intros pair [[AP [NH [NS [NP NL]]]] C]. apply (N pair). split. 2: { intro x. specialize (C x) as [C1 C2].
@@ -710,9 +670,9 @@ Proof.
       no_free_vars_2 (Map.overriding_add variable tt $ Map.overriding_union cant_bind $ Map.overriding_union b1 u1))]. {
       intros. apply Map.in_overriding_add. destruct (String.eqb_spec x variable); [left | right]. { exact e. }
       apply no_free_vars. apply UsedIn.FoB. { exact n. } exact U. }
-    eassert (cant_bind_context' : _); [| specialize (IHt2 cant_bind_context')]. {
+    eassert (bound_or_used_context' : _); [| specialize (IHt2 bound_or_used_context')]. {
       intro x. repeat rewrite Map.in_overriding_add. destruct (String.eqb_spec x variable); [left | right]. { exact e. }
-      destruct I as [E | I]. { apply n in E as []. } repeat rewrite Map.in_overriding_union. left. apply cant_bind_context. exact I. }
+      destruct I as [E | I]. { apply n in E as []. } repeat rewrite Map.in_overriding_union. left. apply bound_or_used_context. exact I. }
     destruct well_formed_in_acc as [[b2 u2] |] eqn:E2 in IHt2; rewrite E2 in *; invert IHt2. 2: {
       constructor. intros pair [[AP [NH [NS [NP NL]]]] C]. apply (N0 pair). split. {
         split. { invert AP. exact APb. } repeat split; intro NA; [apply NH | apply NS | apply NP | apply NL]; apply ARFB; exact NA. }
@@ -752,7 +712,7 @@ Proof.
         apply (C2 x). { exact bound_in_body. } apply Map.in_overriding_add. right. apply Map.in_overriding_union. left. exact I.
       * invert U. { apply no_free_vars_1. exact used_in_type. } apply no_free_vars_2 in used_in_body.
         apply Map.in_overriding_add in used_in_body as [E | U]. { apply not_shadowed in E as []. } exact U.
-  - eassert (no_free_vars_2 : _); [| specialize (IHt2 context no_free_vars_2 cant_bind cant_bind_context)]. {
+  - eassert (no_free_vars_2 : _); [| specialize (IHt2 context no_free_vars_2 cant_bind bound_or_used_context)]. {
       intros. apply no_free_vars. apply UsedIn.CaO. exact U. }
     destruct well_formed_in_acc as [[b2 u2] |] eqn:E2 in IHt2; rewrite E2; invert IHt2. 2: {
       constructor. intros pair [[AP [NH [NS [NP NL]]]] C]. apply (N pair). split. 2: { intro x. specialize (C x) as [C1 C2].
@@ -770,9 +730,9 @@ Proof.
       no_free_vars_1 (Map.overriding_union (BoundIn.pattern pattern) $ Map.overriding_union cant_bind $ Map.overriding_union b2 u2))]. {
       intros. apply Map.in_overriding_union. destruct (BoundIn.pattern_spec pattern x). { left. apply BoundIn.pattern_iff. exact Y2. }
       right. apply no_free_vars. apply UsedIn.CaB. { exact N. } exact U. }
-    eassert (cant_bind_context' : _); [| specialize (IHt1 cant_bind_context')]. {
+    eassert (bound_or_used_context' : _); [| specialize (IHt1 bound_or_used_context')]. {
       intro x. repeat rewrite Map.in_overriding_union. intros [I | I]; [left | right]. { exact I. }
-      left. apply cant_bind_context. exact I. }
+      left. apply bound_or_used_context. exact I. }
     destruct well_formed_in_acc as [[b1 u1] |] eqn:E1 in IHt1; rewrite E1 in *; invert IHt1. 2: {
       constructor. intros pair [[AP [NH [NS [NP NL]]]] C]. apply (N pair). split. {
         split. { invert AP. exact APb. } repeat split; intro NA; [apply NH | apply NS | apply NP | apply NL]; apply ARCB; exact NA. }
@@ -834,12 +794,12 @@ Inductive WellFormedInAcc (cant_bind context : Map.set) : Term.term -> Prop :=
   | Var {name} (I : Map.In context name) ownership
       : WellFormedInAcc cant_bind context $ Term.Var name ownership
   | App
-      {argument cant_bind_in_function} (Uf
-        : forall x, Map.In cant_bind_in_function x <-> (Map.In cant_bind x \/ BoundIn.Term argument x \/ UsedIn.Term argument x))
-      {function cant_bind_in_argument} (Ua
-        : forall x, Map.In cant_bind_in_argument x <-> (Map.In cant_bind x \/ BoundIn.Term function x \/ UsedIn.Term function x))
-      (WFf : WellFormedInAcc cant_bind_in_function context function)
-      (WFa : WellFormedInAcc cant_bind_in_argument context argument)
+      {argument bound_or_used_in_function} (Uf
+        : forall x, Map.In bound_or_used_in_function x <-> (Map.In cant_bind x \/ BoundIn.Term argument x \/ UsedIn.Term argument x))
+      {function bound_or_used_in_argument} (Ua
+        : forall x, Map.In bound_or_used_in_argument x <-> (Map.In cant_bind x \/ BoundIn.Term function x \/ UsedIn.Term function x))
+      (WFf : WellFormedInAcc bound_or_used_in_function context function)
+      (WFa : WellFormedInAcc bound_or_used_in_argument context argument)
       (Db : forall x (Bf : BoundIn.Term function x) (Ba : BoundIn.Term argument x), False)
       : WellFormedInAcc cant_bind context $ Term.App function argument
   | For
@@ -847,14 +807,15 @@ Inductive WellFormedInAcc (cant_bind context : Map.set) : Term.term -> Prop :=
       {type} (NBt : forall (B : BoundIn.Term type variable), False)
       {body} (NBb : forall (B : BoundIn.Term body variable), False)
       (NUt : forall (U : UsedIn.Term type variable), False)
-      {cant_bind_in_type} (Ut
-        : forall x, Map.In cant_bind_in_type x <-> (Map.In cant_bind x \/ BoundIn.Term body x \/ UsedIn.Term body x))
-      {tmp_body} (Tb
+      {tmp_type} (Ut
+        : forall x, Map.In tmp_type x <-> (Map.In cant_bind x \/ BoundIn.Term body x \/ UsedIn.Term body x))
+      {bound_or_used_in_type} (Vt : Map.Add variable tt tmp_type bound_or_used_in_type)
+      {tmp_body} (Ub
         : forall x, Map.In tmp_body x <-> (Map.In cant_bind x \/ BoundIn.Term type x \/ UsedIn.Term type x))
-      {cant_bind_in_body} (Ub : Map.Add variable tt tmp_body cant_bind_in_body)
+      {bound_or_used_in_body} (Vb : Map.Add variable tt tmp_body bound_or_used_in_body)
       {body_context} (Cb : Map.Add variable tt context body_context)
-      (WFt : WellFormedInAcc cant_bind_in_type context type)
-      (WFb : WellFormedInAcc cant_bind_in_body body_context body)
+      (WFt : WellFormedInAcc bound_or_used_in_type context type)
+      (WFb : WellFormedInAcc bound_or_used_in_body body_context body)
       (Db : forall x (Bt : BoundIn.Term type x) (Bb : BoundIn.Term body x), False)
       : WellFormedInAcc cant_bind context $ Term.For variable type body
   | Cas
@@ -862,20 +823,23 @@ Inductive WellFormedInAcc (cant_bind context : Map.set) : Term.term -> Prop :=
       {other_cases} (NBo : forall x (Bp : BoundIn.Pattern pattern x) (B : BoundIn.Term other_cases x), False)
       {body_if_match} (NBb : forall x (Bp : BoundIn.Pattern pattern x) (B : BoundIn.Term body_if_match x), False)
       (NUo : forall x (Bp : BoundIn.Pattern pattern x) (U : UsedIn.Term other_cases x), False)
-      {cant_bind_in_other_cases} (Uo
-        : forall x, Map.In cant_bind_in_other_cases x <-> (
+      {tmp_other_cases : Map.set} (Uo
+        : forall x, Map.In tmp_other_cases x <-> (
           Map.In cant_bind x \/ BoundIn.Term body_if_match x \/ UsedIn.Term body_if_match x))
-      {tmp_body_if_match : Map.set} (Tb
+      {bound_or_used_in_other_cases} (Vo
+        : forall x, Map.In bound_or_used_in_other_cases x <-> (
+          BoundIn.Pattern pattern x \/ Map.In tmp_other_cases x))
+      {tmp_body_if_match : Map.set} (Ub
         : forall x, Map.In tmp_body_if_match x <-> (
           Map.In cant_bind x \/ BoundIn.Term other_cases x \/ UsedIn.Term other_cases x))
-      {cant_bind_in_body_if_match} (Ub
-        : forall x, Map.In cant_bind_in_body_if_match x <-> (
+      {bound_or_used_in_body_if_match} (Vb
+        : forall x, Map.In bound_or_used_in_body_if_match x <-> (
           BoundIn.Pattern pattern x \/ Map.In tmp_body_if_match x))
       {body_if_match_context} (Cb
         : forall x, Map.In body_if_match_context x <-> (
         BoundIn.Pattern pattern x \/ Map.In context x))
-      (WFo : WellFormedInAcc cant_bind_in_other_cases context other_cases)
-      (WFb : WellFormedInAcc cant_bind_in_body_if_match body_if_match_context body_if_match)
+      (WFo : WellFormedInAcc bound_or_used_in_other_cases context other_cases)
+      (WFb : WellFormedInAcc bound_or_used_in_body_if_match body_if_match_context body_if_match)
       (Db : forall x (Bo : BoundIn.Term other_cases x) (Bb : BoundIn.Term body_if_match x), False)
       : WellFormedInAcc cant_bind context $ Term.Cas pattern body_if_match other_cases
   .
@@ -901,8 +865,9 @@ Proof.
     + exact NBb.
     + exact NUt.
     + intro x. rewrite Ut. erewrite (Map.in_eq Er). reflexivity.
-    + intro x. rewrite Tb. erewrite (Map.in_eq Er). reflexivity.
-    + exact Ub.
+    + exact Vt.
+    + intro x. rewrite Ub. rewrite <- (Map.in_eq Er). reflexivity.
+    + exact Vb.
     + eapply Map.add_eq. { exact Cb. } { reflexivity. } { reflexivity. } { exact Ec. } apply Map.eq_refl.
     + apply IHWF1. { apply Map.eq_refl. } exact Ec.
     + apply IHWF2. { apply Map.eq_refl. } apply Map.eq_refl.
@@ -914,8 +879,9 @@ Proof.
     + exact NBb.
     + exact NUo.
     + intro x. rewrite Uo. erewrite (Map.in_eq Er). reflexivity.
-    + intro x. rewrite Tb. erewrite (Map.in_eq Er). reflexivity.
-    + intro x. rewrite Ub. reflexivity.
+    + exact Vo.
+    + intro x. rewrite Ub. erewrite (Map.in_eq Er). reflexivity.
+    + exact Vb.
     + intro x. rewrite Cb. rewrite (Map.in_eq Ec). reflexivity.
     + apply IHWF1. { apply Map.eq_refl. } exact Ec.
     + apply IHWF2. { apply Map.eq_refl. } apply Map.eq_refl.
@@ -951,8 +917,9 @@ Proof.
         -- apply Ht in R as [].
         -- apply Hb in R as [].
         -- destruct here as [x [U B]]. eapply IHb in B as [].
-           do 2 eapply or_intror in U. apply Tb in U as [[] U]. exists tt. apply Ub. right. exact U.
-        -- destruct here as [x [U B]]. eapply IHt in B as []. apply Ut. right. right. exact U.
+           do 2 eapply or_intror in U. apply Ub in U as [[] U]. exists tt. apply Vb. right. exact U.
+        -- destruct here as [x [U B]]. eapply IHt in B as []. apply Map.find_tt. apply Vt.
+           right. apply Map.find_tt. apply Ut. right. right. exact U.
         -- apply St in R as [].
         -- apply Sb in R as [].
         -- destruct here as [x [Bt Bb]]. apply (Db x). { exact Bt. } exact Bb.
@@ -964,8 +931,9 @@ Proof.
         -- apply Lt in R as [].
         -- apply Lb in R as [].
       * split; intros.
-        -- invert B; [apply NB in I as [] | |]. { eapply IHt. { exact bound_in_type. } apply Ut. left. exact I. }
-           eapply IHb. { exact bound_in_body. } eapply or_introl in I. apply Tb in I as [[] F]. exists tt. apply Ub. right. exact F.
+        -- invert B; [apply NB in I as [] | |]. { eapply IHt. { exact bound_in_type. }
+             apply Map.find_tt. apply Vt. right. apply Map.find_tt. apply Ut. left. exact I. }
+           eapply IHb. { exact bound_in_body. } eapply or_introl in I. apply Ub in I as [[] F]. exists tt. apply Vb. right. exact F.
         -- invert U. { apply IHt. exact used_in_type. } eapply IHb in used_in_body as [[] U].
            apply Cb in U as [[E _] | U]. { apply not_shadowed in E as []. } exists tt. exact U.
     + destruct IHWF1 as [[WPo [Hb [Sb [Pb Lb]]]] IHo]. destruct IHWF2 as [[WPb [Ho [So [Po Lo]]]] IHb]. split.
@@ -975,8 +943,8 @@ Proof.
         -- destruct here as [x [Bp B]]. apply NBo in B as []. exact Bp.
         -- apply Ho in R as [].
         -- apply Hb in R as [].
-        -- destruct here as [x [U B]]. eapply IHo in B as []. apply Uo. right. right. exact U.
-        -- destruct here as [x [U B]]. eapply IHb in B as []. apply Ub. right. apply Tb. right. right. exact U.
+        -- destruct here as [x [U B]]. eapply IHo in B as []. apply Vo. right. apply Uo. right. right. exact U.
+        -- destruct here as [x [U B]]. eapply IHb in B as []. apply Vb. right. apply Ub. right. right. exact U.
         -- apply So in R as [].
         -- apply Sb in R as [].
         -- destruct here as [x [Bo Bb]]. apply (Db x). { exact Bb. } exact Bo.
@@ -989,8 +957,8 @@ Proof.
         -- apply Lb in R as [].
       * split; intros.
         -- invert B; [apply NB in I as []; exact bound_in_pattern | |].
-           ++ eapply IHb. { exact bound_in_body. } apply Ub. right. eapply or_introl in I. apply Tb in I. exact I.
-           ++ eapply IHo. { exact bound_in_another_case. } apply Uo. left. exact I.
+           ++ eapply IHb. { exact bound_in_body. } apply Vb. right. eapply or_introl in I. apply Ub in I. exact I.
+           ++ eapply IHo. { exact bound_in_another_case. } apply Vo. right. apply Uo. left. exact I.
         -- invert U. 2: { apply IHo. exact used_in_another_case. } eapply IHb in used_in_body as I.
            apply Cb in I as [B | I]. { apply not_shadowed in B as []. } exact I.
   - generalize dependent context. generalize dependent cant_bind. induction t; intros; cbn in *.
@@ -1035,6 +1003,7 @@ Proof.
            [apply BoundIn.term_iff | apply UsedIn.term_iff]; exact I.
         -- intro IBU. repeat rewrite Map.in_overriding_union. destruct IBU as [I | [B | U]]; [left; exact I | |]; right;
            [left | right]; [apply BoundIn.term_iff | apply UsedIn.term_iff]; assumption.
+      * apply Map.add_set.
       * split.
         -- intro I. apply Map.in_overriding_union in I as [I | I]; [left | right]. { exact I. }
            apply Map.in_overriding_union in I as [I | I]; [left | right];
@@ -1045,8 +1014,9 @@ Proof.
       * apply Map.add_set.
       * apply IHt1. split. { split. { invert AP. exact APt. }
           repeat split; intro C; [apply NH | apply NS | apply NP | apply NL]; apply ARFT; exact C. }
-        split. 2: { intro U. apply WF. apply UsedIn.FoT. exact U. }
-        intros. apply Map.in_overriding_union in I as [I | I]. { eapply WF. 2: { exact I. } apply BoundIn.TFoT. exact B. }
+        split. 2: { intro U. apply WF. apply UsedIn.FoT. exact U. } intros. apply Map.in_overriding_add in I as [-> | I]. {
+          apply NH. apply APFT. exists variable. split. { reflexivity. } exact B. }
+        apply Map.in_overriding_union in I as [I | I]. { eapply WF. 2: { exact I. } apply BoundIn.TFoT. exact B. }
         apply Map.in_overriding_union in I as [I | I]; [apply BoundIn.term_iff in I | apply UsedIn.term_iff in I].
         -- apply NP. apply APFT. exists x. split. { exact B. } exact I.
         -- apply NS. apply APFB. { constructor. } exists x. split. { exact I. } exact B.
@@ -1073,18 +1043,17 @@ Proof.
            [apply BoundIn.term_iff | apply UsedIn.term_iff]; exact I.
         -- intro IBU. repeat rewrite Map.in_overriding_union. destruct IBU as [I | [B | U]]; [left; exact I | |]; right;
            [left | right]; [apply BoundIn.term_iff | apply UsedIn.term_iff]; assumption.
-      * split.
-        -- intro I. apply Map.in_overriding_union in I as [I | I]; [left | right]. { exact I. }
-           apply Map.in_overriding_union in I as [I | I]; [left | right];
-           [apply BoundIn.term_iff | apply UsedIn.term_iff]; exact I.
-        -- intro IBU. repeat rewrite Map.in_overriding_union. destruct IBU as [I | [B | U]]; [left; exact I | |]; right;
-           [left | right]; [apply BoundIn.term_iff | apply UsedIn.term_iff]; assumption.
-      * intro x. assert (B := BoundIn.pattern_iff). cbn in B. rewrite <- B. apply Map.in_overriding_union.
-      * intro x. assert (B := BoundIn.pattern_iff). cbn in B. rewrite <- B. apply Map.in_overriding_union.
+      * intro x. rewrite Map.in_overriding_union at 1. rewrite <- (BoundIn.pattern_iff _ _). reflexivity.
+      * intro x. rewrite (Map.in_overriding_union cant_bind). rewrite Map.in_overriding_union.
+        rewrite <- (BoundIn.term_iff _ _). rewrite <- (UsedIn.term_iff _ _). reflexivity.
+      * intro x. rewrite <- (BoundIn.pattern_iff _ _). apply Map.in_overriding_union.
+      * intro x. rewrite <- (BoundIn.pattern_iff _ _). apply Map.in_overriding_union.
       * apply IHt2. split. { split. { invert AP. exact APo. }
           repeat split; intro C; [apply NH | apply NS | apply NP | apply NL]; apply ARCO; exact C. }
         split. 2: { intro U. apply WF. apply UsedIn.CaO. exact U. }
-        intros. apply Map.in_overriding_union in I as [I | I]. { apply (WF x). { apply BoundIn.TCaO. exact B. } exact I. }
+        intros. apply Map.in_overriding_union in I as [I | I]. {
+          apply NH. apply APCO. exists x. split. { apply BoundIn.pattern_iff. exact I. } exact B. }
+        apply Map.in_overriding_union in I as [I | I]. { apply (WF x). { apply BoundIn.TCaO. exact B. } exact I. }
         apply Map.in_overriding_union in I as [I | I]; [apply BoundIn.term_iff in I | apply UsedIn.term_iff in I].
         -- apply NP. apply APCB. { constructor. } exists x. split. { exact I. } exact B.
         -- apply NS. apply APCB. { constructor. } exists x. split. { exact I. } exact B.
@@ -1114,14 +1083,52 @@ Proof.
   - constructor.
   - constructor. destruct I as [[] F]. exists tt. apply subset. exact F.
   - econstructor. { exact Uf. } { exact Ua. } { apply IHWF1. exact subset. } { apply IHWF2. exact subset. } exact Db.
-  - econstructor. { exact NB. } { exact NBt. } { exact NBb. } { exact NUt. } { exact Ut. } { exact Tb. } { exact Ub. }
+  - econstructor. { exact NB. } { exact NBt. } { exact NBb. } { exact NUt. } { exact Ut. } { exact Vt. } { exact Ub. } { exact Vb. }
     { apply Map.add_set. } { apply IHWF1. exact subset. } 2: { exact Db. } apply IHWF2. intros. apply Map.add_set.
     apply Cb in F as [[-> ->] | F]; [left | right]. { split; reflexivity. } apply subset. exact F.
-  - econstructor. { exact WFp. } { exact NB. } { exact NBo. } { exact NBb. } { exact NUo. } { exact Uo. } { exact Tb. } { exact Ub. }
-    { intro x. rewrite <- (BoundIn.pattern_iff pattern x). apply Map.in_overriding_union. } { apply IHWF1. exact subset. }
+  - econstructor. { exact WFp. } { exact NB. } { exact NBo. } { exact NBb. } { exact NUo. } { exact Uo. } { exact Vo. } { exact Ub. }
+    { exact Vb. } { intro x. rewrite <- (BoundIn.pattern_iff pattern x). apply Map.in_overriding_union. } { apply IHWF1. exact subset. }
     2: { exact Db. } apply IHWF2. intros k [] F. apply Map.union_set. eassert (I : Map.In _ _). { exists tt. exact F. }
     apply Cb in I as [I | I]; [left | right]. { apply BoundIn.pattern_iff in I as [[] F']. exact F'. }
     destruct I as [[] F']. apply subset. exact F'.
+Qed.
+
+Lemma context_minus {cant_bind big t} (WF : WellFormedInAcc cant_bind big t)
+  {x y lil} (A : Map.Add x y lil big)
+  (N : Map.In lil x \/ (forall (U : UsedIn.Term t x), False))
+  : WellFormedInAcc cant_bind lil t.
+Proof.
+  destruct y. generalize dependent lil. generalize dependent x. induction WF; intros; cbn in *.
+  - constructor.
+  - constructor. destruct I as [[] F]. apply A in F as [[-> _] | F]. 2: { exists tt. exact F. }
+    destruct N as [I | N]. { exact I. } contradiction N. constructor.
+  - econstructor. { exact Uf. } { exact Ua. } 3: { exact Db. }
+    + eapply IHWF1. { exact A. } destruct N as [I | N]; [left | right]. { exact I. }
+      intro U. apply N. apply UsedIn.ApF. exact U.
+    + eapply IHWF2. { exact A. } destruct N as [I | N]; [left | right]. { exact I. }
+      intro U. apply N. apply UsedIn.ApA. exact U.
+  - econstructor. { exact NB. } { exact NBt. } { exact NBb. } { exact NUt. } { exact Ut. }
+    { exact Vt. } { exact Ub. } { exact Vb. } { apply Map.add_set. } 3: { exact Db. }
+    + eapply IHWF1. { exact A. } destruct N as [I | N]; [left | right]. { exact I. }
+      intro U. apply N. apply UsedIn.FoT. exact U.
+    + eapply IHWF2.
+      * intros k []. rewrite Cb. rewrite A. rewrite (Map.add_set _).
+        rewrite <- or_assoc. rewrite (or_comm (_ /\ _)). rewrite or_assoc. reflexivity.
+      * destruct (String.eqb_spec x variable). { left. apply Map.in_overriding_add. left. exact e. }
+        destruct N as [I | N]; [left | right]. { apply Map.in_overriding_add. right. exact I. }
+        intro U. apply N. apply UsedIn.FoB. { exact n. } exact U.
+  - econstructor. { exact WFp. } { exact NB. } { exact NBo. } { exact NBb. } { exact NUo. } { exact Uo. }
+    { exact Vo. } { exact Ub. } { exact Vb. } 4: { exact Db. } {
+      intros. rewrite <- (BoundIn.pattern_iff _ _). apply Map.in_overriding_union. }
+    + eapply IHWF1. { exact A. } destruct N as [I | N]; [left | right]. { exact I. }
+      intro U. apply N. apply UsedIn.CaO. exact U.
+    + eapply IHWF2.
+      * intros k []. rewrite Map.find_tt. rewrite Cb. rewrite <- Map.find_tt. rewrite A. rewrite (Map.union_set _ _ _).
+        repeat rewrite Map.find_tt. rewrite (BoundIn.pattern_iff _ _). rewrite <- or_assoc.
+        rewrite (or_comm $ BoundIn.Pattern _ _). rewrite or_assoc. reflexivity.
+      * destruct (BoundIn.pattern_spec pattern x). { left. apply Map.in_overriding_union. left. apply BoundIn.pattern_iff. exact Y. }
+        destruct N as [I | N]; [left | right]. { apply Map.in_overriding_union. right. exact I. }
+        intro U. apply N. apply UsedIn.CaB. { exact N0. } exact U.
 Qed.
 
 Lemma cant_bind_subset {big context t} (WF : WellFormedInAcc big context t)
@@ -1152,21 +1159,22 @@ Proof.
     + apply NUt in U as [].
     + rewrite <- (BoundIn.term_iff body x). rewrite <- (UsedIn.term_iff body x).
       repeat rewrite <- Map.in_overriding_union. reflexivity.
+    + apply Map.add_set.
     + rewrite <- (BoundIn.term_iff type x). rewrite <- (UsedIn.term_iff type x).
       repeat rewrite <- Map.in_overriding_union. reflexivity.
     + apply Map.add_set.
     + apply Map.add_set.
     + apply IHWF1. intros x [] F. eassert (I : @Map.In unit _ _). 2: { destruct I as [[] F']. exact F'. }
-      apply Ut. apply Map.union_set in F as [F | F]; [left | right]. { exists tt. eapply subset. exact F. }
+      apply Map.find_tt. apply Vt. apply Map.add_set in F as [[-> _] | F]; [left | right]. { split; reflexivity. }
+      apply Map.find_tt. apply Ut. apply Map.union_set in F as [F | F]; [left | right]. { exists tt. eapply subset. exact F. }
       apply Map.union_set in F as [F | F]; [left | right]. { apply BoundIn.term_iff. exists tt. exact F. }
       apply UsedIn.term_iff. exists tt. exact F.
     + eapply context_superset; [apply IHWF2 |]. 2: {
         intros x [] F. apply Map.add_set. apply Cb in F as [[-> _] | F]; [left | right]. { split; reflexivity. } exact F. }
-      intros x [] F. apply Ub. apply Map.add_set in F as [E | F]; [left | right]. { exact E. }
-      eassert (I : @Map.In unit _ _). 2: { destruct I as [[] F']. exact F'. } apply Tb.
-      apply Map.union_set in F as [F | F]; [left | right]. { exists tt. apply subset. exact F. }
-      apply Map.union_set in F as [F | F]; [left | right]. { apply BoundIn.term_iff. exists tt. exact F. }
-      apply UsedIn.term_iff. exists tt. exact F.
+      intros x [] F. apply Vb. apply Map.add_set in F as [[-> _] | F]; [left | right]. { split; reflexivity. }
+      apply Map.find_tt. apply Ub. apply Map.union_set in F as [F | F]. { left. exists tt. apply subset. exact F. }
+      right. apply Map.union_set in F as [F | F]; [left | right];
+      [apply BoundIn.term_iff | apply UsedIn.term_iff]; exists tt; exact F.
     + apply (Db x). { exact Bt. } exact Bb.
   - econstructor; intros.
     + exact WFp.
@@ -1176,23 +1184,24 @@ Proof.
     + apply NUo in U as []. exact Bp.
     + rewrite <- (BoundIn.term_iff body_if_match x). rewrite <- (UsedIn.term_iff body_if_match x).
       repeat rewrite <- Map.in_overriding_union. reflexivity.
+    + rewrite Map.in_overriding_union at 1. rewrite <- (BoundIn.pattern_iff _ _). reflexivity.
     + rewrite <- (BoundIn.term_iff other_cases x). rewrite <- (UsedIn.term_iff other_cases x).
       repeat rewrite <- Map.in_overriding_union. reflexivity.
     + rewrite <- (BoundIn.pattern_iff pattern x). apply Map.in_overriding_union.
     + rewrite <- (BoundIn.pattern_iff pattern x). apply Map.in_overriding_union.
     + apply IHWF1. intros x [] F. eassert (I : @Map.In unit _ _). 2: { destruct I as [[] F']. exact F'. }
-      apply Uo. apply Map.union_set in F as [F | F]; [left | right]. { exists tt. eapply subset. exact F. }
-      apply Map.union_set in F as [F | F]; [left | right]. { apply BoundIn.term_iff. exists tt. exact F. }
+      apply Vo. apply Map.union_set in F as [F | F]; [left | right]. { apply BoundIn.pattern_iff. exists tt. exact F. }
+      apply Uo. apply Map.union_set in F as [F | F]. { left. exists tt. apply subset. exact F. }
+      right. apply Map.union_set in F as [F | F]; [left | right]. { apply BoundIn.term_iff. exists tt. exact F. }
       apply UsedIn.term_iff. exists tt. exact F.
     + eapply context_superset; [apply IHWF2 |]. 2: {
         intros x [] F. apply Map.union_set. eassert (I : Map.In _ _). { exists tt. exact F. }
         apply Cb in I as [I | I]; [left | right]. { apply BoundIn.pattern_iff in I as [[] F']. exact F'. }
         destruct I as [[] F']. exact F'. }
-      intros x [] F. eassert (I : @Map.In unit _ _). 2: { destruct I as [[] F']. exact F'. } apply Ub.
-      apply Map.union_set in F as [F | F]; [left | right]. { apply BoundIn.pattern_iff. exists tt. exact F. }
-      apply Tb. apply Map.union_set in F as [F | F]; [left | right]. { exists tt. apply subset. exact F. }
-      apply Map.union_set in F as [F | F]; [left | right]. { apply BoundIn.term_iff. exists tt. exact F. }
-      apply UsedIn.term_iff. exists tt. exact F.
+      intros x [] F. apply Map.find_tt. apply Vb. apply Map.union_set in F as [F | F]; [left | right]. {
+        apply BoundIn.pattern_iff. exists tt. exact F. }
+      apply Ub. apply Map.union_set in F as [F | F]; [left | right]. { exists tt. apply subset. exact F. }
+      apply Map.union_set in F as [F | F]; [left | right]; [apply BoundIn.term_iff | apply UsedIn.term_iff]; exists tt; exact F.
     + apply (Db x). { exact Bo. } exact Bb.
 Qed.
 
@@ -1241,40 +1250,28 @@ Proof.
     + apply NUt in U as [].
     + rewrite <- (BoundIn.term_iff body x). rewrite <- (UsedIn.term_iff body x).
       repeat rewrite <- Map.in_overriding_union. reflexivity.
+    + apply Map.add_set.
     + rewrite <- (BoundIn.term_iff type x). rewrite <- (UsedIn.term_iff type x).
       repeat rewrite <- Map.in_overriding_union. reflexivity.
     + apply Map.add_set.
     + apply Map.add_set.
     + eapply IHWF1. { intros. apply (NB0 x). { apply BoundIn.TFoT. exact B. } exact I. } intros x []. split.
-      * intro F. apply Map.union_set in F as [F | F].
-        -- apply union in F as [F | F]. 2: { right. exact F. }
-           left. eassert (I : @Map.In unit _ _). 2: { destruct I as [[] F']. exact F'. }
-           apply Ut. left. exists tt. exact F.
-        -- left. eassert (I : @Map.In unit _ _). 2: { destruct I as [[] F']. exact F'. }
-           apply Ut. right. apply Map.union_set in F as [F | F]; [left | right];
-           [apply BoundIn.term_iff | apply UsedIn.term_iff]; exists tt; assumption.
-      * intro FF. apply Map.union_set. rewrite union. destruct FF as [F | F]. 2: { left. right. exact F. }
-        eassert (I : Map.In _ _). { exists tt. exact F. } apply Ut in I as [[[] F'] | I]. { left. left. exact F'. }
-        right. apply Map.union_set. destruct I as [B | U]; [left | right];
-        [apply BoundIn.term_iff in B as [[] F'] | apply UsedIn.term_iff in U as [[] F']]; exact F'.
+      * intro F. apply Map.add_set in F as [[-> _] | F]. { left. apply Vt. left. split; reflexivity. }
+        apply Map.union_set in F as [F | F]. { apply union in F as [F | F]. 2: { right. exact F. }
+          left. apply Vt. right. apply Map.find_tt. apply Ut. left. exists tt. exact F. }
+        left. apply Vt. right. apply Map.find_tt. apply Ut. right.
+        apply Map.union_set in F as [F | F]; [left | right]; [apply BoundIn.term_iff | apply UsedIn.term_iff]; exists tt; exact F.
+      * intro FF. apply Map.add_set. repeat rewrite (Map.union_set _ _ _). rewrite union. rewrite or_assoc.
+        repeat rewrite Map.find_tt. rewrite (BoundIn.term_iff _ _). rewrite (UsedIn.term_iff _ _).
+        destruct FF as [F | F]. 2: { right. right. left. exists tt. exact F. }
+        apply Vt in F as [[-> _] | F]; [left | right]. { split; reflexivity. } apply Map.find_tt in F.
+        apply Ut in F as [I | [B | U]]. { left. exact I. } { right. right. left. exact B. } right. right. right. exact U.
     + eapply context_superset; [eapply IHWF2 |]. { intros. apply (NB0 x). { apply BoundIn.TFoB. exact B. } exact I. } 2: {
-        intros x [] F. apply Map.add_set. apply Cb. exact F. } intros x []. split.
-      * intro F. apply Map.add_set in F as [[-> _] | F]. { left. apply Ub. left. split; reflexivity. }
-        apply Map.union_set in F as [F | F].
-        -- apply union in F as [F | F]. 2: { right. exact F. }
-           left. eassert (I : @Map.In unit _ _). 2: { destruct I as [[] F']. exact F'. }
-           exists tt. apply Ub. right. eassert (I : @Map.In unit _ _). 2: { destruct I as [[] F']. exact F'. }
-           apply Tb. left. exists tt. exact F.
-        -- left. eassert (I : @Map.In unit _ _). 2: { destruct I as [[] F']. exact F'. }
-           exists tt. apply Ub. right. eassert (I : @Map.In unit _ _). 2: { destruct I as [[] F']. exact F'. }
-           apply Tb. right. apply Map.union_set in F as [F | F]; [left | right];
-           [apply BoundIn.term_iff | apply UsedIn.term_iff]; exists tt; assumption.
-      * intro FF. apply Map.add_set. assert (E := Map.union_set); cbn in E; repeat rewrite E; clear E.
-        rewrite union. destruct FF as [F | F]. 2: { right. left. right. exact F. }
-        apply Ub in F as [E | F]; [left | right]. { exact E. }
-        eassert (I : Map.In _ _). { exists tt. exact F. } apply Tb in I as [[[] F'] | I]. { left. left. exact F'. }
-        right. destruct I as [B | U]; [left | right];
-        [apply BoundIn.term_iff in B as [[] F'] | apply UsedIn.term_iff in U as [[] F']]; exact F'.
+        intros x [] F. apply Map.add_set. apply Cb. exact F. }
+      intros x []. rewrite (Map.add_set _). repeat rewrite (Map.union_set _ _ _). rewrite union. rewrite Vb.
+      repeat rewrite Map.find_tt. rewrite Ub. repeat rewrite or_assoc. rewrite (BoundIn.term_iff _ _). rewrite (UsedIn.term_iff _ _).
+      rewrite (or_comm _ $ Map.In marginal x). repeat rewrite <- (or_assoc _ $ Map.In marginal x).
+      rewrite (or_comm (BoundIn.Term type x) $ Map.In marginal x). repeat rewrite or_assoc. reflexivity.
     + apply (Db x). { exact Bt. } exact Bb.
   - econstructor; intros.
     + exact WFp.
@@ -1283,71 +1280,422 @@ Proof.
     + apply NBo in B as []. exact Bp.
     + apply NBb in B as []. exact Bp.
     + apply NUo in U as []. exact Bp.
-    + rewrite <- (BoundIn.term_iff body_if_match x). rewrite <- (UsedIn.term_iff body_if_match x).
-      repeat rewrite <- Map.in_overriding_union. reflexivity.
+    + rewrite (Map.in_overriding_union big). rewrite Map.in_overriding_union.
+      rewrite <- (BoundIn.term_iff _ _). rewrite <- (UsedIn.term_iff _ _). reflexivity.
+    + rewrite <- (BoundIn.pattern_iff _ _). apply Map.in_overriding_union.
     + rewrite <- (BoundIn.term_iff other_cases x). rewrite <- (UsedIn.term_iff other_cases x).
       repeat rewrite <- Map.in_overriding_union. reflexivity.
     + rewrite <- (BoundIn.pattern_iff pattern x). apply Map.in_overriding_union.
     + rewrite <- (BoundIn.pattern_iff pattern x). apply Map.in_overriding_union.
     + eapply IHWF1. { intros. apply (NB0 x). { apply BoundIn.TCaO. exact B. } exact I. } intros x []. split.
-      * intro F. apply Map.union_set in F as [F | F].
-        -- apply union in F as [F | F]. 2: { right. exact F. }
-           left. eassert (I : @Map.In unit _ _). 2: { destruct I as [[] F']. exact F'. }
-           apply Uo. left. exists tt. exact F.
-        -- left. eassert (I : @Map.In unit _ _). 2: { destruct I as [[] F']. exact F'. }
-           apply Uo. right. apply Map.union_set in F as [F | F]; [left | right];
-           [apply BoundIn.term_iff | apply UsedIn.term_iff]; exists tt; assumption.
-      * intro FF. apply Map.union_set. rewrite union. destruct FF as [F | F]. 2: { left. right. exact F. }
-        eassert (I : Map.In _ _). { exists tt. exact F. } apply Uo in I as [[[] F'] | I]. { left. left. exact F'. }
-        right. apply Map.union_set. destruct I as [B | U]; [left | right];
-        [apply BoundIn.term_iff in B as [[] F'] | apply UsedIn.term_iff in U as [[] F']]; exact F'.
+      * intro F. apply Map.union_set in F as [F | F]. {
+          left. apply Map.find_tt. apply Vo. left. apply BoundIn.pattern_iff. exists tt. exact F. }
+        apply Map.union_set in F as [F | F]. { apply union in F as [F | F]. 2: { right. exact F. }
+          left. apply Map.find_tt. apply Vo. right. apply Uo. left. exists tt. exact F. }
+        left. apply Map.find_tt. apply Vo. right. apply Uo. right.
+        apply Map.union_set in F as [F | F]; [left | right]; [apply BoundIn.term_iff | apply UsedIn.term_iff]; exists tt; exact F.
+      * intro FF. repeat rewrite (Map.union_set _ _ _). rewrite union. rewrite or_assoc.
+        destruct FF as [F | F]. 2: { right. right. left. exact F. }
+        apply Map.find_tt in F as I; clear F. apply Vo in I as [B | I]. { left. apply BoundIn.pattern_iff in B as [[] F]. exact F. }
+        right. apply Uo in I as [I | [B | U]]. { left. apply Map.find_tt. exact I. } {
+          right. right. left. apply BoundIn.term_iff in B as [[] F]. exact F. } right. right. right.
+        apply UsedIn.term_iff in U as [[] F]. exact F.
     + eapply context_superset; [eapply IHWF2 |]. { intros. apply (NB0 x). { apply BoundIn.TCaB. exact B. } exact I. } 2: {
         intros x [] F. apply Map.union_set. destruct (Cb x) as [[B | [[] F']] _]; [exists tt; exact F | left | right]. {
           apply BoundIn.pattern_iff in B as [[] B]. exact B. } exact F'. }
-      intros x []. split.
-      * intro F. apply Map.union_set in F as [F | F]. {
-          left. eassert (I : @Map.In unit _ _). 2: { destruct I as [[] F']. exact F'. }
-          apply Ub. left. apply BoundIn.pattern_iff. exists tt. exact F. }
-        apply Map.union_set in F as [F | F].
-        -- apply union in F as [F | F]. 2: { right. exact F. }
-           left. eassert (I : @Map.In unit _ _). 2: { destruct I as [[] F']. exact F'. }
-           apply Ub. right. apply Tb. left. exists tt. exact F.
-        -- left. eassert (I : @Map.In unit _ _). 2: { destruct I as [[] F']. exact F'. }
-           apply Ub. right. apply Tb. right. apply Map.union_set in F as [F | F]; [left | right];
-           [apply BoundIn.term_iff | apply UsedIn.term_iff]; exists tt; assumption.
-      * intro FF. assert (E := Map.union_set); cbn in E; repeat rewrite E; clear E.
-        rewrite union. destruct FF as [F | F]. 2: { right. left. right. exact F. }
-        eassert (I : Map.In _ _). { exists tt. exact F. }
-        apply Ub in I as [B | I]; [left | right]. { apply BoundIn.pattern_iff in B as [[] F']. exact F'. }
-        apply Tb in I as [[[] F'] | I]; [left | right]. { left. exact F'. }
-        destruct I as [B | U]; [left | right];
-        [apply BoundIn.term_iff in B as [[] F'] | apply UsedIn.term_iff in U as [[] F']]; exact F'.
+      intros x []. repeat rewrite (Map.union_set _ _ _). rewrite union. repeat rewrite Map.find_tt. rewrite Vb. rewrite Ub.
+      repeat rewrite or_assoc. rewrite (BoundIn.term_iff _ _). rewrite (UsedIn.term_iff _ _). rewrite (BoundIn.pattern_iff _ _).
+      rewrite (or_comm _ $ Map.In marginal x). rewrite <- (or_assoc (BoundIn.Term other_cases x) $ Map.In marginal x).
+      rewrite (or_comm _ $ Map.In marginal x). rewrite or_assoc. reflexivity.
     + apply (Db x). { exact Bo. } exact Bb.
 Qed.
 
 
 
-(* TODO: make sure that bindings are disjoint: i.e., binding the same name implies that two terms are the same *)
-Definition WellFormedContext context : Prop := (
-  forall domain (D : Map.Domain context domain),
-  Map.ForAll (fun _ => Unshadow.WellFormedIn domain) context) /\
-  forall x1 y1 (F1 : Map.Find context x1 y1) x (B1 : BoundIn.Term y1 x)
-  x2 y2 (F2 : Map.Find context x2 y2) (B2 : BoundIn.Term y2 x),
-  y1 = y2.
+Lemma used_before
+  {acc cant_bind} (cant_bind_range : forall y (IR : Map.InRange acc y), Map.In cant_bind y)
+  {t cant_bind' t'} (E : unshadow_acc acc cant_bind t = Some (cant_bind', t')) {y}
+  : UsedIn.Term t' y <-> exists x, (Map.Find acc x y /\ UsedIn.Term t x).
+Proof.
+  generalize dependent y. generalize dependent t'. generalize dependent cant_bind'.
+  generalize dependent cant_bind. generalize dependent acc. induction t; intros.
+  - invert E. split. { intro U. invert U. } intros [x [F U]]. invert U.
+  - unfold unshadow_acc in E. destruct Map.find eqn:F in E; invert E. apply Map.find_iff in F.
+    split. { intro U. invert U. eexists. split. { exact F. } constructor. }
+    intros [z [F' U]]. invert U. destruct (Map.find_det F F'). constructor.
+  - rewrite unshadow_app in E. destruct unshadow_acc as [[bound_or_used_f f'] |] eqn:Ef in E. 2: { discriminate E. }
+    destruct unshadow_acc as [[bound_or_used_a a'] |] eqn:Ea in E; invert E. specialize (IHt1 _ _ cant_bind_range _ _ Ef y).
+    eassert (cant_bind_range' : _); [| specialize (IHt2 _ _ cant_bind_range' _ _ Ea y)]. {
+      intros z IR. apply (bound_or_used Ef). right. right. apply cant_bind_range. exact IR. }
+    split.
+    + intro U. invert U.
+      * apply IHt1 in used_in_function as [x [F U]]. exists x. split. { exact F. } apply UsedIn.ApF. exact U.
+      * apply IHt2 in used_in_argument as [x [F U]]. exists x. split. { exact F. } apply UsedIn.ApA. exact U.
+    + intros [x [F U]]. invert U.
+      * apply UsedIn.ApF. apply IHt1. exists x. split. { exact F. } exact used_in_function.
+      * apply UsedIn.ApA. apply IHt2. exists x. split. { exact F. } exact used_in_argument.
+  - rewrite unshadow_for in E. rename t' into term'.
+    destruct unshadow_acc as [[bound_or_used_t t'] |] eqn:Et in E. 2: { discriminate E. }
+    destruct unshadow_acc as [[bound_or_used_b b'] |] eqn:Eb in E; invert E.
+    eassert (cant_bind_range_t : _); [| specialize (IHt1 _ _ cant_bind_range_t _ _ Et y)]. {
+      intros z IR. apply Map.in_overriding_add. right. apply cant_bind_range. exact IR. }
+    eassert (cant_bind_range_b : _); [| specialize (IHt2 _ _ cant_bind_range_b _ _ Eb y)]. {
+      intros z [x F]. apply (bound_or_used Et). right. right. apply Map.in_overriding_add.
+      apply Map.find_overriding_add in F as [[-> ->] | [N F]]; [left | right]. { reflexivity. }
+      apply cant_bind_range. exists x. exact F. }
+    split.
+    + intro U. invert U.
+      * apply IHt1 in used_in_type as [x [F U]]. exists x. split. { exact F. } apply UsedIn.FoT. exact U.
+      * apply IHt2 in used_in_body as [x [F U]]. apply Map.find_overriding_add in F as [[-> ->] | [N F]]. {
+          contradiction not_shadowed. reflexivity. }
+        exists x. split. { exact F. } apply UsedIn.FoB. { exact N. } exact U.
+    + intros [x [F U]]. invert U.
+      * apply UsedIn.FoT. apply IHt1. exists x. split. { exact F. } exact used_in_type.
+      * apply UsedIn.FoB. { intros ->. eapply NewNames.not_in_new_name. eapply cant_bind_range. exists x. exact F. }
+        apply IHt2. exists x. split. 2: { exact used_in_body. } apply Map.find_overriding_add. right. split; assumption.
+  - rewrite unshadow_cas in E. destruct unshadow_acc as [[bound_or_used_o o'] |] eqn:Eo in E. 2: { discriminate E. }
+    destruct (Rename.pattern_spec (NewNames.one_to_one_generate cant_bind $ BoundIn.pattern pattern) pattern). 2: { discriminate E. }
+    destruct unshadow_acc as [[bound_or_used_b b'] |] eqn:Eb in E; invert E.
+    eassert (cant_bind_range_o : _); [| specialize (IHt2 _ _ cant_bind_range_o _ _ Eo y)]. {
+      intros z IR. apply Map.in_overriding_union. right. apply cant_bind_range. exact IR. }
+    eassert (cant_bind_range_b : _); [| specialize (IHt1 _ _ cant_bind_range_b _ _ Eb y)]. {
+      intros y' [x' F]. apply (bound_or_used Eo). right. right. apply Map.in_overriding_union.
+      apply Map.bulk_overwrite_bulk_overwrite in F as [F | [N F]]; [left | right]. { apply Map.in_space_range. exists x'. exact F. }
+      apply cant_bind_range. exists x'. exact F. }
+    split.
+    + intro U. invert U.
+      * apply IHt1 in used_in_body as [x' [F U]]. apply Map.bulk_overwrite_bulk_overwrite in F as [F | [N F]]. 2: {
+          exists x'. split. { exact F. } apply UsedIn.CaB. 2: { exact U. }
+          intro B. apply not_shadowed. apply (Rename.bound_in_pattern Y). exists x'. split. { exact B. }
+          contradiction N. apply NewNames.in_generate. apply BoundIn.pattern_iff. exact B. }
+        contradiction not_shadowed. apply (Rename.bound_in_pattern Y). exists x'. split. 2: { exact F. }
+        apply BoundIn.pattern_iff. eapply NewNames.in_generate. exists y. exact F.
+      * apply IHt2 in used_in_another_case as [x' [F U]]. exists x'. split. { exact F. } apply UsedIn.CaO. exact U.
+    + intros [x' [F U]]. invert U.
+      * apply UsedIn.CaB.
+        -- intro B. apply (Rename.bound_in_pattern Y) in B as [x'' [B F']].
+           eapply NewNames.not_in_generate. 2: { exists x''. exact F'. } apply cant_bind_range. exists x'. exact F.
+        -- apply IHt1. exists x'. split. 2: { exact used_in_body. } apply Map.bulk_overwrite_bulk_overwrite. right.
+           split. 2: { exact F. } intro I. apply not_shadowed. apply BoundIn.pattern_iff. eapply NewNames.in_generate. exact I.
+      * apply UsedIn.CaO. apply IHt2. exists x'. split. { exact F. } exact used_in_another_case.
+Qed.
+
+Lemma in_range {acc cant_bind t bound_or_used' t'} (E : unshadow_acc acc cant_bind t = Some (bound_or_used', t'))
+  {x} (U : UsedIn.Term t' x)
+  : Map.InRange acc x.
+Proof.
+  generalize dependent x. generalize dependent t'. generalize dependent bound_or_used'.
+  generalize dependent cant_bind. generalize dependent acc. induction t; intros.
+  - cbn in E. invert E. invert U.
+  - cbn in E. destruct (Map.find_spec acc name); invert E. invert U. exists name. exact Y.
+  - cbn in E. destruct unshadow_acc as [[bound_or_used_f f'] |] eqn:E1 in E. 2: { discriminate E. }
+    specialize (IHt1 _ _ _ _ E1). destruct unshadow_acc as [[bound_or_used_a a'] |] eqn:E2 in E; invert E.
+    specialize (IHt2 _ _ _ _ E2). invert U; [apply IHt1 | apply IHt2]; assumption.
+  - rewrite unshadow_for in E. destruct unshadow_acc as [[bound_or_used_y y'] |] eqn:E1 in E. 2: { discriminate E. }
+    specialize (IHt1 _ _ _ _ E1). destruct unshadow_acc as [[bound_or_used_b b'] |] eqn:E2 in E; invert E.
+    specialize (IHt2 _ _ _ _ E2). invert U. { apply IHt1. exact used_in_type. } specialize (IHt2 _ used_in_body) as [z F].
+    apply Map.overwrite_if_present_overwrite in F as [[-> ->] | [N F]]. { contradiction not_shadowed. reflexivity. }
+    exists z. exact F.
+  - rewrite unshadow_cas in E. destruct unshadow_acc as [[bound_or_used_o o'] |] eqn:E2 in E. 2: { discriminate E. }
+    specialize (IHt2 _ _ _ _ E2). destruct Rename.pattern eqn:ER in E. 2: { discriminate E. }
+    apply (Rename.pattern_iff $ NewNames.one_to_one_generate _ _) in ER.
+    destruct unshadow_acc as [[bound_or_used_b b'] |] eqn:E1 in E; invert E.
+    specialize (IHt1 _ _ _ _ E1). invert U. 2: { apply IHt2. exact used_in_another_case. }
+    specialize (IHt1 _ used_in_body) as [z F]. apply Map.bulk_overwrite_bulk_overwrite in F as [F | [N F]]. 2: { exists z. exact F. }
+    assert (I : Map.In (BoundIn.pattern pattern) z). { eapply NewNames.in_generate. exists x. exact F. }
+    contradiction not_shadowed. apply (Rename.bound_in_pattern ER). exists z.
+    split. { apply BoundIn.pattern_iff. eapply NewNames.in_generate. exists x. exact F. } exact F.
+Qed.
+
+(* Can't rewrite this in situ below. I'm guessing it has something to do with universes. *)
+Lemma what_the_fuck_is_wrong_with_coq_here
+  {k T m} (N : Map.find m k = None)
+  {v : T} (F : Map.find m k = Some v)
+  : False.
+Proof. rewrite N in F. discriminate F. Qed.
+
+Lemma or_same P
+  : (P \/ P) <-> P.
+Proof. split. { intros [p | p]; exact p. } intro p. left. exact p. Qed.
+
+Lemma wf_spec_acc {acc} (O2O : Map.OneToOne acc)
+  {cant_bind} (cant_bind_range : forall y (IR : Map.InRange acc y), Map.In cant_bind y)
+  {t} (FV : forall x (U : UsedIn.Term t x), Map.In acc x)
+  : Reflect.Option (fun '(_, t') =>
+      forall ctx (AU : forall x (U : UsedIn.Term t' x), Map.In ctx x),
+      WellFormedInAcc cant_bind ctx t'
+    ) $ unshadow_acc acc cant_bind t.
+Proof.
+  generalize dependent cant_bind. generalize dependent acc. induction t; intros.
+  - cbn. constructor. constructor.
+  - cbn. destruct Map.find eqn:Ef; constructor. { constructor. apply AU. constructor. }
+    intros [cant_bind' t'] WF. specialize (FV _ $ UsedIn.Var _ _) as [v F].
+    apply Map.find_iff in F. Fail rewrite Ef in F. Fail rewrite F in Ef.
+    eapply what_the_fuck_is_wrong_with_coq_here. { exact Ef. } exact F.
+  - simpl unshadow_acc.
+    eassert (FVf : _); [| specialize (IHt1 acc O2O FVf cant_bind cant_bind_range)]. {
+      intros. apply FV. apply UsedIn.ApF. exact U. }
+    destruct unshadow_acc as [[bound_or_used_f f'] |] eqn:Ef in IHt1; invert IHt1; rewrite Ef. 2: {
+      constructor. contradiction (N (Map.empty, Term.Ctr $ Constructor.Builtin Constructor.Error)). intros. constructor. }
+    rename Y into WFf. eassert (FVa : _); [| specialize (IHt2 acc O2O FVa)]. {
+      intros. apply FV. apply UsedIn.ApA. exact U. }
+    eassert (cant_bind_range_a : _); [| specialize (IHt2 bound_or_used_f cant_bind_range_a)]. {
+      intros. apply (bound_or_used Ef). right. right. apply cant_bind_range. exact IR. }
+    destruct unshadow_acc as [[bound_or_used_a a'] |] eqn:Ea in IHt2; invert IHt2; rewrite Ea; constructor. 2: {
+      contradiction (N (Map.empty, Term.Ctr $ Constructor.Builtin Constructor.Error)). intros. constructor. }
+    rename Y into WFa. intros. econstructor.
+    + intro x. rewrite (Map.in_overriding_union cant_bind). rewrite Map.in_overriding_union.
+      rewrite <- (BoundIn.term_iff _ _). rewrite <- (UsedIn.term_iff _ _). reflexivity.
+    + intro x. rewrite (Map.in_overriding_union cant_bind). rewrite Map.in_overriding_union.
+      rewrite <- (BoundIn.term_iff _ _). rewrite <- (UsedIn.term_iff _ _). reflexivity.
+    + eapply cant_bind_union. { eapply WFf. intros. apply AU. apply UsedIn.ApF. exact U. } { apply Map.union_set. }
+      intros. apply Map.in_overriding_union in I as [I | I].
+      * apply BoundIn.term_iff in I. eapply (disjoint_bound Ea). 2: { exact I. } apply (bound_or_used Ef). left. exact B.
+      * apply UsedIn.term_iff in I. eapply (disjoint_used Ea) in I as [w F]. 2: { apply (bound_or_used Ef). left. exact B. }
+        eapply (disjoint_bound Ef). 2: { exact B. } apply cant_bind_range. exists w. exact F.
+    + eapply cant_bind_subset. { eapply WFa. intros. apply AU. apply UsedIn.ApA. exact U. }
+      intros x [] I. repeat rewrite Map.find_tt in *. apply (bound_or_used Ef).
+      apply Map.in_overriding_union in I as [I | I]. { right. right. exact I. }
+      apply Map.in_overriding_union in I as [I | I]; [| right]; left; [apply BoundIn.term_iff | apply UsedIn.term_iff]; exact I.
+    + intros. eapply (disjoint_bound Ea). 2: { exact Ba. } apply (bound_or_used Ef). left. exact Bf.
+  - rewrite unshadow_for. eassert (FVt : _); [| specialize (IHt1 acc O2O FVt)]. { intros. apply FV. apply UsedIn.FoT. exact U. }
+    specialize (IHt1 $ Map.set_add (NewNames.new_name cant_bind variable) cant_bind).
+    eassert (cant_bind_range_t : _); [| specialize (IHt1 cant_bind_range_t)]. {
+      intros y IR. apply Map.in_overriding_add. right. apply cant_bind_range. exact IR. }
+    destruct unshadow_acc as [[bound_or_used_t t'] |] eqn:Et in IHt1; invert IHt1; rewrite Et. rename Y into WFt. 2: {
+      constructor. contradiction (N (Map.empty, Term.Ctr $ Constructor.Builtin Constructor.Error)). intros. constructor. }
+    eassert (O2O' : _); [| specialize (IHt2 (Map.overwrite variable (NewNames.new_name cant_bind variable) acc) O2O')]. {
+      unfold Map.OneToOne. intros. apply Map.overwrite_if_present_overwrite in F1 as [[-> ->] | [N1 F1]];
+      apply Map.overwrite_if_present_overwrite in F2 as [[-> E2] | [N2 F2]]; subst. { reflexivity. }
+      * edestruct (@NewNames.not_in_new_name cant_bind variable) as []. apply cant_bind_range. exists k2. exact F2.
+      * edestruct (@NewNames.not_in_new_name cant_bind variable) as []. apply cant_bind_range. exists k1. exact F1.
+      * eapply O2O. { exact F1. } exact F2. }
+    eassert (FVb : _); [| specialize (IHt2 FVb)]. {
+      intros. apply Map.in_overriding_add. destruct (String.eqb_spec x variable); [left | right]. { exact e. }
+      apply FV. apply UsedIn.FoB. { exact n. } exact U. }
+    eassert (cant_bind_range_b : _); [| specialize (IHt2 bound_or_used_t cant_bind_range_b)]. {
+      intros y [x F]. apply (bound_or_used Et). right. right. apply Map.in_overriding_add.
+      apply Map.overwrite_if_present_overwrite in F as [[-> ->] | [N F]]; [left | right]. { reflexivity. }
+      apply cant_bind_range. exists x. exact F. }
+    destruct unshadow_acc as [[bound_or_used_b b'] |] eqn:Eb in IHt2; invert IHt2; rewrite Eb; constructor. 2: {
+      contradiction (N (Map.empty, Term.Ctr $ Constructor.Builtin Constructor.Error)). intros. constructor. }
+    rename Y into WFb. intros. econstructor.
+    + apply NewNames.not_in_new_name.
+    + intro B. eapply (disjoint_bound Et). 2: { exact B. } apply Map.in_overriding_add. left. reflexivity.
+    + intro B. eapply (disjoint_bound Eb). 2: { exact B. }
+      apply (bound_or_used Et). right. right. apply Map.in_overriding_add. left. reflexivity.
+    + intro U. eapply disjoint_used in U as [k F]. 2: { exact Et. } 2: { apply Map.in_overriding_add. left. reflexivity. }
+      eapply NewNames.not_in_new_name. apply cant_bind_range. exists k. exact F.
+    + intro x. rewrite (Map.in_overriding_union cant_bind). rewrite Map.in_overriding_union.
+      rewrite <- (BoundIn.term_iff _ _). rewrite <- (UsedIn.term_iff _ _). reflexivity.
+    + apply Map.add_set.
+    + intro x. rewrite (Map.in_overriding_union cant_bind). rewrite Map.in_overriding_union.
+      rewrite <- (BoundIn.term_iff _ _). rewrite <- (UsedIn.term_iff _ _). reflexivity.
+    + apply Map.add_set.
+    + apply Map.add_set.
+    + eapply cant_bind_union. { eapply WFt. intros. apply AU. apply UsedIn.FoT. exact U. } {
+        intros x []. do 2 erewrite (Map.add_set _) at 1. rewrite or_assoc. erewrite <- (Map.union_set _ _ _). reflexivity. }
+      intros. apply Map.in_overriding_union in I as [I | I]. {
+        apply BoundIn.term_iff in I. eapply (disjoint_bound Eb). 2: { exact I. } apply (bound_or_used Et). left. exact B. }
+      apply UsedIn.term_iff in I. eapply (disjoint_used Eb) in I as [z F]. 2: { apply (bound_or_used Et). left. exact B. }
+      eapply (disjoint_bound Et). 2: { exact B. } apply Map.in_overriding_add.
+      apply Map.overwrite_if_present_overwrite in F as [[-> ->] | [N F]]; [left | right]. { reflexivity. }
+      apply cant_bind_range. exists z. exact F.
+    + eapply cant_bind_subset. { apply WFb. intros. apply Map.in_overriding_add.
+        destruct (String.eqb_spec x $ NewNames.new_name cant_bind variable); [left | right]. { exact e. }
+        apply AU. apply UsedIn.FoB. { exact n. } exact U. }
+      intros x [] I. repeat rewrite Map.find_tt in *. apply (bound_or_used Et). unfold Map.set_add. rewrite Map.in_overriding_add.
+      apply Map.in_overriding_add in I as [-> | I]. { right. right. left. reflexivity. }
+      apply Map.in_overriding_union in I as [I | I]. { right. right. right. exact I. }
+      apply Map.in_overriding_union in I as [I | I]; [| right]; left; [apply BoundIn.term_iff | apply UsedIn.term_iff]; exact I.
+    + intros. eapply (disjoint_bound Eb). 2: { exact Bb. } apply (bound_or_used Et). left. exact Bt.
+  - rewrite unshadow_cas. eassert (FVo : _); [| specialize (IHt2 acc O2O FVo)]. { intros. apply FV. apply UsedIn.CaO. exact U. }
+    specialize (IHt2 $ Map.set_union (Map.range $ NewNames.generate cant_bind $ BoundIn.pattern pattern) cant_bind).
+    eassert (cant_bind_range_o : _); [| specialize (IHt2 cant_bind_range_o)]. {
+      intros y IR. apply Map.in_overriding_union. right. apply cant_bind_range. exact IR. }
+    destruct unshadow_acc as [[bound_or_used_o o'] |] eqn:Eo in IHt2; invert IHt2; rewrite Eo. rename Y into WFo. 2: {
+      constructor. contradiction (N (Map.empty, Term.Ctr $ Constructor.Builtin Constructor.Error)). intros. constructor. }
+    destruct (Rename.pattern_spec (NewNames.one_to_one_generate cant_bind $ BoundIn.pattern pattern) pattern). 2: {
+      constructor. intros [bound_or_used' t'] WF. Abort.
+(* TODO: some measure of equivalence up to renaming, but that's kind of tautological here, since we're *defining* renaming.
+ * the problem above is that we're not constraining the result to something *like* the original `t`, so
+ * when the reflectee is `None`, we have to prove that no term *at all* *ever* satisfies this pretty easily satisfiable Prop.
+ * so, if we want to be extra sure, we should constrain the reflected property s.t. `t` and `t'` are equivalent *)
+
+Lemma on_the_tin_acc
+  {acc cant_bind t bound_or_used' t'} (E : unshadow_acc acc cant_bind t = Some (bound_or_used', t'))
+  (cant_bind_range : forall y (IR : Map.InRange acc y), Map.In cant_bind y)
+  {ctx} (AU : forall x (U : UsedIn.Term t' x), Map.In ctx x)
+  : WellFormedInAcc cant_bind ctx t'.
+Proof.
+  generalize dependent ctx. generalize dependent t'. generalize dependent bound_or_used'.
+  generalize dependent cant_bind. generalize dependent acc. { induction t; intros.
+  - invert E. constructor.
+  - cbn in E. destruct (Map.find_spec acc name); invert E. constructor. apply AU. constructor.
+  - cbn in E. destruct unshadow_acc as [[bound_or_used_f f'] |] eqn:Ef in E at 1. 2: { discriminate E. }
+    destruct unshadow_acc as [[bound_or_used_a a'] |] eqn:Ea in E at 1; invert E. econstructor.
+    + intro. rewrite (Map.in_overriding_union cant_bind). rewrite Map.in_overriding_union.
+      rewrite <- (BoundIn.term_iff _ _). rewrite <- (UsedIn.term_iff _ _). reflexivity.
+    + intro. rewrite (Map.in_overriding_union cant_bind). rewrite Map.in_overriding_union.
+      rewrite <- (BoundIn.term_iff _ _). rewrite <- (UsedIn.term_iff _ _). reflexivity.
+    + eapply cant_bind_union. { eapply (IHt1 _ _ _ _ _ Ef). intros. apply AU. apply UsedIn.ApF. exact U. } { apply Map.union_set. }
+      intros. apply Map.in_overriding_union in I as [I | I]; [apply BoundIn.term_iff in I | apply UsedIn.term_iff in I].
+      * eapply (disjoint_bound Ea). 2: { exact I. } apply (bound_or_used Ef). left. exact B.
+      * eapply (disjoint_used Ea) in I as [z F]. 2: { apply (bound_or_used Ef). left. exact B. }
+        eapply (disjoint_bound Ef). 2: { exact B. } apply cant_bind_range. exists z. exact F.
+    + eapply cant_bind_subset. { eapply (IHt2 _ _ _ _ _ Ea). intros. apply AU. apply UsedIn.ApA. exact U. }
+      intros x [] F. apply Map.find_tt. apply (bound_or_used Ef).
+      apply Map.union_set in F as [F | F]. { right. right. exists tt. exact F. }
+      apply Map.union_set in F as [F | F]; [| right]; left; [apply BoundIn.term_iff | apply UsedIn.term_iff]; exists tt; exact F.
+    + intros. eapply (disjoint_bound Ea). 2: { exact Ba. } apply (bound_or_used Ef). left. exact Bf.
+  - rewrite unshadow_for in E. rename t' into term'.
+    destruct unshadow_acc as [[bound_or_used_t t'] |] eqn:Et in E at 1. 2: { discriminate E. }
+    destruct unshadow_acc as [[bound_or_used_b b'] |] eqn:Eb in E at 1; invert E. econstructor.
+    + apply NewNames.not_in_new_name.
+    + intro B. eapply (disjoint_bound Et). 2: { exact B. } apply Map.in_overriding_add. left. reflexivity.
+    + intro B. eapply (disjoint_bound Eb). 2: { exact B. }
+      apply (bound_or_used Et). right. right. apply Map.in_overriding_add. left. reflexivity.
+    + intro U. eapply (disjoint_used Et) in U as [x F]. 2: { apply Map.in_overriding_add. left. reflexivity. }
+      eapply NewNames.not_in_new_name. apply cant_bind_range. exists x. exact F.
+    + intro. rewrite (Map.in_overriding_union cant_bind). rewrite Map.in_overriding_union.
+      rewrite <- (BoundIn.term_iff _ _). rewrite <- (UsedIn.term_iff _ _). reflexivity.
+    + apply Map.add_set.
+    + intro. rewrite (Map.in_overriding_union cant_bind). rewrite Map.in_overriding_union.
+      rewrite <- (BoundIn.term_iff _ _). rewrite <- (UsedIn.term_iff _ _). reflexivity.
+    + apply Map.add_set.
+    + apply Map.add_set.
+    + eapply cant_bind_union. { eapply (IHt1 _ _ _ _ _ Et). intros. apply AU. apply UsedIn.FoT. exact U. } {
+        intros x []. fold (Map.set_add $ NewNames.new_name cant_bind variable). repeat rewrite (Map.add_set _) at 1.
+        rewrite or_assoc. rewrite <- (Map.union_set _ _ _). reflexivity. }
+      intros. apply Map.in_overriding_union in I as [I | I]; [apply BoundIn.term_iff in I | apply UsedIn.term_iff in I].
+      * eapply (disjoint_bound Eb). 2: { exact I. } apply (bound_or_used Et). left. exact B.
+      * eapply (disjoint_used Eb) in I as [z F]. 2: { apply (bound_or_used Et). left. exact B. }
+        apply Map.overwrite_if_present_overwrite in F as [[-> ->] | [N F]]. {
+          eapply (disjoint_bound Et). 2: { exact B. } apply Map.in_overriding_add. left. reflexivity. }
+        eapply (disjoint_bound Et). 2: { exact B. } apply Map.in_overriding_add. right. apply cant_bind_range. exists z. exact F.
+    + eapply cant_bind_subset. { eapply (IHt2 _ _ _ _ _ Eb). intros. apply Map.in_overriding_add.
+        destruct (String.eqb_spec x $ NewNames.new_name cant_bind variable); [left | right]. { exact e. }
+        apply AU. apply UsedIn.FoB. { exact n. } exact U. }
+      intros x [] F. apply Map.find_tt. apply (bound_or_used Et). unfold Map.set_add. rewrite Map.in_overriding_add.
+      apply Map.add_set in F as [[-> _] | F]. { right. right. left. reflexivity. }
+      apply Map.union_set in F as [F | F]. { right. right. right. exists tt. exact F. }
+      apply Map.union_set in F as [F | F]; [| right]; left; [apply BoundIn.term_iff | apply UsedIn.term_iff]; exists tt; exact F.
+    + intros. eapply (disjoint_bound Eb). 2: { exact Bb. } apply (bound_or_used Et). left. exact Bt.
+  - rewrite unshadow_cas in E. destruct unshadow_acc as [[bound_or_used_o o'] |] eqn:Eo in E at 1. 2: { discriminate E. }
+    destruct (Rename.pattern_spec (NewNames.one_to_one_generate cant_bind $ BoundIn.pattern pattern) pattern). 2: { discriminate E. }
+    rename Y into R. rename x into p. destruct unshadow_acc as [[bound_or_used_b b'] |] eqn:Eb in E at 1; invert E. econstructor.
+    + invert R; constructor. invert rename_move_or_reference; constructor; eapply Rename.wf_strict; exact rename_strict.
+    + intro y; intros. apply (Rename.bound_in_pattern R) in Bp as [x [Bp F]].
+      eapply NewNames.not_in_generate. { exact I. } exists x. exact F.
+    + intro y; intros. apply (Rename.bound_in_pattern R) in Bp as [x [Bp F]].
+      eapply (disjoint_bound Eo). 2: { exact B. } apply Map.in_overriding_union. left. apply Map.in_space_range. exists x. exact F.
+    + intro y; intros. apply (Rename.bound_in_pattern R) in Bp as [x [Bp F]].
+      eapply (disjoint_bound Eb). 2: { exact B. } apply (bound_or_used Eo). right. right.
+      apply Map.in_overriding_union. left. apply Map.in_space_range. exists x. exact F.
+    + intro v; intros. apply (Rename.bound_in_pattern R) in Bp as [x [Bp F]].
+      eapply (disjoint_used Eo) in U as [k F']. {
+        eapply NewNames.not_in_generate. 2: { exists x. exact F. } apply cant_bind_range. exists k. exact F'. }
+      apply Map.in_overriding_union. left. apply Map.in_space_range. exists x. exact F.
+    + intro. rewrite (Map.in_overriding_union cant_bind). rewrite Map.in_overriding_union.
+      rewrite <- (BoundIn.term_iff _ _). rewrite <- (UsedIn.term_iff _ _). reflexivity.
+    + intro. erewrite Map.in_overriding_union at 1. rewrite <- (BoundIn.pattern_iff _ _). reflexivity.
+    + intro. rewrite (Map.in_overriding_union cant_bind). rewrite Map.in_overriding_union.
+      rewrite <- (BoundIn.term_iff _ _). rewrite <- (UsedIn.term_iff _ _). reflexivity.
+    + intro. erewrite Map.in_overriding_union at 1. rewrite <- (BoundIn.pattern_iff _ _). reflexivity.
+    + intro. erewrite Map.in_overriding_union at 1. rewrite <- (BoundIn.pattern_iff _ _). reflexivity.
+    + eapply cant_bind_union. { eapply (IHt2 _ _ _ _ _ Eo). intros. apply AU. apply UsedIn.CaO. exact U. } {
+        intros x []. repeat fold Map.set_union. do 4 erewrite (Map.union_set _ _ _) at 1.
+        erewrite Map.find_range at 1. rewrite or_assoc. repeat rewrite Map.find_tt at 1. rewrite (BoundIn.pattern_iff _ _) at 1.
+        rewrite (Rename.bound_in_pattern R). split.
+        * intros [[z [B F]] | I]; [left | right]. { exists z. exact F. } destruct I as [I | I]; [left | right]. { exact I. }
+          rewrite Map.in_overriding_union. exact I.
+        * intros [[z F] | I]; [left | right]. { exists z. split. 2: { exact F. }
+            apply BoundIn.pattern_iff. eapply NewNames.in_generate. exists x. exact F. }
+          destruct I as [I | I]; [left | right]. { exact I. } apply Map.in_overriding_union. exact I. }
+      intros. apply Map.in_overriding_union in I as [I | I]; [apply BoundIn.term_iff in I | apply UsedIn.term_iff in I].
+      * eapply (disjoint_bound Eb). 2: { exact I. } apply (bound_or_used Eo). left. exact B.
+      * eapply (disjoint_used Eb) in I as [z F]. 2: { apply (bound_or_used Eo). left. exact B. }
+        apply Map.bulk_overwrite_bulk_overwrite in F as [F | [N F]]. { eapply (disjoint_bound Eo). 2: { exact B. }
+          apply Map.in_overriding_union. left. apply Map.in_space_range. exists z. exact F. }
+        eapply (disjoint_bound Eo). 2: { exact B. } apply Map.in_overriding_union. right. apply cant_bind_range. exists z. exact F.
+    + eapply cant_bind_subset. { eapply (IHt1 _ _ _ _ _ Eb). intros. apply Map.in_overriding_union.
+        destruct (BoundIn.pattern_spec p x); [left | right]. { apply BoundIn.pattern_iff. exact Y. }
+        apply AU. apply UsedIn.CaB. { exact N. } exact U. }
+      intros x [] F. rewrite Map.find_tt in *. apply (bound_or_used Eo). rewrite Map.in_overriding_union. rewrite Map.in_space_range.
+      apply Map.in_overriding_union in F as [I | I]. { apply BoundIn.pattern_iff in I. right. right. left.
+        apply (Rename.bound_in_pattern R) in I as [z [B F]]. exists z. exact F. }
+      apply Map.in_overriding_union in I as [I | I]. { right. right. right. exact I. }
+      apply Map.in_overriding_union in I as [I | I]; [| right]; left; [apply BoundIn.term_iff | apply UsedIn.term_iff]; exact I.
+    + intros. eapply (disjoint_bound Eb). 2: { exact Bb. } apply (bound_or_used Eo). left. exact Bo. }
+  Unshelve.
+  - exact cant_bind_range.
+  - intros. apply (bound_or_used Ef). right. right. apply cant_bind_range. exact IR.
+  - intros. apply Map.in_overriding_add. right. apply cant_bind_range. exact IR.
+  - intros y [x F]. apply (bound_or_used Et). right. right. apply Map.in_overriding_add.
+    apply Map.overwrite_if_present_overwrite in F as [[-> ->] | [N F]]; [left | right]. { reflexivity. }
+    apply cant_bind_range. exists x. exact F.
+  - intros. apply Map.in_overriding_union. right. apply cant_bind_range. exact IR.
+  - intros y [x F]. apply (bound_or_used Eo). right. right. apply Map.in_overriding_union. rewrite Map.in_space_range.
+    apply Map.bulk_overwrite_bulk_overwrite in F as [F | [N F]]; [left | right]. { exists x. exact F. }
+    apply cant_bind_range. exists x. exact F.
+Qed.
+
+Lemma on_the_tin_bindings
+  {cant_bind t bound_or_used' t'} (E : unshadow_reserve_bindings cant_bind t = Some (bound_or_used', t'))
+  {ctx : Map.set} (AU : forall x (U : UsedIn.Term t' x), Map.In ctx x)
+  : WellFormedInAcc (Map.set_union cant_bind $ UsedIn.term t) ctx t'.
+Proof.
+  unfold unshadow_reserve_bindings in E. eapply on_the_tin_acc. { exact E. } 2: { exact AU. }
+  intros. apply Map.in_overriding_union. right. destruct IR as [x F]. apply Map.to_self_to_self in F as [I ->]. exact I.
+Qed.
+
+Lemma on_the_tin_reserve
+  {cant_bind t t'} (E : unshadow_reserve cant_bind t = Some t')
+  {ctx : Map.set} (AU : forall x (U : UsedIn.Term t' x), Map.In ctx x)
+  : WellFormedInAcc (Map.set_union cant_bind $ UsedIn.term t) ctx t'.
+Proof.
+  unfold unshadow_reserve in E. destruct unshadow_reserve_bindings as [[] |] eqn:E'; invert E.
+  eapply on_the_tin_bindings. { exact E'. } exact AU.
+Qed.
+
+Lemma on_the_tin
+  {t t'} (E : unshadow t = Some t')
+  {ctx : Map.set} (AU : forall x (U : UsedIn.Term t' x), Map.In ctx x)
+  : WellFormedInAcc (UsedIn.term t) ctx t'.
+Proof.
+  eapply on_the_tin_reserve in E. 2 :{ exact AU. } eapply cant_bind_subset. { exact E. }
+  intros x [] F. apply Map.union_set. right. exact F.
+Qed.
+
+
+
+Definition UniqueBindings context :=
+  forall k v1 (F1 : Map.Find context k v1) x (B1 : BoundIn.Term v1 x) v2 (F2 : Map.Find context k v2) (B2 : BoundIn.Term v2 x),
+  v1 = v2.
+Arguments UniqueBindings context/.
+
+Definition WellFormedContextAcc context domain : Prop :=
+  UniqueBindings context /\
+  Map.ForAll (fun _ => WellFormedInAcc domain domain) context.
+Arguments WellFormedContextAcc context domain/.
+
+Definition WellFormedContext context : Prop :=
+  forall domain (D : Map.Domain context domain), WellFormedContextAcc context domain.
 Arguments WellFormedContext context/.
 
 Definition WellFormedInContext context term : Prop :=
-  WellFormedContext context /\ (* Yes, this `domain` is redundant, but efficiency doesn't matter, and this can be `destruct`ed *)
+  WellFormedContext context /\
   forall domain (D : Map.Domain context domain),
-  Unshadow.WellFormedIn domain term.
+  forall cant_bind (R : Map.Reflect (fun x => Map.In domain x \/ exists v, (Map.InRange context v /\ BoundIn.Term v x)) cant_bind),
+  WellFormedInAcc cant_bind domain term.
 Arguments WellFormedInContext context term/.
 
 
 
 Definition unshadow_context_each k v (acc : option (Map.set * Context.context)) : option (Map.set * Context.context) :=
-  match acc with | None => None | Some (cant_bind, acc) =>
+  match acc with | None => None | Some (cant_bind, so_far) =>
     match unshadow_reserve_bindings cant_bind v with None => None | Some (bindings, v') =>
-      Some (Map.set_union bindings cant_bind, Map.overriding_add k v' acc)
+      Some (Map.set_union bindings cant_bind, Map.overriding_add k v' so_far)
     end
   end.
 Arguments unshadow_context_each k v acc/.
@@ -1356,51 +1704,381 @@ Definition unshadow_context_acc :=
   Map.fold unshadow_context_each.
 Arguments unshadow_context_acc/ acc context : rename.
 
+Definition unshadow_context_reserve_bindings cant_bind :=
+  unshadow_context_acc (Some (cant_bind, Map.empty)).
+Arguments unshadow_context_reserve_bindings cant_bind/ context : rename.
+
+Definition unshadow_context_reserve cant_bind context :=
+  option_map snd $ unshadow_context_reserve_bindings cant_bind context.
+Arguments unshadow_context_reserve cant_bind context/ : rename.
+
 Definition unshadow_context (context : Context.context) :=
-  unshadow_context_acc (Some (Map.domain context, Map.empty)) context.
+  unshadow_context_reserve (Map.domain context) context.
 Arguments unshadow_context context/.
 
 Lemma unfold_right {X Y} (f : X -> Y -> Y) init head tail
   : List.fold_right f init (head :: tail) = f head $ List.fold_right f init tail.
 Proof. reflexivity. Qed.
 
-Lemma unshadow_context_spec_acc
+Lemma unshadow_context_prev_spec_acc
   {acc} (Ra : Reflect.Option (fun '(cant_bind', ctx) => Map.ForAll (fun _ => WellFormed.AllPatternsIn) ctx) acc) ctx
-  : Reflect.Option (fun '(cant_bind', ctx') =>
-      Map.ForAll (fun _ => WellFormed.AllPatternsIn) ctx /\
-      Map.ForAll (fun _ => WellFormed.AllPatternsIn) ctx'
-    ) $ unshadow_context_acc acc ctx.
+  : Reflect.Option (fun '(cant_bind', ctx') => Map.ForAll (fun _ => WellFormed.AllPatternsIn) ctx) $ unshadow_context_acc acc ctx.
 Proof.
   unfold unshadow_context_acc. unfold Map.fold. rewrite MapCore.fold_spec. rewrite <- List.fold_left_rev_right.
-  eapply (@Reflect.option_eq _ $ fun '(cant_bind', ctx') => (forall k v (F
-    : SetoidList.InA MapCore.eq_key_elt (k, v) $ List.rev (MapCore.bindings ctx)), _) /\
-      Map.ForAll (fun _ => WellFormed.AllPatternsIn) ctx'). {
-    intros [cant_bind' ctx']. split; intros [H same]; (split; [| exact same]);
-    intros k v F; apply (H k v); [apply -> SetoidList.InA_rev in F |];
+  eapply (@Reflect.option_eq _ $ fun '(cant_bind', ctx') => forall k v (F
+    : SetoidList.InA MapCore.eq_key_elt (k, v) $ List.rev (MapCore.bindings ctx)), _). {
+    intros [cant_bind' ctx']. split; intros H k v F; apply (H k v); [apply -> SetoidList.InA_rev in F |];
     apply MapCore.bindings_spec1 in F; [| apply SetoidList.InA_rev in F]; exact F. }
   remember (List.rev (MapCore.bindings ctx)) as b eqn:Eb; clear ctx Eb.
   generalize dependent acc. induction b as [| [k v] tail IH]; intros. {
-    cbn. destruct acc as [[bindings acc] |]; cbn in *; invert Ra; constructor. {
-      split; intros k v F. { invert F. } eapply Y. exact F. }
-    intros [cant_bind' ctx'] [C C']. apply (N (cant_bind', ctx')). exact C'. }
+    cbn. destruct Ra as [[bindings acc] |]; constructor. { intros k v F. invert F. }
+    intros [cant_bind' ctx']. specialize (N (cant_bind', Map.empty)) as []. intros k v F. invert F. }
   rewrite unfold_right. simpl fst. simpl snd. unfold unshadow_context_each at 1. specialize (IH acc Ra).
-  destruct IH as [[cant_bind' ctx'] [Y Y'] |]. 2: { constructor. intros [cant_bind' ctx'] [C C'].
-    apply (N (cant_bind', ctx')). split. { intros k' v' F'. eapply C. right. exact F'. } exact C'. }
-  destruct (wf_patterns_spec_bindings cant_bind' v) as [[cant_bind'' ctx''] [Y'' Y'''] |]; constructor. 2: {
-    intros [cant_bind'' ctx''] [C C']. eapply (N (cant_bind'', v)). split; eapply C; left; split; reflexivity. }
-  split; intros k' v' F'. { invert F'. { destruct H0. cbn in *. subst. exact Y''. } eapply Y. exact H0. }
-  apply Map.overwrite_if_present_overwrite in F' as [[-> ->] | [N' F']]. { exact Y'''. } eapply Y'. exact F'.
+  destruct IH as [[cant_bind' ctx'] Y |]. 2: { constructor. intros [cant_bind' ctx'] C.
+    apply (N (cant_bind', ctx')). intros k' v' F'. eapply C. right. exact F'. }
+  destruct (wf_patterns_spec_bindings cant_bind' v) as [[cant_bind'' ctx''] Y' |]; constructor. 2: {
+    intros [cant_bind'' ctx''] C. eapply (N (cant_bind'', v)). split; eapply C; left; split; reflexivity. }
+  intros k' v' F'. invert F'. { destruct H0. cbn in *. subst. apply Y'. } eapply Y. exact H0.
 Qed.
 
-Lemma unshadow_context_spec ctx
-  : Reflect.Option (fun '(cant_bind', ctx') =>
-      Map.ForAll (fun _ => WellFormed.AllPatternsIn) ctx /\
-      Map.ForAll (fun _ => WellFormed.AllPatternsIn) ctx'
-    ) $ unshadow_context ctx.
+Lemma unshadow_context_prev_spec ctx
+  : Reflect.Option (fun _ => Map.ForAll (fun _ => WellFormed.AllPatternsIn) ctx) $ unshadow_context ctx.
 Proof.
-  unfold unshadow_context. eassert (A : _); [|
-    destruct (@unshadow_context_spec_acc (Some (Map.domain ctx, Map.empty)) A ctx) as [[cant_bind' ctx'] [Y Y'] |]].
-  - constructor. intros k v C. invert C.
-  - constructor. split. { exact Y. } exact Y'.
-  - constructor. intros [cant_bind' ctx'] [C C']. apply (N (cant_bind', ctx')). split. { exact C. } exact C'.
+  unfold unshadow_context. unfold unshadow_context_reserve. unfold unshadow_context_reserve_bindings.
+  eassert (A : _); [| destruct (@unshadow_context_prev_spec_acc (Some (Map.domain ctx, Map.empty))
+    A ctx) as [[] |]]; constructor. { intros k v C. invert C. } { exact Y. }
+  intros _ C. apply (N (Map.empty, Map.empty)). exact C.
 Qed.
+
+Lemma used_in_acc {acc cant_bind} (CB : forall x y (F : Map.Find acc x y), Map.In cant_bind y)
+  {t bindings t'} (E : unshadow_acc acc cant_bind t = Some (bindings, t'))
+  {x} (U : UsedIn.Term t x) {y} (F : Map.Find acc x y)
+  : UsedIn.Term t' y.
+Proof.
+  generalize dependent y. generalize dependent x. generalize dependent t'. generalize dependent bindings.
+  generalize dependent cant_bind. generalize dependent acc. induction t; intros.
+  - invert U.
+  - invert U. unfold unshadow_acc in E. destruct Map.find eqn:EF in E; invert E.
+    apply Map.find_iff in EF. destruct (Map.find_det F EF). constructor.
+  - rewrite unshadow_app in E. destruct unshadow_acc as [[bound_or_used_f f'] |] eqn:Ef in E. 2: { discriminate E. }
+    destruct unshadow_acc as [[bound_or_used_a a'] |] eqn:Ea in E; invert E.
+    specialize (IHt1 _ _ CB _ _ Ef). eassert (CBa : _); [| specialize (IHt2 _ _ CBa _ _ Ea)]. {
+      intros k v F'. apply (bound_or_used Ef). right. right. eapply CB. exact F'. }
+    invert U.
+    + apply UsedIn.ApF. eapply IHt1. { exact used_in_function. } exact F.
+    + apply UsedIn.ApA. eapply IHt2. { exact used_in_argument. } exact F.
+  - rewrite unshadow_for in E. rename t' into term'.
+    destruct unshadow_acc as [[bound_or_used_t t'] |] eqn:Et in E. 2: { discriminate E. }
+    destruct unshadow_acc as [[bound_or_used_b b'] |] eqn:Eb in E; invert E.
+    eassert (CBt : _); [| specialize (IHt1 _ _ CBt _ _ Et)]. {
+      intros k v F'. apply Map.in_overriding_add. right. eapply CB. exact F'. }
+    eassert (CBb : _); [| specialize (IHt2 _ _ CBb _ _ Eb)]. {
+      intros k v F'. apply (bound_or_used Et). right. right. apply Map.in_overriding_add.
+      apply Map.overwrite_if_present_overwrite in F' as [[-> ->] | [N' F']]; [left | right]. { reflexivity. }
+      eapply CB. exact F'. }
+    invert U. { apply UsedIn.FoT. eapply IHt1. { exact used_in_type. } exact F. }
+    apply UsedIn.FoB. 2: { eapply IHt2. { exact used_in_body. }
+      apply Map.overwrite_if_present_overwrite. right. split. { exact not_shadowed. } exact F. }
+    intros ->. eapply NewNames.not_in_new_name. eapply CB. exact F.
+  - rewrite unshadow_cas in E.
+    destruct unshadow_acc as [[bound_or_used_o o'] |] eqn:Eo in E. 2: { discriminate E. }
+    destruct (Rename.pattern_spec (NewNames.one_to_one_generate cant_bind $ BoundIn.pattern pattern) pattern). 2: { discriminate E. }
+    destruct unshadow_acc as [[bound_or_used_b b'] |] eqn:Eb in E; invert E.
+    eassert (CBo : _); [| specialize (IHt2 _ _ CBo _ _ Eo)]. {
+      intros k v F'. apply Map.in_overriding_union. right. eapply CB. exact F'. }
+    eassert (CBb : _); [| specialize (IHt1 _ _ CBb _ _ Eb)]. {
+      intros k v F'. apply (bound_or_used Eo). right. right. apply Map.in_overriding_union.
+      apply Map.bulk_overwrite_bulk_overwrite in F' as [F' | [N' F']]; [left | right]. { apply Map.in_space_range. exists k. exact F'. }
+      eapply CB. exact F'. }
+    invert U. 2: { apply UsedIn.CaO. eapply IHt2. { exact used_in_another_case. } exact F. }
+    apply UsedIn.CaB. 2: { eapply IHt1. { exact used_in_body. }
+      apply Map.bulk_overwrite_bulk_overwrite. right. split. 2: { exact F. }
+      intro I. apply NewNames.in_generate in I. apply not_shadowed. apply BoundIn.pattern_iff. exact I. }
+    intro B. apply (Rename.bound_in_pattern Y) in B as [z [B F']].
+    eapply NewNames.not_in_generate. 2: { exists z. exact F'. } eapply CB. exact F.
+Qed.
+
+Lemma used_in_bindings {cant_bind t bindings t'}
+  (E : unshadow_reserve_bindings cant_bind t = Some (bindings, t'))
+  {x} (U : UsedIn.Term t x)
+  : UsedIn.Term t' x.
+Proof.
+  eapply used_in_acc. 2: { exact E. } 2: { exact U. } 2: {
+    apply Map.to_self_to_self. split. { apply UsedIn.term_iff. exact U. } reflexivity. }
+  intros. apply Map.in_overriding_union. apply Map.to_self_to_self in F as [I ->]. right. exact I.
+Qed.
+
+Lemma eq_spec_unit (a b : unit)
+  : Reflect.Bool (a = b) true.
+Proof. destruct a. destruct b. constructor. reflexivity. Qed.
+
+Lemma used_idem_acc {acc t} (no_free_vars : forall x (U : UsedIn.Term t x), Map.In acc x)
+  {cant_bind} (cant_bind_acc : forall x (I : Map.In acc x), Map.In cant_bind x)
+  (cant_bind_range : forall y (IR : Map.InRange acc y), Map.In cant_bind y)
+  (A : forall x (U : UsedIn.Term t x) y (F : Map.Find acc x y), y = x)
+  {bindings t'} (E : unshadow_acc acc cant_bind t = Some (bindings, t')) {x}
+  : UsedIn.Term t' x <-> UsedIn.Term t x.
+Proof.
+  generalize dependent x. generalize dependent t'. generalize dependent bindings.
+  generalize dependent cant_bind. generalize dependent acc. induction t; intros.
+  - cbn in E. invert E. reflexivity.
+  - unfold unshadow_acc in E. destruct Map.find eqn:F in E; invert E.
+    apply Map.find_iff in F. apply A in F as ->. { reflexivity. } constructor.
+  - rewrite unshadow_app in E. destruct unshadow_acc as [[bound_or_used_f f'] |] eqn:Ef in E. 2: { discriminate E. }
+    destruct unshadow_acc as [[bound_or_used_a a'] |] eqn:Ea in E; invert E.
+    eassert (no_free_vars_f : _); [| eassert (Af : _); [|
+      specialize (IHt1 _ no_free_vars_f Af _ cant_bind_acc cant_bind_range _ _ Ef)]]. {
+      intros. apply no_free_vars. apply UsedIn.ApF. exact U. } {
+      intros. apply A. 2: { exact F. } apply UsedIn.ApF. exact U. }
+    eassert (no_free_vars_a : _); [| eassert (Aa : _); [| eassert (cant_bind_acc' : _); [| eassert (cant_bind_range' : _); [|
+      specialize (IHt2 _ no_free_vars_a Aa _ cant_bind_acc' cant_bind_range' _ _ Ea)]]]]. {
+      intros. apply no_free_vars. apply UsedIn.ApA. exact U. } {
+      intros. apply A. 2: { exact F. } apply UsedIn.ApA. exact U. } {
+      intros. apply (bound_or_used Ef). right. right. apply cant_bind_acc. exact I. } {
+      intros. apply (bound_or_used Ef). right. right. apply cant_bind_range. exact IR. }
+    split; intro U; (invert U; [apply UsedIn.ApF | apply UsedIn.ApA]; [apply IHt1 | apply IHt2]); assumption.
+  - rewrite unshadow_for in E. rename t' into term'.
+    destruct unshadow_acc as [[bound_or_used_t t'] |] eqn:Et in E. 2: { discriminate E. }
+    destruct unshadow_acc as [[bound_or_used_b b'] |] eqn:Eb in E; invert E.
+    eassert (no_free_vars_t : _); [| eassert (At : _); [| eassert (cant_bind_acc_t : _); [| eassert (cant_bind_range_t : _); [|
+      specialize (IHt1 _ no_free_vars_t At _ cant_bind_acc_t cant_bind_range_t _ _ Et)]]]]. {
+      intros. apply no_free_vars. apply UsedIn.FoT. exact U. } {
+      intros. apply A. 2: { exact F. } apply UsedIn.FoT. exact U. } {
+      intros. apply Map.in_overriding_add. right. apply cant_bind_acc. exact I. } {
+      intros. apply Map.in_overriding_add. right. apply cant_bind_range. exact IR. }
+    eassert (no_free_vars_b : forall x (N : x <> variable) (U : UsedIn.Term t2 x), Map.In acc x). {
+      intros. eapply no_free_vars. apply UsedIn.FoB. { exact N. } exact U. }
+    eassert (cant_bind_range_b : forall y, Map.InRange (Map.overwrite variable (NewNames.new_name cant_bind variable) acc) y ->
+      Map.In bound_or_used_t y). { intros y [z F]. apply (bound_or_used Et). right. right. apply Map.in_overriding_add.
+      apply Map.find_overriding_add in F as [[-> ->] | [N F]]; [left | right]. { reflexivity. }
+      apply cant_bind_range. exists z. exact F. }
+    split.
+    + intro U. invert U. { apply UsedIn.FoT. apply IHt1. exact used_in_type. }
+      apply (used_before cant_bind_range_b Eb) in used_in_body as [z [F U]].
+      apply Map.overwrite_if_present_overwrite in F as [[-> ->] | [N F]]. { contradiction not_shadowed. reflexivity. }
+      apply A in F as ->; (apply UsedIn.FoB; [exact N | exact U]).
+    + intro U. invert U. { apply UsedIn.FoT. apply IHt1. exact used_in_type. }
+      apply UsedIn.FoB. 2: { apply (used_before cant_bind_range_b Eb). exists x. split. 2: { exact used_in_body. }
+        apply Map.find_overriding_add. right. split. { exact not_shadowed. }
+        eassert (I : Map.In _ _). 2: { destruct I as [y F]. assert (y = x). 2: { subst. exact F. }
+          apply A. 2: { exact F. } apply UsedIn.FoB. { exact not_shadowed. } exact used_in_body. }
+        apply no_free_vars_b. { exact not_shadowed. } apply used_in_body. }
+      intros ->. eapply NewNames.not_in_new_name. apply cant_bind_acc. apply no_free_vars.
+      apply UsedIn.FoB. { exact not_shadowed. } exact used_in_body.
+  - rewrite unshadow_cas in E.
+    destruct unshadow_acc as [[bound_or_used_o o'] |] eqn:Eo in E. 2: { discriminate E. }
+    destruct (Rename.pattern_spec (NewNames.one_to_one_generate cant_bind $ BoundIn.pattern pattern) pattern). 2: { discriminate E. }
+    destruct unshadow_acc as [[bound_or_used_b b'] |] eqn:Eb in E; invert E.
+    eassert (no_free_vars_o : _); [| eassert (Ao : _); [| eassert (cant_bind_acc_o : _); [| eassert (cant_bind_range_o : _); [|
+      specialize (IHt2 _ no_free_vars_o Ao _ cant_bind_acc_o cant_bind_range_o _ _ Eo)]]]]. {
+      intros. apply no_free_vars. apply UsedIn.CaO. exact U. } {
+      intros. apply A. 2: { exact F. } apply UsedIn.CaO. exact U. } {
+      intros. apply Map.in_overriding_union. right. apply cant_bind_acc. exact I. } {
+      intros. apply Map.in_overriding_union. right. apply cant_bind_range. exact IR. }
+    eassert (no_free_vars_b : forall x (N : ~BoundIn.Pattern pattern x) (U : UsedIn.Term t1 x), Map.In acc x). {
+      intros. eapply no_free_vars. apply UsedIn.CaB. { exact N. } exact U. }
+    eassert (cant_bind_range_b : forall y (IR : Map.InRange (Map.bulk_overwrite (NewNames.generate cant_bind $ BoundIn.pattern pattern)
+      acc) y), Map.In bound_or_used_o y). { intros y [z F]. apply (bound_or_used Eo). right. right. apply Map.in_overriding_union.
+      apply Map.bulk_overwrite_bulk_overwrite in F as [F | [N F]]; [left | right]. { apply Map.in_space_range. exists z. exact F. }
+      apply cant_bind_range. exists z. exact F. }
+    split.
+    + intro U. invert U. 2: { apply UsedIn.CaO. apply IHt2. exact used_in_another_case. }
+      apply (used_before cant_bind_range_b Eb) in used_in_body as [z [F U]].
+      apply Map.bulk_overwrite_bulk_overwrite in F as [F | [N F]]. {
+        contradiction not_shadowed. apply (Rename.bound_in_pattern Y). exists z. split. 2: { exact F. }
+        apply BoundIn.pattern_iff. eapply NewNames.in_generate. exists x. exact F. }
+      apply A in F as ->; (apply UsedIn.CaB; [| exact U]); intro B; apply N;
+      apply NewNames.in_generate; apply BoundIn.pattern_iff; exact B.
+    + intro U. invert U. 2: { apply UsedIn.CaO. apply IHt2. exact used_in_another_case. }
+      apply UsedIn.CaB. 2: { apply (used_before cant_bind_range_b Eb). exists x. split. 2: { exact used_in_body. }
+        apply Map.bulk_overwrite_bulk_overwrite. right. split. {
+          intro I. apply not_shadowed. apply BoundIn.pattern_iff. eapply NewNames.in_generate. exact I. }
+        eassert (I : Map.In _ _). 2: { destruct I as [y F]. assert (y = x). 2: { subst. exact F. }
+          apply A. 2: { exact F. } apply UsedIn.CaB. { exact not_shadowed. } exact used_in_body. }
+        apply no_free_vars_b. { exact not_shadowed. } apply used_in_body. }
+      intro B. apply (Rename.bound_in_pattern Y) in B as [x' [B F]]. eapply NewNames.not_in_generate. 2: { exists x'. exact F. }
+      apply cant_bind_acc. apply no_free_vars. apply UsedIn.CaB. { exact not_shadowed. } exact used_in_body.
+Qed.
+
+Lemma used_idem {cant_bind t bindings t'} (E : unshadow_reserve_bindings cant_bind t = Some (bindings, t')) {x}
+  : UsedIn.Term t' x <-> UsedIn.Term t x.
+Proof.
+  eapply used_idem_acc; try exact E; intros.
+  - apply Map.in_to_self. apply UsedIn.term_iff. exact U.
+  - apply Map.in_overriding_union. apply Map.in_to_self in I. right. exact I.
+  - apply Map.in_overriding_union. destruct IR as [z F]. apply Map.to_self_to_self in F as [I ->]. right. exact I.
+  - apply Map.to_self_to_self in F as [I ->]. reflexivity.
+Qed.
+
+
+
+(*
+Definition cant_bind_ctx (ctx : Map.to Term.term) : Map.set := Todo.
+Lemma cant_bind_spec ctx
+  : Map.Reflect (fun x => exists t, Map.InRange ctx t /\ (BoundIn.Term t x \/ UsedIn.Term t x)) $ cant_bind_ctx ctx.
+Proof. Todo.
+
+Lemma no_free_vars {ctx domain} (WF : WellFormedContextAcc ctx domain)
+  {t} (IR : Map.InRange ctx t) {x} (U : UsedIn.Term t x)
+  : Map.In ctx x.
+Proof.
+  destruct IR as [k F]. specialize (WF _ (cant_bind_spec _) _ _ F). cbn in WF.
+Qed.
+*)
+
+Lemma no_free_vars_acc {cant_bind context t} (WF : WellFormedInAcc cant_bind context t)
+  {x} (U : UsedIn.Term t x)
+  : Map.In context x.
+Proof.
+  generalize dependent x. induction WF; intros; cbn in *.
+  - invert U.
+  - invert U. exact I.
+  - invert U. { apply IHWF1. exact used_in_function. } apply IHWF2. exact used_in_argument.
+  - invert U. { apply IHWF1. exact used_in_type. } specialize (IHWF2 _ used_in_body). apply Map.find_tt in IHWF2.
+    apply Cb in IHWF2 as [[-> _] | F]. { contradiction not_shadowed. reflexivity. } apply Map.find_tt. exact F.
+  - invert U. 2: { apply IHWF1. exact used_in_another_case. } specialize (IHWF2 _ used_in_body).
+    apply Cb in IHWF2 as [B | I]. { apply not_shadowed in B as []. } exact I.
+Qed.
+
+
+
+Lemma domain_eq_acc {cant_bind acc ctx bound_or_used ctx'}
+  (E : unshadow_context_acc (Some (cant_bind, acc)) ctx = Some (bound_or_used, ctx')) {x}
+  : Map.In ctx' x <-> (Map.In acc x \/ Map.In ctx x).
+Proof.
+  unfold unshadow_context_acc in E. unfold Map.fold in E. rewrite MapCore.fold_spec in E.
+  assert (Iff : Map.In ctx x <-> exists y, SetoidList.InA MapCore.eq_key_elt (x, y) $ MapCore.bindings ctx). {
+    split; intros [y F]; exists y; apply MapCore.bindings_spec1; exact F. } rewrite Iff. clear Iff.
+  remember (MapCore.bindings ctx) as b eqn:Eb; clear ctx Eb. generalize dependent x. generalize dependent ctx'.
+  generalize dependent bound_or_used. generalize dependent acc. generalize dependent cant_bind.
+  induction b as [| [k v] tail IH]; intros. {
+    invert E. split. { intro I. left. exact I. } intros [I | [y I]]. { exact I. } invert I. }
+  rewrite NewNames.unfold_left in E. simpl fst in E. simpl snd in E. unfold unshadow_context_each in E at -1.
+  destruct unshadow_reserve_bindings as [[this_bindings this_unshadowed_term] |] eqn:E' in E. 2: {
+    refine match _ : False with end. clear cant_bind acc k v E' x IH.
+    induction tail. { discriminate E. } apply IHtail. exact E. }
+  specialize (IH _ _ _ _ E x) as ->. rewrite Map.in_overriding_add. split.
+  - intros [[-> | I] | [y I]]. { right. exists v. left. split; reflexivity. } { left. exact I. } right. exists y. right. exact I.
+  - intros [I | [y I]]. { left. right. exact I. } invert I. { left. left. apply H0. } right. exists y. exact H0.
+Qed.
+
+
+
+Lemma on_the_tin_context_acc_acc {so_far tail} (disj : Map.Disjoint so_far tail) {full_context}
+  (Rfc : Map.Reflect (fun x => Map.In so_far x \/ Map.In tail x) full_context) (WFsf : WellFormedContextAcc so_far full_context)
+  (Nfv : forall k v (F : Map.Find so_far k v \/ Map.Find tail k v) x (U : UsedIn.Term v x), Map.In full_context x)
+  {cant_bind_so_far} (Rsf : Map.Reflect (fun x => Map.In full_context x \/
+    exists k v, (Map.Find so_far k v /\ BoundIn.Term v x)) cant_bind_so_far)
+  {final_bound_or_used final_ctx} (E : unshadow_context_acc (Some (cant_bind_so_far, so_far)) tail =
+    Some (final_bound_or_used, final_ctx))
+  : WellFormedContextAcc final_ctx full_context.
+Proof.
+  unfold unshadow_context_acc in E. unfold Map.fold in E. rewrite MapCore.fold_spec in E.
+  eassert (disj' : forall k (Is : Map.In so_far k) v (It : SetoidList.InA MapCore.eq_key_elt (k, v) $
+    MapCore.bindings tail), False). { intros. eapply disj. { exact Is. }
+    exists v. apply MapCore.bindings_spec1. exact It. } clear disj. rename disj' into disj.
+  eassert (Rfc' : Map.Reflect (fun x => Map.In so_far x \/
+    exists y, SetoidList.InA MapCore.eq_key_elt (x, y) $ MapCore.bindings tail) full_context). {
+    intro x. rewrite (Rfc _). split; (intros [I | [y F']]; [left | right]; [exact I |]);
+    exists y; apply MapCore.bindings_spec1; exact F'. } clear Rfc. rename Rfc' into Rfc.
+  eassert (Nfv' : forall k v (F : Map.Find so_far k v \/ SetoidList.InA MapCore.eq_key_elt (k, v) $ MapCore.bindings tail)
+    x (U : UsedIn.Term v x), Map.In full_context x). { intros k' v' F' x U. eapply Nfv. 2: { exact U. }
+    destruct F' as [F' | F']; [left | right]. { exact F'. }
+    apply MapCore.bindings_spec1. exact F'. } clear Nfv. rename Nfv' into Nfv.
+  eassert (ND := MapCore.bindings_spec2w tail). remember (MapCore.bindings tail) as b eqn:Eb; clear tail Eb.
+  generalize dependent Nfv. generalize dependent Rfc. generalize dependent disj. generalize dependent Rsf.
+  generalize dependent WFsf. generalize dependent final_ctx. generalize dependent final_bound_or_used.
+  generalize dependent cant_bind_so_far. generalize dependent so_far.
+  induction ND as [| [this_name this_term] tail Nd ND IH]; intros. { invert E. eapply WFsf. }
+  rewrite NewNames.unfold_left in E. simpl fst in E. simpl snd in E. unfold unshadow_context_each in E at -1.
+  destruct unshadow_reserve_bindings as [[this_bindings this_unshadowed_term] |] eqn:E' in E. 2: {
+    refine match _ : False with end.
+    clear full_context this_name this_term Nd ND IH so_far disj Rfc cant_bind_so_far E' WFsf Nfv Rsf.
+    induction tail. { discriminate E. } apply IHtail. exact E. }
+  eapply IH. { exact E. }
+  - destruct WFsf as [UB WF]. cbn in UB. cbn in WF. split; intro; intros.
+    + apply Map.find_overriding_add in F1 as [[-> ->] | [N1 F1]];
+      apply Map.find_overriding_add in F2 as [[tmp ->] | [N2 F2]]; subst;
+      [| contradiction N2 | contradiction N1 |]; try reflexivity. eapply UB; eassumption.
+    + apply Map.find_overriding_add in F as [[-> ->] | [N F]]. 2: { eapply WF. exact F. }
+      eapply cant_bind_subset; [eapply (on_the_tin_bindings E') |]. {
+        intros. apply (used_idem E') in U. eapply Nfv. 2: { exact U. } right. left. split; reflexivity. }
+      intros x [] F. apply Map.union_set. left. apply Map.find_tt. apply Rsf. left. exists tt. exact F.
+  - intro x. rewrite Map.in_overriding_union. rewrite (bound_or_used E' _).
+    rewrite Map.in_overriding_union. rewrite (UsedIn.term_iff _ _). rewrite (Rsf _). split.
+    + intros [[B | [U | [[I | [k [v [F B]]]] | U]]] | [I | [k [v [F B]]]]].
+      * right. exists this_name. exists this_unshadowed_term. split. 2: { exact B. }
+        apply Map.find_overriding_add. left. split; reflexivity.
+      * apply (used_idem E') in U. left. eapply Nfv. 2: { exact U. } right. left. split; reflexivity.
+      * left. exact I.
+      * right. exists k. exists v. split. 2: { exact B. } apply Map.find_overriding_add. right. split. 2: { exact F. }
+        intros ->. eapply disj. { exists v. exact F. } left. split; reflexivity.
+      * left. eapply Nfv. 2: { exact U. } right. left. split; reflexivity.
+      * left. exact I.
+      * right. exists k. exists v. split. 2: { exact B. } apply Map.find_overriding_add. right. split. 2: { exact F. }
+        intros ->. eapply disj. { exists v. exact F. } left. split; reflexivity.
+    + intros [I | [k [v [F B]]]]. { left. right. right. left. left. exact I. }
+      apply Map.find_overriding_add in F as [[-> ->] | [N F]]. { left. left. exact B. }
+      right. right. exists k. exists v. split. { exact F. } exact B.
+  - intros. apply Map.in_overriding_add in Is as [-> | Is]. 2: { eapply disj. { exact Is. } right. exact It. }
+    eapply Nd. apply Map.eq_key_elt. exists v. exact It.
+  - intro x. rewrite (Rfc _). rewrite Map.in_overriding_add. split.
+    + intros [I | [y I]]. { left. right. exact I. }
+      invert I. { destruct H0; cbn in *; subst. left. left. reflexivity. } right. exists y. exact H0.
+    + intros [[-> | I] | [y I]]. { right. exists this_term. left. split; reflexivity. } { left. exact I. }
+      right. exists y. right. exact I.
+  - intros. destruct F as [F | F]. 2: { apply (Nfv k v). 2: { exact U. } right. right. exact F. }
+    apply Map.find_overriding_add in F as [[-> ->] | [N F]]. 2: { apply (Nfv k v). 2: { exact U. } left. exact F. }
+    apply (used_idem E') in U. eapply Nfv. 2: { exact U. } right. left. split; reflexivity.
+Qed.
+
+Lemma on_the_tin_context_acc {so_far tail} (disj : Map.Disjoint so_far tail) {full_context}
+  (Rfc : Map.Reflect (fun x => Map.In so_far x \/ Map.In tail x) full_context) (WFsf : WellFormedContextAcc so_far full_context)
+  (Nfv : forall k v (F : Map.Find so_far k v \/ Map.Find tail k v) x (U : UsedIn.Term v x), Map.In full_context x)
+  {cant_bind_so_far} (Rsf : Map.Reflect (fun x => Map.In full_context x \/
+    exists k v, (Map.Find so_far k v /\ BoundIn.Term v x)) cant_bind_so_far)
+  {final_bound_or_used final_ctx} (E : unshadow_context_acc (Some (cant_bind_so_far, so_far)) tail =
+    Some (final_bound_or_used, final_ctx))
+  : WellFormedContext final_ctx.
+Proof.
+  unfold WellFormedContext. intros. eapply on_the_tin_context_acc_acc; try exact E; try assumption.
+  - intro x. rewrite <- (D _). apply (domain_eq_acc E).
+  - destruct WFsf as [UB WF]. split; intro; intros. { eapply UB; eassumption. }
+    eapply cant_bind_subset; [eapply context_superset; [eapply WF |] |]. { exact F. }
+    + intros x [] I. apply Map.find_tt in I. apply Map.find_tt. apply Rfc in I. apply D. apply (domain_eq_acc E). exact I.
+    + intros x [] I. apply Map.find_tt in I. apply Map.find_tt. apply Rfc. apply D in I. apply (domain_eq_acc E) in I. exact I.
+  - intros. apply D. apply (domain_eq_acc E). apply Rfc. eapply Nfv. { exact F. } exact U.
+  - intro x. rewrite (Rsf _). rewrite (Rfc _). rewrite <- (D _). rewrite (domain_eq_acc E). reflexivity.
+Qed.
+
+Lemma on_the_tin_context_bindings
+  {context} (Nfv : forall k v (F : Map.Find context k v) x (U : UsedIn.Term v x), Map.In context x)
+  {domain} (D : Map.Domain context domain) {final_bound_or_used final_ctx} (E
+    : unshadow_context_reserve_bindings domain context = Some (final_bound_or_used, final_ctx))
+  : WellFormedContext final_ctx.
+Proof.
+  eapply on_the_tin_context_acc; try exact E.
+  - intros ? C. apply Map.empty_empty in C as [].
+  - intro x. rewrite (D _). split. { intro I. right. exact I. }
+    intros [I | I]. { apply Map.empty_empty in I as []. } exact I.
+  - split; cbn; intros. { invert F1. } invert F.
+  - intros. destruct F as [F | F]. { invert F. } apply D. eapply Nfv. { exact F. } exact U.
+  - intro x. split. { intro I. left. exact I. }
+    intros [I | [k [v [F B]]]]. { exact I. } invert F.
+Qed.
+
+Lemma on_the_tin_context_reserve
+  {context} (Nfv : forall k v (F : Map.Find context k v) x (U : UsedIn.Term v x), Map.In context x)
+  {domain} (D : Map.Domain context domain) {final_ctx} (E
+    : unshadow_context_reserve domain context = Some final_ctx)
+  : WellFormedContext final_ctx.
+Proof.
+  unfold unshadow_context_reserve in E. destruct unshadow_context_reserve_bindings as [[] |] eqn:E' in E; invert E.
+  eapply on_the_tin_context_bindings; try exact E'; assumption.
+Qed.
+
+Lemma on_the_tin_context
+  {context} (Nfv : forall k v (F : Map.Find context k v) x (U : UsedIn.Term v x), Map.In context x)
+  {final_ctx} (E : unshadow_context context = Some final_ctx)
+  : WellFormedContext final_ctx.
+Proof. eapply on_the_tin_context_reserve; try exact E. { exact Nfv. } apply Map.domain_domain. Qed.
